Add walk-through of attempts to prove LL(1) determinism

LL1/DeterminismProof.v
@@ -13,7 +13,7 @@ Inductive derivesProd {g : grammar} :
       In (x, gamma) g.(productions)
       -> derivesGamma gamma tokens f
       -> derivesProd x gamma tokens (Node x f)
-with derivesGamma {g : grammar} : 
+with derivesGamma {g : grammar} :
        list symbol -> list string -> forest -> Prop :=
      | derivesFnil : derivesGamma [] [] Fnil
      | derivesFcons : 
@@ -49,7 +49,7 @@ Lemma derivesSym_nil_nullable :
   forall tr g sym,
     (@derivesSym g) sym [] tr
     -> (@nullableSym g) sym.
- Proof.
+Proof.
   induction tr using tree_mutual_ind with
       (P := fun tr =>
               forall g sym,
@@ -393,29 +393,3342 @@ Proof.
     + apply IHgPre; auto.
 Qed.
 
-Lemma last_case :
+Lemma tree_eq_dec : forall (tr tr2 : tree),
+    {tr = tr2} + {~tr = tr2}.
+Proof.
+Admitted.
+
+Lemma forest_eq_dec : forall (f f2 : forest),
+    {f = f2} + {~f = f2}.
+Proof.
+Admitted.
+
+Lemma prefixes_eq :
+  forall (suf pre pre' : list string),
+    app pre suf = app pre' suf
+    -> pre = pre'.
+Proof.
+  induction suf; intros; simpl in *.
+  - repeat rewrite app_nil_r in H.
+    auto.
+  - assert (a :: suf = app [a] suf) by auto.
+    repeat rewrite H0 in H.
+    repeat rewrite app_assoc in H.
+    apply IHsuf in H.
+    apply app_inj_tail in H.
+    destruct H.
+    auto.
+Qed.
+
+Lemma suffixes_eq :
+  forall (pre suf suf' : list string),
+    app pre suf = app pre suf'
+    -> suf = suf'.
+Proof.
+  induction pre; intros; simpl in *.
+  - auto.
+  - inv H.
+    apply IHpre; auto.
+Qed.
+
+Fixpoint inF tr f :=
+  match f with
+  | Fnil => False
+  | Fcons tr' f' =>
+    tr = tr' \/ inF tr f'
+  end.
+
+Lemma forest_neq :
+  forall f f' tr tr',
+    Fcons tr f <> Fcons tr' f'
+    -> tr <> tr' \/ f <> f'.
+Proof.
+  intros.
+  destruct (forest_eq_dec f f').
+  - subst.
+    left.
+    unfold not; intros.
+    subst.
+    congruence.
+  - right; auto.
+Qed.
+
+Lemma eof_fgamma :
+  forall g la gamma,
+    (@firstGamma g) la gamma
+    -> la = EOF
+    -> False.
+Proof.
+  intros g la gamma H.
+  induction H using firstGamma_mutual_ind with
+      (P := fun la x gamma (pf : firstProd la x gamma) =>
+              la = EOF -> False)
+      (P0 := fun la gamma (pf : firstGamma la gamma) =>
+               la = EOF -> False)
+      (P1 := fun la sym (pf : firstSym la sym) =>
+               la = EOF -> False); intros.
+  - apply IHfirstGamma; trivial.
+  - apply IHfirstGamma; trivial.
+  - apply IHfirstGamma; trivial. 
+  - inv H.
+  - apply IHfirstGamma; trivial.
+Qed.
+
+Lemma derives_lookahead :
   forall tbl g,
     isParseTableFor tbl g
-    -> forall sufGamma preGamma x x2 word f f',
-      In (x, preGamma ++ NT x2 :: sufGamma) (productions g)
-      -> (@derivesGamma g) (NT x2 :: sufGamma) word f
-      -> (@derivesGamma g) (NT x2 :: sufGamma) word f'
-      -> f = f'.
+    -> forall tr sym word,
+      (@derivesSym g) sym word tr
+      -> (@firstSym g) (peek word) sym
+         \/ ((@nullableSym g) sym
+             /\ (@followSym g) (peek word) sym).
+Proof.
+  intros.
+  inv H0.
+  - left.
+    simpl.
+    constructor.
+  - destruct word.
+    + inv H1.
+      right.
+      simpl.
+      apply derivesGamma_nil_nullable in H2.
+      split.
+      * econstructor.
+        econstructor; eauto.
+      * eapply FoNu; eauto.
+        econstructor; eauto.
+    + inv H1.
+      left.
+      simpl.
+      apply derivesGamma_cons_firstGamma in H2.
+      econstructor.
+      econstructor; eauto.
+Qed.
+
+Lemma derivesGamma_lookahead :
+  forall tbl g,
+    isParseTableFor tbl g
+    -> forall gamma f word,
+      (@derivesGamma g) gamma word f
+      -> (@firstGamma g) (peek word) gamma
+         \/ (@nullableGamma g) gamma.
+Proof.
+  intros tbl g Htbl.
+  induction gamma; intros; simpl in *.
+  - inv H.
+    right; constructor.
+  - inv H.
+    destruct prefix; simpl in *.
+    + apply IHgamma in H5.
+      destruct H5.
+      * destruct suffix; simpl in *.
+        -- apply eof_fgamma in H.
+           ++ inv H.
+           ++ auto.
+        -- left.
+           destruct a.
+           ++ inv H2.
+           ++ eapply FiGammaTl.
+              ** inv H2.
+                 inv H1.
+                 apply derivesGamma_nil_nullable in H2.
+                 econstructor.
+                 econstructor; eauto.
+              ** auto.
+      * right.
+        destruct a.
+        -- inv H2.
+        -- eapply NuCons.
+           ++ inv H2.
+              inv H1.
+              apply derivesGamma_nil_nullable in H2.
+              econstructor.
+              econstructor; eauto.
+           ++ auto.
+    + destruct a.
+      * inv H2.
+        left.
+        constructor.
+        constructor.
+      * inv H2.
+        inv H0.
+        apply derivesGamma_cons_firstGamma in H1.
+        left.
+        constructor.
+        econstructor.
+        econstructor; eauto.
+Qed.
+
+Lemma derives_det :
+  forall tbl g,
+    isParseTableFor tbl g
+    -> forall sym word tr,
+      (@derivesTree g) sym word tr
+      -> forall tr',
+        (@derivesTree g) sym word tr'
+        -> tr = tr'.
+Proof.
+  intros tbl g Htbl sym word tr Hder.
+  induction Hder using derivesTree_mutual_ind with
+      (P := fun sym word tr =>
+              forall tr',
+                (@derivesTree g) sym word tr'
+                -> tr = tr')
+      (P0 := fun gsuf wsuf fsuf =>
+                 derivesForest gsuf wsuf fsuf
+                 -> forall x gpre wpre wpre' wsuf wsuf' fpre fpre' fsuf',
+                     In (x, gpre ++ gsuf) (productions g)
+                     -> derivesForest gpre wpre fpre
+                     -> derivesForest gpre wpre' fpre'
+                     -> derivesForest gsuf wsuf' fsuf'
+                     -> wpre ++ wsuf = wpre' ++ wsuf'
+                     -> wpre = wpre'
+                        /\ wsuf = wsuf'
+                        /\ fsuf = fsuf').
+
+  - intros.
+    inv H.
+    auto.
+
+  - intros.
+    inv H1.
+    assert (gamma0 = gamma) by admit; subst.
+    eapply IHHder with (gpre := nil)
+                       (wpre := nil)
+                       (fpre := Fnil) in H4; eauto.
+    + destruct H4.
+      destruct H2.
+      subst; auto.
+    + constructor.
+    + constructor.
+
+  - intros.
+    inv H.
+    inv H3.
+    repeat rewrite app_nil_r in *.
+    subst.
+    assert (wsuf = nil) by admit.
+    subst.
+    repeat (split; auto).
+    rewrite app_nil_r.
+    auto.
+    
+  - intros.
+    inv H1.
+    
+
+
+Lemma derives_det :
+  forall tbl g,
+    isParseTableFor tbl g
+    -> forall tr tr'
+              x
+              gpre wpre wpre' fpre fpre'
+              sym  wmid wmid'
+              gsuf wsuf wsuf' fsuf fsuf',
+      In (x, gpre ++ sym :: gsuf) (productions g)
+         
+      -> (@derivesGamma g) gpre wpre fpre
+      -> (@derivesGamma g) gpre wpre' fpre'
+                           
+      -> (@derivesSym g) sym wmid tr
+      -> (@derivesSym g) sym wmid' tr'
+                           
+      -> (@derivesGamma g) gsuf wsuf fsuf
+      -> (@derivesGamma g) gsuf wsuf' fsuf'
+                           
+      -> wpre ++ wmid = wpre' ++ wmid'
+      -> wmid ++ wsuf = wmid' ++ wsuf'
+                              
+      -> wpre = wpre'
+         /\ wmid = wmid'
+         /\ wsuf = wsuf'
+         /\ tr = tr'.
+Proof.
+  intros tbl g Htbl.
+  induction tr using tree_mutual_ind with
+      (P0 := fun fmid =>
+               forall fmid'
+                      x
+                      gpre wpre wpre' fpre fpre'
+                      gmid wmid wmid'
+                      gsuf wsuf wsuf' fsuf fsuf',
+      In (x, gpre ++ gmid ++ gsuf) (productions g)
+         
+      -> (@derivesGamma g) gpre wpre fpre
+      -> (@derivesGamma g) gpre wpre' fpre'
+                           
+      -> (@derivesGamma g) gmid wmid fmid
+      -> (@derivesGamma g) gmid wmid' fmid'
+                           
+      -> (@derivesGamma g) gsuf wsuf fsuf
+      -> (@derivesGamma g) gsuf wsuf' fsuf'
+                           
+      -> wpre ++ wmid = wpre' ++ wmid'
+      -> wmid ++ wsuf = wmid' ++ wsuf'
+                              
+      -> wpre = wpre'
+         /\ wmid = wmid'
+         /\ wsuf = wsuf'
+         /\ fmid = fmid').
+  - intros.
+    inv H2.
+    + inv H3.
+      inv H7.
+      apply prefixes_eq in H6.
+      subst.
+      repeat (split; auto).
+    + inv H8.
+      
+  - intros.
+    inv H2; inv H3.
+    inv H8; inv H9.
+    assert (gamma0 = gamma) by admit; subst.
+Abort.
+
+Fixpoint forest_det f g :=
+  match f with
+  | Fnil => forall gamma word f',
+      (@derivesGamma g) gamma word f
+      -> (@derivesGamma g) gamma word f'
+      -> f = f'
+  | Fcons tr tl =>
+    (forall sym word tr',
+        (@derivesSym g) sym word tr
+        -> (@derivesSym g) sym word tr'
+        -> tr = tr')
+    /\ forest_det tl g
+  end.
+
+Lemma ambig :
+  forall g sym word tr,
+    (@derivesSym g) sym word tr
+    -> forall tr',
+      (@derivesSym g) sym word tr'
+      -> tr <> tr'
+      -> exists x gamma gamma' word' f f',
+          In (x, gamma) (productions g)
+          /\ In (x, gamma') (productions g)
+          /\ (@derivesGamma g) gamma word' f
+          /\ (@derivesGamma g) gamma' word' f'
+          /\ gamma <> gamma'.
+Proof.
+  intros g sym word tr Hder.
+  induction Hder using derivesSym_mut_ind
+    with (P := fun x gamma word tr
+                   (pf : (@derivesProd g) x gamma word tr) =>
+                 forall tr',
+                   (@derivesProd g) x gamma word tr'
+                   -> tr <> tr'
+                   -> exists x gamma gamma' word' f f',
+                       In (x, gamma) (productions g)
+                       /\ In (x, gamma') (productions g)
+                       /\ (@derivesGamma g) gamma word' f
+                       /\ (@derivesGamma g) gamma' word' f'
+                       /\ gamma <> gamma')
+         (P0 := fun gsuf wsuf fsuf
+                   (pf : (@derivesGamma g) gsuf wsuf fsuf) =>
+                  forall x gpre wpre fpre fsuf',
+                    In (x, gpre ++ gsuf) (productions g)
+                    -> (@derivesGamma g) gpre wpre fpre
+                    -> (@derivesGamma g) gsuf wsuf fsuf'
+                    -> fsuf <> fsuf'
+                   -> exists x gamma gamma' word' f f',
+                       In (x, gamma) (productions g)
+                       /\ In (x, gamma') (productions g)
+                       /\ (@derivesGamma g) gamma word' f
+                       /\ (@derivesGamma g) gamma' word' f'
+                       /\ gamma <> gamma').
+  - intros.
+    inv H.
+    eapply IHHder with (gpre := nil)
+      in H2; eauto.
+    + constructor.
+    + destruct (forest_eq_dec f f0).
+      * subst.
+        congruence.
+      * auto.
+
+  - intros.
+    inv H1.
+    congruence.
+
+  - intros.
+    inv H1.
+
+
+
+
+
+
+
+
+
+
+
+
+    
+    
+Lemma derives_det :
+  forall tbl g,
+    isParseTableFor tbl g
+    -> forall tr tr' sym word,
+      (@derivesSym g) sym word tr
+      -> (@derivesSym g) sym word tr'
+      -> tr = tr'.
 Proof.
   intros tbl g Htbl.
   pose proof Htbl as Htbl'.
   destruct Htbl as [Hmin Hcom].
-  induction sufGamma as [| sym syms].
+  induction tr using tree_mutual_ind with
+      (P0 := fun f =>
+               forall f' gamma word,
+                 (@derivesGamma g) gamma word f
+                 -> (@derivesGamma g) gamma word f'
+                 ->  f = f').
   
+  - intros.
+    inv H; inv H0; auto.
+    inv H1.
+
+  - intros.
+    inv H; inv H0.
+    inv H1; inv H2.
+    assert (gamma0 = gamma) by admit. (* get this from LL(1) *)
+    subst.
+    erewrite IHtr; eauto.
+
+  - intros.
+    inv H.
+    inv H0.
+    auto.
+
+  - intros.
+    inv H; inv H0.
 Abort.
 
-Lemma derivesSym_det : 
+
+
+
+Lemma derives_det :
   forall tbl g,
     isParseTableFor tbl g
-    -> forall f f' x pre gamma word,
+    -> forall tr tr' sym wpre wpre' wsuf wsuf',
+      (@derivesSym g) sym wsuf tr
+      -> (@derivesSym g) sym wsuf' tr'
+      -> wpre ++ wsuf = wpre' ++ wsuf'
+      -> wpre = wpre'
+         /\ wsuf = wsuf'
+         /\ tr = tr'.
+Proof.
+  intros tbl g Htbl.
+  pose proof Htbl as Htbl'.
+  destruct Htbl as [Hmin Hcom].
+  induction tr using tree_mutual_ind with
+      (P0 := fun fsuf =>
+               forall fsuf'
+                      gpre wpre wpre' fpre fpre'
+                      gsuf wsuf wsuf',
+                 (@derivesGamma g) gpre wpre fpre
+                 -> (@derivesGamma g) gpre wpre' fpre'
+                 -> (@derivesGamma g) gsuf wsuf fsuf
+                 -> (@derivesGamma g) gsuf wsuf' fsuf'
+                 ->  wpre ++ wsuf = wpre' ++ wsuf'
+                 -> wpre = wpre'
+                    /\ wsuf = wsuf'
+                    /\ fsuf = fsuf').
+  - admit.
+  - intros.
+    inv H; inv H0.
+    inv H2; inv H3.
+    assert (gamma0 = gamma) by admit.
+    subst.
+    eapply IHtr with (gpre := nil)
+                     (wpre := nil)
+                     (wpre' := nil) in H0; eauto.
+Abort.    
+
+
+
+(* trying just prefixes *)
+Lemma derives_det :
+  forall tbl g,
+    isParseTableFor tbl g
+    -> forall tr tr' x
+              gpre wpre wpre' fpre fpre'
+              sym  wmid wmid'
+              gsuf,
+              (* gsuf wsuf wsuf' fsuf fsuf', *)
+      In (x, gpre ++ sym :: gsuf) (productions g)
+      -> (@derivesGamma g) gpre wpre fpre
+      -> (@derivesGamma g) gpre wpre' fpre'
+      -> (@derivesSym g) sym wmid tr
+      -> (@derivesSym g) sym wmid' tr'
+(*
+      -> (@derivesGamma g) gsuf wsuf fsuf
+      -> (@derivesGamma g) gsuf wsuf' fsuf'
+*)
+      -> wpre ++ wmid = wpre' ++ wmid'
+      -> wpre = wpre'
+         /\ wmid = wmid'
+         /\ tr = tr'.
+Proof.
+  intros tbl g Htbl.
+  induction tr using tree_mutual_ind with
+      (P0 := fun fsuf =>
+               forall 
+                      gpre wpre wpre' fpre fpre'
+                      gsuf wsuf wsuf'      fsuf',
+                 (@derivesGamma g) gpre wpre fpre
+                 -> (@derivesGamma g) gpre wpre' fpre'
+                 -> (@derivesGamma g) gsuf wsuf fsuf
+                 -> (@derivesGamma g) gsuf wsuf' fsuf'
+                 -> wpre ++ wsuf = wpre' ++ wsuf'
+                 -> wpre = wpre'
+                    /\ wsuf = wsuf'
+                    /\ fsuf = fsuf').
+  - intros.
+    inv H2.
+    + inv H3.
+      apply prefixes_eq in H4.
+      subst.
+      repeat (split; auto).
+    + inv H5.
+
+  - intros.
+    inv H2; inv H3.
+    inv H5; inv H6.
+    assert (gamma0 = gamma) by admit.
+    subst.
+    eapply IHtr with
+        (gpre := gpre)
+        (wpre := wpre)
+        (wpre' := wpre')
+        (gsuf := gamma)
+        (wsuf := wmid)
+        (wsuf' := wmid') in H3; eauto.
+    destruct H3.
+    destruct H5.
+    subst.
+    repeat (split; auto).
+
+  - intros.
+    inv H1; inv H2.
+    repeat rewrite app_nil_r in *; subst.
+    repeat (split; auto).
+
+  - intros.
+    inv H1; inv H2.
+    pose proof H10 as H10'.
+    eapply IHtr0 with
+        (gpre := gpre ++ [hdSym])
+        (wpre := wpre ++ prefix)
+        (wpre' := wpre' ++ prefix0) in H10; eauto.
+    + destruct H10.
+      destruct H2.
+      subst.
+      eapply IHtr with
+          (gpre := gpre)
+          (wpre := wpre)
+          (wpre' := wpre')
+          (wmid := prefix)
+          (wmid' := prefix0) in H5; eauto.
+      * destruct H5.
+        destruct H4.
+        subst.
+        repeat (split; auto).
+      * admit.
+    + eapply derives_app.
+      * eauto.
+      * admit.
+    + admit.
+    + repeat rewrite <- app_assoc.
+      auto.
+Abort. (* pretty close! *)
+
+
+(* three-part word *)
+Lemma derives_det :
+  forall tbl g,
+    isParseTableFor tbl g
+    -> forall tr tr' x
+              gpre wpre wpre' fpre fpre'
+              sym  wmid wmid'
+              gsuf wsuf wsuf' fsuf fsuf',
+      
+      In (x, gpre ++ sym :: gsuf) (productions g)
+         
+      -> (@derivesGamma g) gpre wpre fpre
+      -> (@derivesGamma g) gpre wpre' fpre'
+                           
+      -> (@derivesSym g) sym wmid tr
+      -> (@derivesSym g) sym wmid' tr'
+
+      -> (@derivesGamma g) gsuf wsuf fsuf
+      -> (@derivesGamma g) gsuf wsuf' fsuf'
+
+      -> wmid ++ wsuf = wmid' ++ wsuf'
+      -> wpre ++ wmid ++ wsuf = wpre' ++ wmid' ++ wsuf'
+
+      -> tr = tr'.
+Proof.
+  intros tbl g Htbl.
+  induction tr using tree_mutual_ind with
+      (P0 := fun fsuf =>
+               forall x
+                      gpre wpre wpre' fpre fpre'
+                      gsuf wsuf wsuf'      fsuf',
+                 In (x, gpre ++ gsuf) (productions g)
+                 -> (@derivesGamma g) gpre wpre fpre
+                 -> (@derivesGamma g) gpre wpre' fpre'
+                 -> (@derivesGamma g) gsuf wsuf fsuf
+                 -> (@derivesGamma g) gsuf wsuf' fsuf'
+                 -> wpre ++ wsuf = wpre' ++ wsuf'
+                 -> fsuf = fsuf').
+  - intros.
+    inv H2.
+    + inv H3.
+      auto.
+    + inv H8.
+
+  - intros.
+    inv H2; inv H3.
+    inv H8; inv H9.
+    assert (gamma0 = gamma) by admit.
+    subst.
+    eapply IHtr with
+        (gpre := nil)
+        (wpre := nil)
+        (wpre' := nil)
+        (gsuf := gamma)
+        (wsuf := wmid)
+        (wsuf' := wmid') in H3; eauto.
+Abort. (* IH doesn't have the right form *)
+
+Lemma derives_det :
+  forall tbl g,
+    isParseTableFor tbl g
+    -> forall sym word tr,
+      (@derivesSym g) sym word tr
+      -> forall tr',
+        (@derivesSym g) sym word tr'
+        -> tr = tr'.
+Proof.
+  intros tbl g Htbl sym word tr Hder.
+  induction Hder using derivesSym_mut_ind with
+      (P := fun x gamma word tr
+                (pf : (@derivesProd g) x gamma word tr) =>
+              forall tr',
+                (@derivesProd g) x gamma word tr'
+                -> tr = tr')
+      (P0 := fun gsuf wsuf fsuf
+                 (pf : (@derivesGamma g) gsuf wsuf fsuf) =>
+               forall x gpre wpre fpre,
+                 In (x, gpre ++ gsuf) (productions g)
+                 -> (@derivesGamma g) gpre wpre fpre
+                 -> forall wpre' fpre' wsuf' fsuf',
+                     (@derivesGamma g) gpre wpre' fpre'
+                     -> (@derivesGamma g) gsuf wsuf' fsuf'
+                     -> wpre ++ wsuf = wpre' ++ wsuf'
+                     -> wpre = wpre'
+                        /\ wsuf = wsuf'
+                        /\ fsuf = fsuf').
+  - intros.
+    inv H.
+    eapply IHHder with
+        (gpre := nil)
+        (wpre := nil) in H1; eauto.
+    + destruct H1.
+      destruct H1.
+      subst; auto.
+    + constructor.
+    + constructor.
+      
+  - intros.
+    inv H2.
+    repeat rewrite app_nil_r in *.
+    subst.
+    repeat (split; auto).
+
+  - intros.
+    inv H2.
+    eapply IHHder0 with 
+        (gpre := gpre ++ [hdSym])
+        (wpre := wpre ++ prefix)
+        (wpre' := wpre' ++ prefix0)
+        (fpre := appF fpre (Fcons hdTree Fnil))
+        (fpre' := appF fpre' (Fcons hdTree0 Fnil))
+        (wsuf' := suffix0) in H9; eauto.
+    * destruct H9.
+      destruct H4.
+      subst.
+      (* can't apply IHHder here *)
+      admit.
+      * assert (hdSym :: tlSyms = [hdSym] ++ tlSyms) by auto.
+        rewrite H2 in H.
+        rewrite app_assoc in H.
+        eauto.
+      * apply derives_app with
+            (gPre := gpre)
+            (wPre := wpre)
+            (fPre := fpre)
+            (gSuf := [hdSym])
+            (wSuf := prefix)
+            (fSuf := Fcons hdTree Fnil).
+        -- auto.
+        -- assert (prefix = prefix ++ nil) by
+              (rewrite app_nil_r; auto).
+           rewrite H2.
+           eapply derivesFcons; eauto.
+           constructor.
+      * apply derives_app with
+            (gPre := gpre)
+            (wPre := wpre')
+            (fPre := fpre')
+            (gSuf := [hdSym])
+            (wSuf := prefix0)
+            (fSuf := Fcons hdTree0 Fnil).
+        -- auto.
+        -- assert (prefix0 = prefix0 ++ nil) by
+              (rewrite app_nil_r; auto).
+           rewrite H2.
+           eapply derivesFcons; eauto.
+           constructor.
+      * repeat rewrite <- app_assoc.
+        auto.
+        
+  - intros.
+    inv H.
+    auto.
+
+  - intros.
+    inv d.
+
+    inv H.
+    inv H3.
+    assert (gamma0 = gamma) by admit.
+    subst.
+    apply IHHder.
+    constructor; auto.
+Abort. (* So close! *)
+
+
+(* Most promising so far? *)
+Lemma derives_det :
+  forall tbl g,
+    isParseTableFor tbl g
+    -> forall sym wmid tr,
+      (@derivesSym g) sym wmid tr
+      -> forall x
+                gpre wpre fpre
+                gsuf wsuf fsuf,
+        In (x, gpre ++ sym :: gsuf) (productions g)
+        -> (@derivesGamma g) gpre wpre fpre
+        -> (@derivesGamma g) gsuf wsuf fsuf
+        -> forall wpre' fpre'
+                  wmid' tr'
+                  wsuf' fsuf',
+            (@derivesSym g) sym wmid' tr'
+            -> (@derivesGamma g) gpre wpre' fpre'
+            -> (@derivesGamma g) gsuf wsuf' fsuf'
+            -> wpre ++ wmid ++ wsuf = wpre' ++ wmid' ++ wsuf'
+            -> wmid = wmid'
+               /\ tr = tr'.
+Proof.
+  intros tbl g Htbl sym wmid tr Hder.
+  induction Hder using derivesSym_mut_ind with
+      (P := fun x gamma word tr
+                (pf : (@derivesProd g) x gamma word tr) =>
+              forall tr',
+                (@derivesProd g) x gamma word tr'
+                -> tr = tr')
+      (P0 := fun gsuf wsuf fsuf
+                 (pf : (@derivesGamma g) gsuf wsuf fsuf) =>
+               forall x gpre wpre fpre,
+                 In (x, gpre ++ gsuf) (productions g)
+                 -> (@derivesGamma g) gpre wpre fpre
+                 -> forall wpre' fpre' wsuf' fsuf',
+                     (@derivesGamma g) gpre wpre' fpre'
+                     -> (@derivesGamma g) gsuf wsuf' fsuf'
+                     -> wpre ++ wsuf = wpre' ++ wsuf'
+                     -> wpre = wpre'
+                        /\ wsuf = wsuf'
+                        /\ fsuf = fsuf').
+  - intros.
+    inv H.
+    eapply IHHder with
+        (gpre := nil)
+        (wpre := nil) in H1; eauto.
+    + destruct H1.
+      destruct H1.
+      subst; auto.
+    + constructor.
+    + constructor.
+      
+  - intros.
+    inv H2.
+    repeat rewrite app_nil_r in *.
+    subst.
+    repeat (split; auto).
+
+  - intros.
+    inv H2.
+    eapply IHHder0 with
+        (gpre := gpre ++ [hdSym])
+        (wpre := wpre ++ prefix)
+        (wpre' := wpre' ++ prefix0) in H9; eauto.
+    + destruct H9.
+      destruct H4.
+      subst.
+      eapply IHHder with
+          (wpre := wpre)
+          (wpre' := wpre')
+          (wmid' := prefix0)
+          (wsuf := suffix0)
+          (wsuf' := suffix0) in H6; eauto.
+      destruct H6.
+      subst.
+      apply prefixes_eq in H2.
+      repeat (split; auto).
+    + admit.
+    + admit.
+    + admit.
+    + repeat rewrite <- app_assoc.
+      auto.
+
+  - intros.
+    inv H2.
+    split; auto.
+
+  - intros.
+    inv H2.
+    assert (gamma0 = gamma) by admit.
+    subst.
+Abort.
+(* Looking even better, though! *)
+
+(* trying to remove the different suffixes -- that works *)
+Lemma derives_det :
+  forall tbl g,
+    isParseTableFor tbl g
+    -> forall sym wmid tr,
+      (@derivesSym g) sym wmid tr
+      -> forall x
+                gpre wpre fpre
+                gsuf wsuf fsuf,
+        In (x, gpre ++ sym :: gsuf) (productions g)
+        -> (@derivesGamma g) gpre wpre fpre
+        -> (@derivesGamma g) gsuf wsuf fsuf
+        -> forall wpre' fpre'
+                  wmid' tr',
+            (@derivesSym g) sym wmid' tr'
+            -> (@derivesGamma g) gpre wpre' fpre'
+            -> wpre ++ wmid = wpre' ++ wmid'
+            -> wpre = wpre'
+               /\wmid = wmid'
+               /\ tr = tr'.
+Proof.
+  intros tbl g Htbl sym wmid tr Hder.
+  induction Hder using derivesSym_mut_ind with
+      (P := fun rx gamma wmid tr
+                (pf : (@derivesProd g) rx gamma wmid tr) =>
+              forall lx gpre wpre fpre
+                        gsuf wsuf fsuf,
+                In (lx, gpre ++ (NT rx) :: gsuf)
+                   (productions g)
+                -> (@derivesGamma g) gpre wpre fpre
+                -> (@derivesGamma g) gsuf wsuf fsuf
+                -> forall wpre' fpre' wmid' tr',
+                    (@derivesGamma g) gpre wpre' fpre'
+                    -> (@derivesProd g) rx gamma wmid' tr'
+                    -> wpre ++ wmid = wpre' ++ wmid'
+                    -> wpre = wpre'
+                       /\ wmid = wmid'
+                       /\ tr = tr')
+      (P0 := fun gsuf wsuf fsuf
+                 (pf : (@derivesGamma g) gsuf wsuf fsuf) =>
+               forall x gpre wpre fpre,
+                 In (x, gpre ++ gsuf) (productions g)
+                 -> (@derivesGamma g) gpre wpre fpre
+                 -> forall wpre' fpre' wsuf' fsuf',
+                     (@derivesGamma g) gpre wpre' fpre'
+                     -> (@derivesGamma g) gsuf wsuf' fsuf'
+                     -> wpre ++ wsuf = wpre' ++ wsuf'
+                     -> wpre = wpre'
+                        /\ wsuf = wsuf'
+                        /\ fsuf = fsuf').
+  - intros.
+Abort. (* IH problems *)
+
+  
+
+Lemma derives_det :
+    forall tbl g,
+    isParseTableFor tbl g
+    -> forall sym wpre tr syms wsuf f,
+        (@derivesSym g) sym wpre tr
+        -> (@derivesGamma g) syms wsuf f
+        -> forall wpre' tr' wsuf' f',
+            (@derivesSym g) sym wpre' tr'
+            -> (@derivesGamma g) syms wsuf' f'
+            -> wpre ++ wsuf = wpre' ++ wsuf'
+            -> wpre = wpre'
+               /\ wsuf = wsuf'
+               /\ tr = tr.
+Proof.
+  intros tbl g Htbl sym wpre tr syms wsuf f Hders.
+  induction Hders using derivesSym_mut_ind with
+      (P := fun 
+      In (x, gpre ++ sym :: gsuf) (productions g)
+      -> (@derivesGamma g) gpre wpre fpre
+      -> (@derivesSym g) sym wmid tr
+      -> (@derivesGamma g) gsuf wsuf fsuf
+
+      -> forall wpre' fpre' wmid' tr' wsuf' fsuf',
+          wpre ++ wmid ++ wsuf = wpre' ++ wmid' ++ wsuf'
+          -> (@derivesGamma g) gpre wpre' fpre'
+          -> (@derivesSym g) sym wmid' tr'
+          -> (@derivesGamma g) gsuf wsuf' fsuf'
+                         
+          -> tr = tr'.
+
+(* three-part word *)
+Lemma derives_det :
+  forall tbl g,
+    isParseTableFor tbl g
+                    
+    -> forall x
+              gpre wpre fpre
+              sym  wmid tr
+              gsuf wsuf fsuf,
+      In (x, gpre ++ sym :: gsuf) (productions g)
+      -> (@derivesGamma g) gpre wpre fpre
+      -> (@derivesSym g) sym wmid tr
+      -> (@derivesGamma g) gsuf wsuf fsuf
+
+      -> forall wpre' fpre' wmid' tr' wsuf' fsuf',
+          wpre ++ wmid ++ wsuf = wpre' ++ wmid' ++ wsuf'
+          -> (@derivesGamma g) gpre wpre' fpre'
+          -> (@derivesSym g) sym wmid' tr'
+          -> (@derivesGamma g) gsuf wsuf' fsuf'
+                         
+          -> tr = tr'.
+Proof.
+  intros tbl g Htbl.
+  induction tr using tree_mutual_ind with
+      (P0 := fun fsuf =>
+               forall x
+                      gpre wpre wpre' fpre fpre'
+                      gsuf wsuf wsuf'      fsuf',
+                 In (x, gpre ++ gsuf) (productions g)
+                 -> (@derivesGamma g) gpre wpre fpre
+                 -> (@derivesGamma g) gpre wpre' fpre'
+                 -> (@derivesGamma g) gsuf wsuf fsuf
+                 -> (@derivesGamma g) gsuf wsuf' fsuf'
+                 -> wpre ++ wsuf = wpre' ++ wsuf'
+                 -> fsuf = fsuf').
+
+
+
+
+
+
+    
+(* Input is empty, symbol could be T or NT *)
+Lemma derives_nil_det :
+  forall tbl g,
+    isParseTableFor tbl g
+    -> forall tr tr' sym,
+      (@derivesSym g) sym [] tr
+      -> (@derivesSym g) sym [] tr'
+      -> tr = tr'.
+Proof.
+  intros tbl g Htbl.
+  pose proof Htbl as Htbl'.
+  destruct Htbl as [Hmin Hcom].
+  induction tr using tree_mutual_ind with
+      (P0 := fun f =>
+               forall f' x pre gamma,
+                 In (x, pre ++ gamma) (productions g)
+                 -> (@derivesGamma g) gamma [] f
+                 -> (@derivesGamma g) gamma [] f'
+                 -> f = f').
+  - intros.
+    inv H.
+    inv H1.
+
+  - intros.
+    inv H.
+    inv H1.
+    inv H0.
+    inv H1.
+    assert (gamma0 = gamma) by admit.
+    subst.
+    assert (gamma = [] ++ gamma) by auto.
+    rewrite H1 in H.
+    erewrite IHtr; eauto.
+
+  - intros.
+    inv H0.
+    inv H1.
+    auto.
+
+  - intros.
+    inv H0.
+    inv H1.
+    assert (prefix = []) by admit.
+    assert (prefix0 = []) by admit.
+    assert (suffix = []) by admit.
+    assert (suffix0 = []) by admit.
+    subst.
+    assert (hdSym :: tlSyms = [hdSym] ++ tlSyms) by auto.
+    rewrite H0 in H.
+    rewrite app_assoc in H.
+    erewrite IHtr; eauto.
+    erewrite IHtr0; eauto.
+Admitted.
+
+Lemma derives_cons_det :
+  forall tbl g,
+    isParseTableFor tbl g
+    -> forall tr tr' sym tok toks,
+      (@derivesSym g) sym (tok :: toks) tr
+      -> (@derivesSym g) sym (tok :: toks) tr'
+      -> tr = tr'.
+Proof.
+  intros tbl g Htbl.
+  pose proof Htbl as Htbl'.
+  destruct Htbl as [Hmin Hcom].
+  induction tr using tree_mutual_ind with
+      (P0 := fun f =>
+               forall f' x gpre gsuf tok toks,
+                 In (x, gpre ++ gsuf) (productions g)
+                 -> (@derivesGamma g) gsuf (tok :: toks) f
+                 -> (@derivesGamma g) gsuf (tok :: toks) f'
+                 -> f = f').
+  - intros.
+    inv H.
+    + inv H0.
+      auto.
+    + inv H1.
+
+  - intros.
+    inv H; inv H0.
+    inv H1; inv H2.
+    assert (gamma0 = gamma) by admit.
+    subst.
+    erewrite IHtr with (gpre := nil); eauto.
+
+  - intros.
+    inv H0.
+
+  - intros.
+    inv H0.
+    inv H1.
+    destruct prefix; simpl in *.
+    + destruct prefix0; simpl in *.
+      * subst.
+        eapply IHtr0 with (gpre := gpre ++ [hdSym])
+          in H9; eauto.
+        -- subst.
+           eapply derives_nil_det in H6; eauto.
+        subst; auto.
+        -- admit.
+      * inv H4.
+        admit.
+    + destruct prefix0; simpl in *.
+      * inv H2.
+        admit.
+      * inv H2.
+        inv H4.
+        
+
+Lemma derives_det :
+  forall tbl g,
+    isParseTableFor tbl g
+    -> forall tr tr' sym wpre wpre' wsuf wsuf',
+      (@derivesSym g) sym wpre tr
+      -> (@derivesSym g) sym wpre' tr'
+      -> wpre ++ wsuf = wpre' ++ wsuf'
+      -> peek (wpre ++ wsuf) = peek (wpre' ++ wsuf')
+      -> wpre = wpre'
+         /\ wsuf = wsuf'
+         /\ tr = tr'.
+Proof.
+  intros tbl g Htbl.
+  induction tr using tree_mutual_ind with
+      (P0 := fun f =>
+               forall f' gamma wpre wpre' wsuf wsuf',
+                 (@derivesGamma g) gamma wpre f
+                 -> (@derivesGamma g) gamma wpre' f'
+                 -> wpre ++ wsuf = wpre' ++ wsuf'
+                 -> peek (wpre ++ wsuf) = peek (wpre' ++ wsuf')
+                 -> wpre = wpre'
+                    /\ wsuf = wsuf'
+                    /\ f = f').
+  - intros.
+    inv H.
+    + inv H0.
+      inv H1.
+      repeat (split; auto).
+    + inv H3.
+      
+  - intros.
+    inv H; inv H0.
+    inv H3; inv H4.
+    assert (gamma0 = gamma).
+    { pose proof H9 as H9'.
+      apply derivesGamma_lookahead with (tbl := tbl) in H9; auto.
+      pose proof H0 as H0'.
+      apply derivesGamma_lookahead with (tbl := tbl) in H0; auto.
+      destruct wpre; simpl in *.
+      - destruct H9.
+        + apply eof_fgamma in H3; auto.
+          inv H3.
+        + destruct wpre'; simpl in *.
+          * destruct H0.
+            -- apply eof_fgamma in H0; auto.
+               inv H0.
+            -- admit.
+          * admit.
+      - destruct wpre'.
+
+Abort.
+
+
+
+
+
+
+
+
+
+    
+
+Lemma derives_det :
+  forall tbl g,
+    isParseTableFor tbl g
+    -> forall tr tr' sym word,
+      (@derivesSym g) sym word tr
+      -> (@derivesSym g) sym word tr'
+      -> tr = tr'.
+Proof.
+  intros tbl g Htbl.
+  pose proof Htbl as Htbl'.
+  destruct Htbl as [Hmin Hcom].
+  induction tr using tree_mutual_ind with
+      (P0 := fun f =>
+               forall f' gamma word,
+                 (@derivesGamma g) gamma word f
+                 -> (@derivesGamma g) gamma word f'
+                 ->  f = f').
+  - admit.
+  - admit.
+  - admit.
+  - intros.
+    inv H; inv H0.
+    eapply derives_lookahead in H5.
+    
+
+Lemma derives_with_res_and_stuff :
+    forall tbl g,
+    isParseTableFor tbl g
+    -> forall tr tr'
+              x gPre sym gSuf
+              wPre wPre' wSuf wSuf'
+              f f' res res',
+        In (x, gPre ++ sym :: gSuf) (productions g)
+        -> (@derivesSym g) sym wPre tr
+        -> (@derivesSym g) sym wPre' tr'
+        -> (@derivesGamma g) gSuf wSuf f
+        -> (@derivesGamma g) gSuf wSuf' f'
+        -> wPre ++ wSuf ++ res = wPre' ++ wSuf' ++ res'
+        -> (wPre = wPre'
+            /\ (wSuf ++ res) = (wSuf' ++ res')
+            /\ tr = tr').
+Proof.
+  intros tbl g Htbl.
+  induction tr using tree_mutual_ind with
+      (P0 := fun f =>
+               forall f' x gPre gSuf wPre wPre' wSuf wSuf',
+                 In (x, gPre ++ gSuf) (productions g)
+                 -> (@derivesGamma g) gSuf wPre f
+                 -> (@derivesGamma g) gSuf wPre' f'
+                 -> wPre ++ wSuf = wPre' ++ wSuf'
+                 -> wPre = wPre'
+                    /\ wSuf = wSuf'
+                    /\ f = f').
+  - intros.
+    inv H0.
+    + inv H1.
+      inv H4.
+      repeat (split; auto).
+    + inv H5.
+
+  - intros.
+    inv H0; inv H1.
+    inv H5; inv H6.
+    assert (gamma0 = gamma) by admit.
+    subst.
+    eapply IHtr with (gPre := nil) in H1; eauto.
+    destruct H1.
+    destruct H5.
+    subst.
+    repeat (split; auto).
+
+  - intros.
+    inv H0; inv H1.
+    simpl in *; subst.
+    repeat (split; auto).
+
+  - intros.
+    inv H0; inv H1.
+    eapply IHtr with
+        (wSuf := suffix)
+        (wSuf' := suffix0)
+        (res := wSuf)
+        (res' := wSuf') in H4; eauto.
+    + destruct H4.
+      destruct H1.
+      subst.
+      eapply IHtr0 in H9; eauto.
+      * destruct H9.
+        destruct H3.
+        subst.
+        repeat (split; auto).
+      * assert (hdSym :: tlSyms = [hdSym] ++ tlSyms) by auto.
+        rewrite H0 in H.
+        rewrite app_assoc in H.
+        eauto.
+    + repeat rewrite <- app_assoc in H2.
+      auto.
+Abort.
+
+
+Lemma derives_det :
+  forall tbl g,
+    isParseTableFor tbl g
+    -> forall tr tr' sym word,
+      (@derivesSym g) sym word tr
+      -> (@derivesSym g) sym word tr'
+      -> tr = tr'.
+Proof.
+  intros tbl g Htbl.
+  pose proof Htbl as Htbl'.
+  destruct Htbl as [Hmin Hcom].
+  induction tr using tree_mutual_ind with
+      (P0 := fun fpre =>
+               forall x fpre' gpre gsuf wpre wpre' wsuf wsuf' fsuf fsuf',
+                 (@derivesGamma g) gpre wpre fpre
+                 -> (@derivesGamma g) gpre wpre' fpre'
+                 -> (@derivesGamma g) gsuf wsuf fsuf
+                 -> (@derivesGamma g) gsuf wsuf' fsuf'
+                 -> wpre ++ wsuf = wpre' ++ wsuf'
+                 -> wpre = wpre'
+                    /\ wsuf = wsuf'
+                    /\ fpre = fpre').
+  - intros.
+    inv H.
+    + inv H0; auto.
+    + inv H1.
+
+  - intros.
+    inv H; inv H0.
+    inv H1; inv H2.
+    assert (gamma0 = gamma) by admit; subst.
+    eapply IHtr with (gpre := gamma)
+                     (gsuf := nil) in H0; eauto.
+    + destruct H0.
+      destruct H1.
+      subst; auto.
+    + constructor.
+    + constructor.
+
+  - intros.
+    inv H.
+    inv H0.
+    simpl in *; subst.
+    repeat (split; auto).
+
+  - intros.
+    inv H.
+    inv H0.
+Abort.
+
+
+(* Here's what we really want to prove *)
+Lemma derives_det :
+  forall tbl g,
+    isParseTableFor tbl g
+    -> forall tr tr' sym word,
+      (@derivesSym g) sym word tr
+      -> (@derivesSym g) sym word tr'
+      -> tr = tr'.
+Proof.
+  intros tbl g Htbl.
+  pose proof Htbl as Htbl'.
+  destruct Htbl as [Hmin Hcom].
+  induction tr using tree_mutual_ind with
+      (P0 := fun f =>
+               forall f' gamma word,
+                 (@derivesGamma g) gamma word f
+                 -> (@derivesGamma g) gamma word f'
+                 ->  f = f').
+  
+  - intros.
+    inv H; inv H0; auto.
+    inv H1.
+
+  - intros.
+    inv H; inv H0.
+    inv H1; inv H2.
+    assert (gamma0 = gamma) by admit. (* get this from LL(1) *)
+    subst.
+    erewrite IHtr; eauto.
+
+  - intros.
+    inv H.
+    inv H0.
+    auto.
+
+  - intros.
+    inv H; inv H0.
+    + (* here, we're going to get stuck because we don't know
+         whether prefix = prefix0. It would help if we knew
+         that prefix and prefix0 shared the first lookahead
+         token *)
+Abort.
+
+Fixpoint lenF f :=
+  match f with
+  | Fnil => 0
+  | Fcons tr f' => 1 + lenF f'
+  end.
+
+(* trying the length idea *)
+Lemma derives_det :
+  forall tbl g,
+    isParseTableFor tbl g
+    -> forall tr tr' sym word,
+      (@derivesSym g) sym word tr
+      -> (@derivesSym g) sym word tr'
+      -> tr = tr'.
+Proof.
+  intros tbl g Htbl.
+  pose proof Htbl as Htbl'.
+  destruct Htbl as [Hmin Hcom].
+  induction tr using tree_mutual_ind with
+      (P0 := fun f =>
+               forall f' gamma word,
+                 (@derivesGamma g) gamma word f
+                 -> (@derivesGamma g) gamma word f'
+                 -> lenF f = lenF f'
+                    /\ f = f').
+  - admit.
+  - intros.
+    inv H; inv H0.
+    inv H1; inv H2.
+    assert (gamma0 = gamma) by admit.
+    subst.
+    eapply IHtr in H0; eauto.
+    destruct H0.
+    subst; auto.
+  - intros.
+    inv H.
+    inv H0.
+    split; auto.
+  - intros.
+    inv H.
+    inv H0.
+    simpl.
+
+
+
+Lemma derives_det :
+  forall tbl g,
+    isParseTableFor tbl g
+    -> forall tr tr' sym word,
+      (@derivesSym g) sym word tr
+      -> (@derivesSym g) sym word tr'
+      -> tr = tr'.
+Proof.
+  intros tbl g Htbl.
+  pose proof Htbl as Htbl'.
+  destruct Htbl as [Hmin Hcom].
+  induction tr using tree_mutual_ind with
+      (P0 := fun fSuf =>
+               forall gPre wPre wPre' fPre fPre'
+                      gSuf wSuf wSuf'      fSuf',
+                 (@derivesGamma g) gPre wPre fPre
+                 -> (@derivesGamma g) gPre wPre' fPre'
+                 -> (@derivesGamma g) gSuf wSuf fSuf
+                 -> (@derivesGamma g) gSuf wSuf' fSuf'
+                 -> wPre ++ wSuf = wPre' ++ wSuf'
+                 -> wPre = wPre'
+                    /\ wSuf = wSuf'
+                    /\ fSuf = fSuf').
+  - intros.
+    inv H.
+    + inv H0.
+      auto.
+    + inv H1.
+
+  - intros.
+    inv H; inv H0.
+    inv H1; inv H2.
+    assert (gamma0 = gamma) by admit.
+    subst.
+    eapply IHtr with
+        (gPre := nil)
+        (wPre := nil)
+        (wPre' := nil)
+        (fPre := Fnil)
+        (fPre' := Fnil) in H0; eauto.
+    + destruct H0.
+      destruct H1.
+      simpl in H2.
+      subst.
+      auto.
+    + constructor.
+    + constructor.
+
+  - intros.
+    inv H1.
+    inv H2.
+    repeat rewrite app_nil_r in *.
+    subst.
+    repeat (split; auto).
+
+  - intros.
+    inv H1.
+    inv H2.
+    eapply IHtr0 with
+        (gPre := gPre ++ [hdSym])
+        (wPre := wPre ++ prefix)
+        (wPre' := wPre' ++ prefix0)
+        (wSuf := suffix) in H10; eauto.
+    + destruct H10.
+      destruct H2.
+      subst.
+Abort.
+
+(* Here's what we really want to prove *)
+Lemma derives_det :
+  forall tbl g,
+    isParseTableFor tbl g
+    -> forall tr tr' x gPre sym gSuf wPre wPre' wSuf wSuf' f f',
+      In (x, gPre ++ sym :: gSuf) (productions g)
+      -> (@derivesSym g) sym wPre tr
+      -> (@derivesSym g) sym wPre' tr'
+      -> (@derivesGamma g) gSuf wSuf f
+      -> (@derivesGamma g) gSuf wSuf' f'
+      -> wPre ++ wSuf = wPre' ++ wSuf'
+      -> wPre = wPre'
+         /\ wSuf = wSuf'
+         /\ tr = tr'.
+Proof.
+  intros tbl g Htbl.
+  pose proof Htbl as Htbl'.
+  destruct Htbl as [Hmin Hcom].
+  induction tr using tree_mutual_ind with
+      (P0 := fun fSuf =>
+               forall gPre gSuf
+                      wPre wPre' wSuf wSuf'
+                      fPre fPre'      fSuf',
+                 (@derivesGamma g) gPre wPre fPre
+                 -> (@derivesGamma g) gPre wPre' fPre'
+                 -> (@derivesGamma g) gSuf wSuf fSuf
+                 -> (@derivesGamma g) gSuf wSuf' fSuf'
+                 -> wPre ++ wSuf = wPre' ++ wSuf'
+                 -> wPre = wPre'
+                    /\ wSuf = wSuf'
+                    /\ fSuf = fSuf').
+  - intros.
+    inv H0.
+    + inv H1.
+      inv H4.
+      repeat (split; auto).
+    + inv H5.
+
+  - intros.
+    inv H0; inv H1.
+    inv H5; inv H6.
+    assert (gamma0 = gamma) by admit.
+    subst.
+Abort.
+  
+
+
+Lemma only_one_span :
+  forall tbl g,
+    isParseTableFor tbl g
+    -> forall tr tr' sym word,
+      (@derivesSym g) sym word tr
+      -> (@derivesSym g) sym word tr'
+      -> span tr = span tr'.
+Proof.
+  intros tbl g.
+  induction tr using tree_mutual_ind with
+      (P0 := fun f =>
+               forall f' gamma word,
+                 (@derivesGamma g) gamma word f
+                 -> (@derivesGamma g) gamma word f'
+                 -> spanForest f = spanForest f').
+  - intros.
+    inv H0.
+    + inv H1.
+      auto.
+    + inv H2.
+
+  - intros.
+    inv H0; inv H1.
+    inv H2; inv H3.
+    simpl.
+    assert (gamma0 = gamma) by admit.
+    subst.
+    eapply IHtr; eauto.
+
+  - intros.
+    inv H0; inv H1.
+    auto.
+
+  - intros.
+    simpl.
+    inv H0; inv H1.
+    simpl.
+Abort.
+
+
+
+Lemma only_one_split :
+  forall tbl g,
+    isParseTableFor tbl g
+    -> forall gPre gSuf
+              wPre wPre' wSuf wSuf'
+              fPre fPre' fSuf fSuf',
+      (@derivesGamma g) gPre wPre fPre
+      -> (@derivesGamma g) gPre wPre' fPre'
+      -> (@derivesGamma g) gSuf wSuf fSuf
+      -> (@derivesGamma g) gSuf wSuf' fSuf'
+      -> wPre ++ wSuf = wPre' ++ wSuf'
+      -> appF fPre fSuf = appF fPre' fSuf'
+      -> wPre = wPre'
+         /\ wSuf = wSuf'.
+Proof.
+  intros tbl g Htbl.
+  induction gPre as [| psym psyms]; intros.
+  - inv H; inv H0.
+    simpl in *; subst.
+    split; auto.
+  - inv H; inv H0.
+    simpl in H4.
+    inv H4.
+    assert (prefix0 = prefix) by admit.
+    subst.
+    repeat rewrite <- app_assoc in H3.
+    apply suffixes_eq in H3.
+    eapply IHpsyms with (gSuf := gSuf)
+                        (wPre := suffix)
+                        (wPre' := suffix0)
+                        (wSuf := wSuf)
+                        (wSuf' := wSuf') in H11; eauto.
+    destruct H11.
+    subst.
+    split; auto.
+Admitted.
+
+
+Lemma derives_det :
+  forall tbl g,
+    isParseTableFor tbl g
+    -> forall tr tr' sym word,
+      (@derivesSym g) sym word tr
+      -> (@derivesSym g) sym word tr'
+      -> tr = tr'.
+Proof.
+  intros tbl g Htbl.
+  pose proof Htbl as Htbl'.
+  destruct Htbl as [Hmin Hcom].
+  induction tr using tree_mutual_ind with
+      (P0 := fun f =>
+               forall f' gamma word,
+                 (@derivesGamma g) gamma word f
+                 -> (@derivesGamma g) gamma word f'
+                 -> f = f').
+  - intros.
+    inv H.
+    + inv H0.
+      auto.
+    + inv H1.
+
+  - intros.
+    inv H.
+    inv H0.
+    inv H1; inv H2.
+    assert (gamma0 = gamma) by admit.
+    subst.
+    erewrite IHtr; eauto.
+
+  - intros.
+    inv H.
+    inv H0.
+    auto.
+
+  - intros.
+    inv H.
+    inv H0.
+Abort.
+  
+
+(* Problem : in the last case, we can't prove that 
+   gamma and gamma0 are equal *)
+Lemma derives_det :
+  forall tbl g,
+    isParseTableFor tbl g
+    -> forall sym wPre tr,
+      (@derivesSym g) sym wPre tr
+      -> forall wPre' wSuf wSuf' tr',
+        (@derivesSym g) sym wPre' tr'
+        -> wPre ++ wSuf = wPre' ++ wSuf'
+        -> wPre = wPre'
+           /\ wSuf = wSuf'
+           /\ tr = tr'.
+Proof.
+  intros tbl g Htbl sym word tr Hder.
+  induction Hder using derivesSym_mut_ind with
+      (P := fun x gamma wPre tr
+                (pf : (@derivesProd g) x gamma wPre tr) =>
+              forall wPre' wSuf wSuf' tr',
+                (@derivesProd g) x gamma wPre' tr'
+                -> wPre ++ wSuf = wPre' ++ wSuf'
+                -> wPre = wPre'
+                   /\ wSuf = wSuf'
+                   /\ tr = tr')
+      (P0 := fun gamma wPre f
+                 (pf : (@derivesGamma g) gamma wPre f) =>
+                  forall wPre' wSuf wSuf' f',
+                    (@derivesGamma g) gamma wPre' f'
+                    -> wPre ++ wSuf = wPre' ++ wSuf'
+                    -> wPre = wPre'
+                       /\ wSuf = wSuf'
+                       /\ f = f').
+  - intros.
+    inv H.
+    eapply IHHder in H2; eauto.
+    destruct H2.
+    destruct H2.
+    subst.
+    repeat (split; auto).
+
+  - intros.
+    inv H.
+    simpl in *.
+    subst.
+    repeat (split; auto).
+
+  - intros.
+    inv H.
+    eapply IHHder with
+        (wSuf := suffix ++ wSuf)
+        (wSuf' := suffix0 ++ wSuf') in H3; eauto.
+    + destruct H3.
+      destruct H1.
+      subst.
+      eapply IHHder0 in H6; eauto.
+      destruct H6.
+      destruct H2.
+      subst.
+      repeat (split; auto).
+    + repeat rewrite app_assoc.
+      auto.
+      
+  - intros.
+    inv H.
+    inv H0.
+    repeat (split; auto).
+
+  - intros.
+    inv H.
+    assert (gamma0 = gamma) by admit.
+    subst.
+Abort.
+
+
+
+
+
+
+
+
+
+
+
+
+
+
+
+
+  
+
+Lemma derives_det :
+  forall tbl g,
+    isParseTableFor tbl g
+    -> forall tr tr' sym word,
+      (@derivesSym g) sym word tr
+      -> (@derivesSym g) sym word tr'
+      -> tr = tr'.
+Proof.
+  intros tbl g Htbl.
+  pose proof Htbl as Htbl'.
+  destruct Htbl as [Hmin Hcom].
+  induction tr using tree_mutual_ind with
+      (P0 := fun fSuf =>
+               forall x gPre gSuf,
+                 In (x, gPre ++ gSuf) (productions g)
+                 -> (forall wPre wPre'
+                            wSuf wSuf'
+                            fPre fPre',
+                        (@derivesGamma g) gPre wPre fPre
+                        -> (@derivesGamma g) gPre wPre' fPre'
+                        -> wPre ++ wSuf = wPre' ++ wSuf'
+                        -> wPre = wPre'
+                           /\ wSuf = wSuf'
+                           /\ fPre = fPre')
+                 -> forall wPre fPre
+                           wPre' fPre'
+                           wSuf wSuf'
+                           fSuf',
+                     (@derivesGamma g) gPre wPre fPre
+                     -> (@derivesGamma g) gPre wPre' fPre'
+                     -> (@derivesGamma g) gSuf wSuf fSuf
+                     -> (@derivesGamma g) gSuf wSuf' fSuf'
+                     -> wPre ++ wSuf = wPre' ++ wSuf'
+                     -> wPre = wPre'
+                        /\ wSuf = wSuf'
+                        /\ fSuf = fSuf').
+
+  - intros.
+    inv H.
+    + inv H0.
+      auto.
+    + inv H1.
+
+  - intros.
+    inv H; inv H0.
+    inv H1; inv H2.
+    assert (gamma0 = gamma) by admit.
+    subst.
+    eapply IHtr with (gPre := nil)
+                     (wPre := nil)
+                     (wPre' := nil) in H0; eauto.
+    + destruct H0.
+      destruct H1.
+      subst.
+      auto.
+    + intros.
+      inv H1; inv H2.
+      simpl in *; subst.
+      repeat (split; auto).
+    + constructor.
+    + constructor.
+
+  - intros.
+    inv H3.
+    inv H4.
+    repeat rewrite app_nil_r in *; subst.
+    repeat (split; auto).
+
+  - intros.
+    inv H3; inv H4.
+    eapply H0 with (wPre := wPre)
+                   (wPre' := wPre') in H2; eauto.
+    destruct H2.
+    destruct H3.
+    subst.
+    eapply IHtr0 with
+        (gPre := gPre ++ [hdSym])
+        (gSuf := tlSyms) in H12; eauto.
+    + destruct H12.
+      destruct H4.
+      subst.
+      eapply IHtr in H7; eauto.
+      subst.
+      repeat (split; auto).
+    + assert (hdSym :: tlSyms = [hdSym] ++ tlSyms) by auto.
+      rewrite H2 in H.
+      rewrite app_assoc in H.
+      eauto.
+    + admit.
+    + admit.
+    + admit.
+Abort.
+    
+
+
+(* SOME THINGS TO TRY TODAY
+   ========================
+   - What do tr and tr' tell us about word and word' ?
+
+   - Can we show that if words are equal and trees are not equal,
+     then there are two (x, gamma)'s that derive the same word?
+
+   - Go back to earlier attempts, but add the fact that gPre accepts
+     some wPre *)     
+
+
+
+Lemma ambig_exists :
+  forall g tr tr' sym word,
+    (@derivesSym g) sym word tr
+    -> (@derivesSym g) sym word tr'
+    -> tr <> tr'
+    -> exists x2 gamma1 gamma2 word' f f',
+        In (x2, gamma1) (productions g)
+        /\ In (x2, gamma2) (productions g)
+        /\ (@derivesGamma g) gamma1 word' f
+        /\ (@derivesGamma g) gamma2 word' f'
+        /\ gamma1 <> gamma2.
+Proof.
+  intro g.
+  induction tr using tree_mutual_ind with
+      (P0 := fun f =>
+               forall f'
+                      x gPre wPre fPre
+                      gSuf gSuf' wSuf,
+                 In (x, gPre ++ gSuf) (productions g)
+                 -> In (x, gPre ++ gSuf') (productions g)
+                 -> (@derivesGamma g) gPre wPre fPre
+                 -> (@derivesGamma g) gSuf wSuf f
+                 -> (@derivesGamma g) gSuf' wSuf f'
+                 -> f <> f'
+                 -> exists x gamma1 gamma2 word' f1 f2,
+                     In (x, gamma1) (productions g)
+                     /\ In (x, gamma2) (productions g)
+                     /\ (@derivesGamma g) gamma1 word' f1
+                     /\ (@derivesGamma g) gamma2 word' f2
+                     /\ gamma1 <> gamma2).
+
+  - intros.
+    admit.
+    
+
+  - intros.
+    inv H; inv H0.
+    inv H2; inv H3.
+    destruct (list_eq_dec symbol_eq_dec gamma gamma0).
+    + subst.
+      eapply IHtr with (gPre := nil)
+                       (wPre := nil)
+                       (fPre := Fnil) in H0; eauto.
+      * constructor.
+      * unfold not; intros; congruence.
+    + exists s; exists gamma; exists gamma0.
+      repeat eexists; eauto.
+
+  - intros.
+    inv H2; inv H3.
+    + congruence.
+    + exists x.
+      exists gPre.
+      exists (gPre ++ hdSym :: tlSyms).
+      exists wPre.
+      exists fPre.
+      exists (appF fPre (Fcons hdTree tlTrees)).
+      repeat (split; auto).
+      * admit.
+      * admit.
+      * admit.
+
+  - intros.
+    inv H2.
+    inv H3.
+    + admit.
+    + 
+
+  - intros.
+    inv H; inv H0.
+ 
+
+
+    
+      * admit.
+        (*destruct H2.
+        repeat destruct H0.
+        destruct H2.
+        destruct H3.
+        destruct H4.
+        exists x.
+        exists (x0 ++ x1).
+        exists (x0 ++ x2).
+        repeat eexists; repeat (split; eauto). auto. auto.
+        repeat eexists; eauto. *)
+      * unfold not; intros.
+        subst.
+        congruence.
+    + exists s. exists gamma; exists gamma'; exists word;
+                  exists f; exists f0.
+      repeat (split; auto).
+
+  - intros.
+    exists x; exists gPre; exists gSuf; exists gSuf';
+      exists word; exists Fnil; exists f'.
+    repeat (split; auto).
+    destruct (list_eq_dec symbol_eq_dec gSuf gSuf').
+    + subst.
+      inv H1.
+      inv H2.
+      congruence.
+    + auto.
+
+  - intros.
+    
+                                          
+
+
+                    fSuf =>
+               forall x
+                      gPre wPre fPre
+                      gSuf wSuf 
+                      gSuf' wSuf' fSuf',
+                 In (x, gPre ++ gSuf) (productions g)
+                 -> In (x, gPre ++ gSuf') (productions g)
+                 -> (@derivesGamma g) gPre wPre fPre
+                 -> (@derivesGamma g) gSuf wSuf fSuf
+                 -> (@derivesGamma g) gSuf' wSuf' fSuf'
+                 -> (fSuf = fSuf' -> gSuf = gSuf'
+                                     /\ wSuf = wSuf')
+                    /\ (fSuf <> fSuf' -> gSuf <> gSuf'
+                                   \/ wSuf <> wSuf')).
+  induction word as [| tok toks]; intros.
+  - inv H.
+    inv H0.
+    destruct 
+  
+
+
+  
+Lemma what_syms_and_trees_tells_us :
+  forall tbl g,
+    isParseTableFor tbl g
+    -> forall tr tr' sym sym' word word',
+      (@derivesSym g) sym word tr
+      -> (@derivesSym g) sym' word' tr'
+      -> (tr = tr' -> sym = sym'
+                      /\ word = word')
+         /\ (tr <> tr' -> sym <> sym'
+                          \/ word <> word').
+Proof.
+  intros tbl g Htbl.
+  pose proof Htbl as Htbl'.
+  destruct Htbl as [Hmin Hcom].
+  induction tr using tree_mutual_ind with
+      (P0 := fun fSuf =>
+               forall x
+                      gPre wPre fPre
+                      gSuf wSuf 
+                      gSuf' wSuf' fSuf',
+                 In (x, gPre ++ gSuf) (productions g)
+                 -> In (x, gPre ++ gSuf') (productions g)
+                 -> (@derivesGamma g) gPre wPre fPre
+                 -> (@derivesGamma g) gSuf wSuf fSuf
+                 -> (@derivesGamma g) gSuf' wSuf' fSuf'
+                 -> (fSuf = fSuf' -> gSuf = gSuf'
+                                     /\ wSuf = wSuf')
+                    /\ (fSuf <> fSuf' -> gSuf <> gSuf'
+                                   \/ wSuf <> wSuf')).
+
+  - intros.
+    inv H.
+    + inv H0.
+      * split; intros.
+        -- inv H.
+           split; auto.
+        -- left.
+           unfold not; intros.
+           congruence.
+      * inv H.
+        split; intros.
+        -- congruence.
+        -- left; congruence.
+    + inv H1.
+
+  - intros.
+    inv H.
+    inv H1.
+    inv H0.
+    + split; intros.
+      * congruence.
+      * left; congruence.
+    + inv H.
+      split; intros.
+      * inv H.
+        eapply IHtr with (gPre := nil)
+                         (wPre := nil)
+                         (fPre := Fnil)
+                         (gSuf := gamma) in H1; eauto.
+        -- destruct H1.
+           destruct H; auto.
+        -- constructor.
+      * destruct (string_dec s x).
+        -- subst.
+           destruct (list_eq_dec string_dec word word').
+           ++ subst.
+              assert (gamma0 = gamma) by admit.
+              subst.
+              eapply IHtr with (gPre := nil)
+                               (wPre := nil)
+                               (fPre := Fnil)
+                               (gSuf := gamma) in H1; eauto.
+              ** destruct H1.
+                 destruct (forest_eq_dec f f0).
+                 --- congruence.
+                 --- apply H2 in n.
+                     destruct n; congruence.
+              ** constructor.
+           ++ right; congruence.
+        -- left; congruence.
+
+  - intros.
+    inv H2.
+    inv H3.
+    + split; intros.
+      * split; auto.
+      * congruence.
+    + split; intros.
+      * congruence.
+      * left; congruence.
+
+  - intros.
+    inv H2.
+    inv H3.
+    + split; intros.
+      * congruence.
+      * left; congruence.
+    + split; intros.
+      * inv H3.
+        eapply IHtr with (sym := hdSym)
+                         (word := prefix) in H2; eauto.
+        destruct H2.
+        destruct H2; subst; auto.
+        eapply IHtr0 with (gPre := gPre ++ [hdSym0])
+                          (wPre := wPre ++ prefix0)
+                          (fPre := appF fPre
+                                        (Fcons hdTree Fnil))
+                          (wSuf := suffix) in H4; eauto.
+        
+        -- destruct H4.
+           destruct H2; auto; subst.
+           split; auto.
+        -- assert (hdSym0 :: tlSyms =
+                   [hdSym0] ++ tlSyms) by auto.
+           rewrite H2 in H.
+           rewrite app_assoc in H.
+           eauto.
+        -- assert (hdSym0 :: tlSyms0 = [hdSym0] ++ tlSyms0)
+            by auto.
+           rewrite H2 in H0.
+           rewrite app_assoc in H0.
+           auto.
+        -- eapply derives_app; eauto.
+           assert (prefix0 = prefix0 ++ nil)
+                  by (rewrite app_nil_r; auto).
+           rewrite H2.
+           eapply derivesFcons with (hdSym := hdSym0)
+                                    (prefix := prefix0)
+                                    (suffix1 := nil)
+                                    (hdTree0 := hdTree)
+                                    (tlSyms1 := nil)
+                                    (tlTrees0 := Fnil).
+           ++ auto.
+           ++ constructor.
+      * Abort.
+
+
+Lemma what_syms_and_trees_tells_us :
+  forall tbl g,
+    isParseTableFor tbl g
+    -> forall tr tr' sym sym' word word',
+      (@derivesSym g) sym word tr
+      -> (@derivesSym g) sym' word' tr'
+      -> (tr = tr' -> sym = sym'
+                      /\ word = word')
+         /\ (tr <> tr' -> sym <> sym'
+                          \/ word <> word').
+Proof.
+  intros tbl g Htbl.
+  pose proof Htbl as Htbl'.
+  destruct Htbl as [Hmin Hcom].
+  induction tr using tree_mutual_ind with
+      (P0 := fun f =>
+               forall f' gamma gamma' word word',
+                 (@derivesGamma g) gamma word f
+                 -> (@derivesGamma g) gamma' word' f'
+                 -> (f = f' -> gamma = gamma'
+                               /\ word = word')
+                    /\ (f <> f' -> gamma <> gamma'
+                                   \/ word <> word')).
+
+  - intros.
+    inv H.
+    + inv H0.
+      * split; intros.
+        -- inv H.
+           split; auto.
+        -- left.
+           unfold not; intros.
+           congruence.
+      * inv H.
+        split; intros.
+        -- congruence.
+        -- left; congruence.
+    + inv H1.
+
+  - intros.
+    inv H.
+    inv H1.
+    inv H0.
+    + split; intros.
+      * congruence.
+      * left; congruence.
+    + inv H.
+      pose proof H1 as H1'.
+      eapply IHtr in H1; eauto.
+      destruct H1.
+      split; intros.
+      * inv H2.
+        destruct H; auto.
+      * destruct (string_dec s x).
+        -- subst.
+           destruct (list_eq_dec string_dec word word').
+           ++ subst.
+              assert (gamma0 = gamma) by admit.
+              subst.
+              destruct (forest_eq_dec f f0).
+              ** congruence.
+              ** apply H1 in n.
+                 destruct n; congruence.
+           ++ auto.
+        -- left; congruence.
+
+  - intros.
+    inv H.
+    inv H0.
+    + split; intros.
+      * split; auto.
+      * congruence.
+    + split; intros.
+      * congruence.
+      * left; congruence.
+
+  - intros.
+    inv H.
+    inv H0.
+    + split; intros.
+      * congruence.
+      * left; congruence.
+    + split; intros.
+      * inv H0.
+        eapply IHtr with (word := prefix) in H; eauto.
+        destruct H.
+        eapply IHtr0 with (word := suffix) in H1; eauto.
+        destruct H1.
+        destruct H; auto.
+        subst.
+        destruct H1; auto.
+        subst.
+        split; auto.
+      * destruct (list_eq_dec string_dec (prefix ++ suffix)
+                              (prefix0 ++ suffix0)).
+        -- pose proof H as H'.
+           eapply IHtr with (word := prefix) in H; eauto.
+           destruct H.
+           pose proof H1 as H1'.
+           eapply IHtr0 with (word := suffix) in H1; eauto.
+           destruct H1.
+           destruct (tree_eq_dec tr hdTree).
+           ++ subst.
+              assert (hdSym = hdSym0 /\ prefix = prefix0)
+                by auto.
+              destruct H4; subst.
+              apply suffixes_eq in e; subst.
+              destruct (forest_eq_dec f tlTrees).
+              ** subst; congruence.
+              ** apply H3 in n.
+                 destruct n.
+                 --- left; congruence.
+                 --- congruence.
+           ++ apply H2 in n.
+              ** destruct n.
+                 --- left; congruence.
+                 --- admit. (* stuck! *)
+        -- right; auto.
+Admitted.
+
+
+
+
+
+
+
+
+
+
+(* Maybe try this with just the "positive" part? *)
+Lemma what_sym_and_words_tells_us :
+  forall tbl g,
+    isParseTableFor tbl g
+    -> forall tr tr' x gamma gamma' word word',
+      (@derivesProd g) x gamma word tr
+      -> (@derivesProd g) x gamma' word' tr'
+      -> (word = word'
+          -> gamma = gamma
+             /\ tr = tr')
+         /\ (word <> word'
+             -> gamma <> gamma'
+                /\ tr <> tr').
+Proof.
+  intros tbl g Htbl.
+  pose proof Htbl as Htbl'.
+  destruct Htbl as [Hmin Hcom].
+  induction tr using tree_mutual_ind with
+      (P0 := fun fSuf =>
+               forall fSuf' x gPre gSuf gSuf'
+                      wPre wSuf wSuf' fPre,
+                 In (x, gPre ++ gSuf) (productions g)
+                 -> In (x, gPre ++ gSuf') (productions g)
+                 -> (@derivesGamma g) gPre wPre fPre 
+                 -> (@derivesGamma g) gSuf wSuf fSuf
+                 -> (@derivesGamma g) gSuf' wSuf' fSuf'
+                 -> (wSuf = wSuf'
+                     -> gSuf = gSuf'
+                        /\ fSuf = fSuf')
+                    /\ (wSuf <> wSuf'
+                        -> gSuf <> gSuf'
+                           /\ fSuf <> fSuf')).
+
+  - intros.
+    inv H.
+
+  - intros.
+    inv H.
+    inv H0.
+    split; intros.
+    + subst.
+      assert (gamma' = gamma) by admit.
+      subst.
+      assert (gamma = [] ++ gamma) by auto.
+      rewrite H0 in H.
+      eapply IHtr in H1; eauto.
+      * destruct H1.
+        destruct H1; auto.
+        subst.
+        split; auto.
+      * econstructor.
+    + assert (gamma = [] ++ gamma) by auto.
+      rewrite H2 in H6.
+      assert (gamma' = [] ++ gamma') by auto.
+      rewrite H3 in H.
+      eapply IHtr with (gPre := nil)
+                       (gSuf := gamma)
+                       (wSuf := word) in H1; eauto.
+      * destruct H1.
+        apply H4 in H0.
+        destruct H0.
+        split; congruence.
+      * constructor.
+
+  - intros.
+    inv H2.
+    inv H3.
+    + split; intros.
+      * split; auto.
+      * congruence.
+    + split; intros.
+      * exfalso.
+        assert (prefix = nil) by admit.
+        assert (suffix = nil) by admit.
+        subst.
+        destruct wPre as [| tok toks].
+        -- assert ((@derivesGamma g) (gPre ++ hdSym :: tlSyms)
+                                     []
+                                     (appF fPre
+                                           (Fcons hdTree tlTrees))).
+           { admit. }
+           assert ((@derivesGamma g) gPre
+                                     []
+                                     (appF fPre
+                                           (Fcons hdTree tlTrees))).
+           { admit. }
+           apply derivesGamma_nil_nullable in H5.
+           apply derivesGamma_nil_nullable in H6.
+           assert ((@isLookaheadFor g) EOF (NT x) gPre).
+           { admit. }
+           assert ((@isLookaheadFor g) EOF (NT x)
+                                       (gPre ++ hdSym :: tlSyms)).
+           { admit. }
+           apply Hcom in H7.
+           apply Hcom in H8.
+           destruct H7 as [m [Hsf Hlf]].
+           destruct H8 as [m' [Hsf' Hlf']].
+           assert (gPre =
+                   (gPre ++ hdSym :: tlSyms)) by congruence.
+           admit.
+
+        -- admit.
+      * split; congruence.
+
+  - intros.
+    inv H2.
+    inv H3.
+    + split; intros.
+      * admit.
+      * split; congruence.
+    + split; intros.
+      * 
+
+
+
+
+
+
+
+
+
+
+      
+
+
+
+  
+
+Lemma what_sym_and_words_tells_us :
+  forall tbl g,
+    isParseTableFor tbl g
+    -> forall tr tr' sym sym' word word',
+      (@derivesSym g) sym word tr
+      -> (@derivesSym g) sym' word' tr'
+      -> (sym = sym'
+          -> word = word'
+          -> tr = tr')
+         /\ (sym <> sym'
+             -> word <> word'
+             -> tr <> tr').
+Proof.
+  intros tbl g Htbl.
+  pose proof Htbl as Htbl'.
+  destruct Htbl as [Hmin Hcom].
+  induction tr using tree_mutual_ind with
+      (P0 := fun f =>
+               forall f' gamma gamma' word word',
+                 (@derivesGamma g) gamma word f
+                 -> (@derivesGamma g) gamma' word' f'
+                 -> (gamma = gamma'
+                     -> word = word'
+                     -> f = f')
+                    /\ (gamma <> gamma'
+                        -> word <> word'
+                        -> f <> f')).
+
+  - intros.
+    inv H.
+    + inv H0.
+      * split; intros.
+        -- inv H; auto.
+        -- unfold not; intros.
+           inv H1.
+           congruence.
+      * inv H.
+        split; intros; congruence.
+    + inv H1.
+
+  - intros.
+    inv H.
+    inv H1.
+    inv H0.
+    + split; intros; congruence.
+    + inv H.
+      split; intros.
+      * inv H.
+        assert (gamma0 = gamma) by admit.
+        subst.
+        eapply IHtr in H1; eauto.
+        destruct H1.
+        destruct H; auto.
+      * unfold not; intros.
+        inv H3.
+        congruence.
+
+  - intros.
+    inv H.
+    inv H0.
+    + split; intros; congruence.
+    + split; intros; congruence.
+
+  - intros.
+    inv H.
+    inv H0.
+    + split; intros; congruence.
+    + split; intros.
+      * inv H0.
+        eapply IHtr with (word := prefix) in H; eauto.
+        destruct H as [Hsymeq Hsymneq].
+        eapply IHtr0 with (word := suffix) in H1; eauto.
+        destruct H1 as [Htleq Htlneq].
+        destruct (list_eq_dec string_dec prefix prefix0).
+        -- subst.
+           apply suffixes_eq in H2.
+           subst.
+           destruct Hsymeq; destruct Htleq; auto.
+        -- destruct (list_eq_dec string_dec suffix suffix0).
+           ++ subst.
+              apply prefixes_eq in H2.
+              subst.
+              destruct Hsymeq; destruct Htleq; auto.
+           ++ 
+Abort.
+
+
+
+
+
+
+
+
+    
+
+
+
+Lemma what_sym_andor_words_tells_us :
+  forall tbl g,
+    isParseTableFor tbl g
+    -> forall tr tr' sym sym' word word',
+      (@derivesSym g) sym word tr
+      -> (@derivesSym g) sym' word' tr'
+      -> (sym = sym'
+          -> word = word'
+          -> tr = tr')
+         /\ ((sym <> sym'
+              \/ word <> word')
+             -> tr <> tr').
+Proof.
+  intros tbl g Htbl.
+  pose proof Htbl as Htbl'.
+  destruct Htbl as [Hmin Hcom].
+  induction tr using tree_mutual_ind with
+      (P0 := fun f =>
+               forall f' gamma gamma' word word',
+                 (@derivesGamma g) gamma word f
+                 -> (@derivesGamma g) gamma' word' f'
+                 -> (gamma = gamma'
+                     -> word = word'
+                     -> f = f')
+                    /\ ((gamma <> gamma'
+                         \/ word <> word')
+                        -> f <> f')).
+  
+  - intros.
+    inv H.
+    + inv H0.
+      * split; intros.
+        -- inv H; auto.
+        -- unfold not; intros.
+           inv H0.
+           destruct H; congruence.
+      * inv H.
+        split; intros; congruence.
+    + inv H1.
+
+  - intros.
+    inv H.
+    inv H1.
+    inv H0.
+    + split; intros; congruence.
+    + inv H.
+      split; intros.
+      * inv H.
+        assert (gamma0 = gamma) by admit.
+        subst.
+        eapply IHtr with (word := word') in H1; eauto.
+        destruct H1.
+        destruct H; auto.
+      * unfold not; intros.
+        inv H2.
+        destruct H.
+        -- congruence.
+        -- eapply IHtr with (word := word) in H1; eauto.
+           destruct H1.
+           assert (f0 <> f0) by auto.
+           congruence.
+           
+  - intros.
+    inv H.
+    inv H0.
+    + split; intros.
+      * auto.
+      * destruct H; congruence.
+    + split; intros; congruence.
+
+  - intros.
+    inv H.
+    inv H0.
+    + split; intros; congruence.
+    + split; intros.
+      * inv H0.
+        eapply IHtr with (word := prefix) in H; eauto.
+        destruct H as [Hsymeq Hsymneq].
+        eapply IHtr0 with (word := suffix) in H1; eauto.
+        destruct H1 as [Htleq Htlneq].
+        destruct (list_eq_dec string_dec prefix prefix0).
+        -- subst.
+           apply suffixes_eq in H2.
+           subst.
+           destruct Hsymeq; destruct Htleq; auto.
+        -- destruct (list_eq_dec string_dec suffix suffix0).
+           ++ subst.
+              apply prefixes_eq in H2.
+              congruence.
+           ++ admit.
+      * Abort.
+
+                       
+
+    
+
+
+
+
+
+
+
+
+
+
+  
+
+Lemma what_trees_tell_us :
+  forall tbl g,
+    isParseTableFor tbl g
+    -> forall tr tr' sym sym' word word',
+      (@derivesSym g) sym word tr
+      -> (@derivesSym g) sym' word' tr'
+      -> (tr = tr' -> sym = sym' /\ word = word')
+         /\ (tr <> tr' -> sym <> sym'
+                          \/ word <> word').
+Proof.
+  intros tbl g Htbl.
+  pose proof Htbl as Htbl'.
+  destruct Htbl as [Hmin Hcom].
+  induction tr using tree_mutual_ind with
+      (P0 := fun f =>
+               forall f' gamma gamma' word word',
+                 (@derivesGamma g) gamma word f
+                 -> (@derivesGamma g) gamma' word' f'
+                 -> (f = f'
+                     -> gamma = gamma' /\ word = word')
+                    /\ (f <> f' 
+                        -> gamma <> gamma' \/ word <> word')).
+  - intros.
+    inv H.
+    + inv H0.
+      * split; intros.
+        -- inv H.
+           split; auto.
+        -- left.
+           unfold not; intros.
+           congruence.
+      * inv H.
+        split; intros.
+        -- congruence.
+        -- left; congruence.
+    + inv H1.
+
+  - intros.
+    inv H.
+    inv H1.
+    inv H0.
+    + split; intros.
+      * congruence.
+      * left; congruence.
+    + inv H.
+      split; intros.
+      * inv H.
+        eapply IHtr with (word := word) in H1; eauto.
+        destruct H1.
+        destruct H; auto.
+      * pose proof H1 as H1'.
+        eapply IHtr with (word := word) in H1; eauto.
+        destruct H1.
+        destruct (string_dec s x).
+        -- subst.
+           destruct (forest_eq_dec f f0).
+           ++ subst.
+              destruct H1; auto.
+           ++ apply H2 in n.
+              ** destruct (list_eq_dec string_dec word word').
+                 --- subst.
+                     (* get this from LL(1)? *)
+                     admit.
+                 --- auto.
+        -- left.
+           congruence.
+
+  - intros.
+    inv H.
+    inv H0.
+    + split; intros; auto.
+    + split; intros.
+      * congruence.
+      * left; congruence.
+
+  - intros.
+    inv H.
+    inv H0.
+    + split; intros.
+      * congruence.
+      * left; congruence.
+    + split; intros.
+      * inv H0.
+        eapply IHtr with (word := prefix) in H; eauto.
+        destruct H.
+        destruct H; auto.
+        subst.
+        eapply IHtr0 with (word := suffix) in H1; eauto.
+        destruct H1.
+        destruct H; auto.
+        subst.
+        split; auto.
+      * eapply IHtr with (sym := hdSym)
+                         (word := prefix) in H; eauto.
+        destruct H as [Htreq Htrneq].
+        eapply IHtr0 with (gamma := tlSyms)
+                          (word := suffix) in H1; eauto.
+        destruct H1 as [Hfeq Hfneq].
+        destruct H. destruct (tree_eq_dec tr hdTree); subst.
+        eapply IHtr with (word := prefix) in H; eauto.
+        destruct H.
+        -- destruct (forest_eq_dec f tlTrees); subst.
+           ++ congruence.
+           ++ (* heads eq, tails neq *)
+             eapply IHtr with (word := prefix) in H; eauto.
+             destruct H.
+             destruct H; auto.
+             subst.
+             eapply IHtr0 with (word := suffix) in H1; eauto.
+             destruct H1.
+             apply H1 in n.
+             destruct n.
+             ** left; congruence.
+             ** right.
+                unfold not; intros.
+                apply suffixes_eq in H4.
+                congruence.
+        -- destruct (forest_eq_dec f tlTrees); subst.
+           ++ apply IHtr0 in 
+             congruence.
+        -- destruct (forest_eq_dec f tlTrees); subst.
+           ++ (* heads neq, tails eq *)
+             eapply IHtr with (word := prefix) in H; eauto.
+             destruct H.
+             apply H2 in n; auto.
+             eapply IHtr0 with (word := suffix) in H1; eauto.
+             destruct H1.
+             destruct H1; auto.
+             subst.
+             congruence.
+
+          pose proof H as H'.
+           eapply IHtr with (word := prefix) in H; eauto.
+           destruct H.
+           apply H2 in n.
+           destruct n.
+           ++ congruence.
+           ++ eapply IHtr0 with (word := suffix) in H1; eauto.
+              destruct H1.
+              destruct (forest_eq_dec f tlTrees).
+              ** subst.
+                 destruct H1; auto.
+                 subst.
+                 
+
+             
+             
+             eapply IHtr with (word := prefix) in H; eauto.
+             destruct H.
+             destruct H; auto.
+             subst.
+             eapply IHtr0 with (word := suffix) in H1; eauto.
+             destruct H1.
+             apply H1 in n.
+             destruct n.
+             ** left.
+                congruence.
+             **  
+               
+
+
+        apply forest_neq in H0.
+        destruct H0.
+        -- pose proof H as H'.
+           eapply IHtr with (word := prefix) in H; eauto.
+           destruct H.
+           apply H2 in H0.
+           destruct H0.
+           ++ left; congruence.
+           ++ pose proof H1 as H1'.
+              eapply IHtr0 with (word := suffix) in H1; eauto.
+              destruct H1.
+              destruct (forest_eq_dec f tlTrees).
+              ** subst.
+                 destruct H1; auto.
+                 subst.
+
+
+
+
+
+
+    
+        
+Lemma if_trees_eq_then_syms_and_words_eq :
+  forall tbl g,
+    isParseTableFor tbl g
+    -> forall tr tr' sym word word',
+      (@derivesSym g) sym word tr
+      -> (@derivesSym g) sym word' tr'
+      -> (word = word' -> tr = tr')
+         /\ (word <> word' -> tr <> tr').
+Proof.
+  intros tbl g Htbl.
+  pose proof Htbl as Htbl'.
+  destruct Htbl as [Hmin Hcom].
+  induction tr using tree_mutual_ind with
+      (P0 := fun f =>
+               forall f' x gPre gSuf word word',
+                 In (x, gPre ++ gSuf) (productions g)
+                 -> (@derivesGamma g) gSuf word f
+                 -> (@derivesGamma g) gSuf word' f'
+                 -> (word = word' -> f = f')
+                    /\ (word <> word' -> f <> f')).
+
+  - intros.
+    inv H.
+    + inv H0.
+      split; intros; auto.
+    + inv H1.
+
+  - intros.
+    inv H; inv H0.
+    inv H1; inv H2.
+    split; intros.
+    + subst.
+      assert (gamma0 = gamma) by admit.
+      subst.
+      assert (gamma = [] ++ gamma) by auto.
+      rewrite H1 in H.
+      eapply IHtr in H0; eauto.
+      destruct H0.
+      rewrite H0; auto.
+    + unfold not; intros.
+      inv H2. (* on the right track, but we don't know that
+                 gamma and gamma0 are equal *)
+Abort.
+
+
+Lemma if_trees_eq_then_syms_and_words_eq :
+  forall g tr tr' sym sym' word word',
+      (@derivesSym g) sym word tr
+      -> (@derivesSym g) sym' word' tr'
+      -> (tr = tr' -> sym = sym' /\ word = word')
+         /\ (tr <> tr' -> sym <> sym'
+                          \/ word <> word'
+                          \/ exists x gamma1 gamma2
+                                    word3
+                                    f1 f2,
+                              In (x, gamma1) (productions g)
+                              /\ In (x, gamma2) (productions g)
+                              /\ (@derivesGamma g) gamma1 word3 f1
+                              /\ (@derivesGamma g) gamma2 word3 f2
+                              /\ gamma1 <> gamma2).
+Proof.
+  intro g.
+  induction tr using tree_mutual_ind with
+      (P0 := fun f =>
+               forall f' x pre gamma gamma' word word',
+                 In (x, pre ++ gamma) (productions g)
+                 -> In (x, pre ++ gamma') (productions g)
+                 -> (@derivesGamma g) gamma word f
+                 -> (@derivesGamma g) gamma' word' f'
+                 ->  (f = f' -> gamma = gamma' /\ word = word')
+                     /\ (f <> f' -> gamma <> gamma'
+                                    \/ word <> word'
+                                    \/ exists x2 gamma1 gamma2
+                                              word3
+                                              f1 f2,
+                                        In (x2, gamma1) (productions g)
+                                        /\ In (x2, gamma2) (productions g)
+                                        /\ (@derivesGamma g) gamma1 word3 f1
+                                        /\ (@derivesGamma g) gamma2 word3 f2
+                                        /\ gamma1 <> gamma2)).
+                                        
+
+  - intros.
+    inv H; inv H0.
+    + split; intros.
+      * inv H.
+        split; auto.
+      * left; unfold not; intros; congruence.
+    + inv H.
+      split; intros.
+      * congruence.
+      * left; unfold not; intros; congruence.
+    + inv H1.
+    + inv H1.
+
+  - intros.
+    inv H; inv H0.
+    + inv H1.
+      split; intros.
+      * congruence.
+      * left; congruence.
+    + inv H1; inv H.
+      split; intros.
+      * inv H.
+        eapply IHtr with
+            (pre := nil)
+            (gamma := gamma)
+            (gamma' := gamma0) in H0; eauto.
+        destruct H0.
+        destruct H; auto.
+      * 
+
+    + auto.
+  - intros.
+    inv H1; inv H2.
+    split; auto.
+    
+  - intros.
+    inv H1; inv H2.
+    eapply IHtr with
+        (sym := hdSym) (word := prefix) in H6; auto.
+    destruct H6; subst.
+    eapply IHtr0 with
+        (gamma := tlSyms) (word := suffix) in H9; auto.
+    + destruct H9.
+      subst; split; auto.
+    + assert (hdSym0 :: tlSyms = [hdSym0] ++ tlSyms) by auto.
+      rewrite H1 in H.
+      rewrite app_assoc in H.
+      eauto.
+    + assert (hdSym0 :: tlSyms0 = [hdSym0] ++ tlSyms0) by auto.
+      rewrite H1 in H0.
+      rewrite app_assoc in H0.
+      auto.
+Qed.      
+
+Lemma ambig_exists :
+  forall tr tr' g sym word,
+    (@derivesSym g) sym word tr
+    -> (@derivesSym g) sym word tr'
+    -> tr <> tr'
+    -> exists x gamma gamma' word' f f',
+        In (x, gamma) (productions g)
+        /\ In (x, gamma') (productions g)
+        /\ (@derivesGamma g) gamma word' f
+        /\ (@derivesGamma g) gamma' word' f'
+        /\ gamma <> gamma'.
+Proof.
+  induction tr using tree_mutual_ind with
+      (P0 := fun fSuf =>
+               forall fSuf' g x gPre gSuf gSuf' word,
+                 In (x, gPre ++ gSuf) (productions g)
+                 -> In (x, gPre ++ gSuf') (productions g)
+                 -> (@derivesGamma g) gSuf word fSuf
+                 -> (@derivesGamma g) gSuf' word fSuf'
+                 -> fSuf <> fSuf'
+                 -> gSuf <> gSuf'
+                    \/ (exists x2 gamma gamma' word' f f',
+                           In (x2, gamma) (productions g)
+                           /\ In (x2, gamma') (productions g)
+                           /\ (@derivesGamma g) gamma word' f
+                           /\ (@derivesGamma g) gamma' word' f'
+                           /\ gamma <> gamma')).
+  
+  - intros.
+    inv H; inv H0.
+    + congruence.
+    + inv H2.
+
+  - intros.
+    inv H; inv H0.
+    inv H2; inv H3.
+    pose proof H0 as H0'.
+    eapply IHtr with (gPre := nil)
+                     (gSuf := gamma)
+                     (gSuf' := gamma0) in H0; eauto.
+    + destruct H0.
+      * exists s; exists gamma; exists gamma0.
+        repeat eexists; eauto.
+      * eauto.
+    + unfold not; intros; congruence.
+
+  - intros.
+    inv H1; inv H2.
+    + congruence.
+    + left; congruence.
+
+  - intros.
+    inv H1; inv H2.
+    + left; congruence.
+    + 
+
+    
+    
+      
+
+
+
+
+
+
+      
+    
+
+Lemma ambig_exists :
+  forall tbl g,
+    isParseTableFor tbl g
+    -> forall gamma word x tr tr',
+    (@derivesProd g) x gamma word tr
+    -> (@derivesProd g) x gamma word tr'
+    -> tr <> tr'
+    -> exists x2 gamma' gamma'' w1 w2 w3 st st',
+        In (NT x2) gamma
+        /\ In (x2, gamma') (productions g)
+        /\ In (x2, gamma'') (productions g)
+        /\ word = w1 ++ w2 ++ w3
+        /\ (@derivesProd g) x2 gamma' w2 st
+        /\ (@derivesProd g) x2 gamma'' w2 st'
+        /\ gamma' <> gamma'.
+Proof.
+  intros tbl g Htbl.
+  induction gamma as [| sym syms].
+  - intros.
+    inv H.
+    inv H0.
+    admit.
+  - intros.
+    inv H; inv H0.
+    inv H3; inv H4.
+    inv H6; inv H7.
+    + inv H5.
+    
+  inv H0; inv H1.
+
+Ab
+
+Lemma lemma4 :
+  forall tbl g,
+    isParseTableFor tbl g
+    -> forall x x2 pre suf w1 w2 w3 gamma gamma' tr tr' f1 f3,
+      In (x, pre ++ (NT x2) :: suf) (productions g)
+      -> (@derivesGamma g) pre w1 f1
+      -> (@derivesProd g) x2 gamma w2 tr
+      -> (@derivesProd g) x2 gamma' w2 tr'
+      -> (@derivesGamma g) suf w3 f3
+      -> gamma = gamma' /\ tr = tr'.
+Proof.
+  intros.
+  inv H2; inv H3.
+  
+Lemma derives_det :
+  forall tbl g,
+    isParseTableFor tbl g
+    -> forall tr tr'
+              x pre sym suf
+              wPre wPre'
+              word word'
+              wSuf wSuf'
+              f f',
+      In (x, pre ++ sym :: suf) (productions g)
+      -> (@derivesSym g) sym wPre tr
+      -> (@derivesSym g) sym wPre' tr'
+      -> (@derivesGamma g) suf word f
+      -> (@derivesGamma g) suf word' f'
+      -> wPre ++ word = wPre' ++ word'
+      -> word ++ wSuf = word' ++ wSuf'
+      -> wPre = wPre'
+         /\ word = word'
+         /\ wSuf = wSuf'
+         /\ tr = tr'.
+Proof.
+  intros tbl g Htbl.
+  pose proof Htbl as Htbl'.
+  destruct Htbl as [Hmin Hcom].
+  induction tr using tree_mutual_ind with
+      (P0 := fun f =>
+               forall f' x pre gamma wPre wPre' wSuf wSuf',
+                 In (x, pre ++ gamma) (productions g)
+                 -> (@derivesGamma g) gamma wPre f
+                 -> (@derivesGamma g) gamma wPre' f'
+                 -> wPre ++ wSuf = wPre' ++ wSuf'
+                 -> wPre = wPre' /\ wSuf = wSuf' /\ f = f').
+  
+  - intros.
+    inv H0; inv H1; auto.
+    + inv H4.
+      apply suffixes_eq in H5.
+      subst.
+      repeat (split; auto).
+    + inv H6.
+
+  - intros.
+    inv H0; inv H1.
+    inv H6; inv H7.
+    assert (gamma0 = gamma) by admit. (* get this from LL(1) *)
+    subst.
+    eapply IHtr in H1; eauto.
+    + destruct H1.
+      destruct H6.
+      subst.
+      apply suffixes_eq in H5.
+      subst.
+      repeat (split; auto).
+    + assert (gamma = [] ++ gamma) by auto.
+      rewrite H6 in H0.
+      eauto.
+
+  - intros.
+    inv H0; inv H1.
+    simpl in *.
+    subst.
+    repeat (split; auto).
+
+  - intros.
+    inv H0.
+    inv H1.
+    eapply IHtr with
+        (wPre := prefix)
+        (wPre' := prefix0)
+        (word := suffix)
+        (word' := suffix0)
+        (wSuf := wSuf)
+        (wSuf' := wSuf') in H4; eauto.
+    + destruct H4.
+      destruct H1.
+      destruct H9.
+      destruct H3.
+      subst.
+      inv H8.
+      * repeat (split; auto).
+      * 
+    + destruct H
+    eapply IHtr0 with
+        (wPre := wPre ++ prefix)
+        (wPre' := wPre' ++ prefix0) in H9; eauto.
+    + destruct H9.
+      destruct H1.
+      subst.
+      eapply IHtr in H4; eauto.
+      * destruct H4.
+        destruct H3.
+        destruct H4.
+        subst.
+        repeat (split; auto).
+      * 
+      
+    destruct hdSym as [y | x2].
+    + inv H6; inv H4.
+      inv H3.
+      assert (T y :: tlSyms = [T y] ++ tlSyms) by auto.
+      rewrite H0 in H.
+      rewrite app_assoc in H.
+      erewrite IHtr0; eauto.
+    + (* here, we're going to get stuck because we don't know
+         whether prefix = prefix0. It would help if we knew
+         that prefix and prefix0 shared the first lookahead
+         token *)
+Abort.
+
+
+(* Here's what we really want to prove *)
+Lemma derives_det :
+  forall tbl g,
+    isParseTableFor tbl g
+    -> forall tr tr' sym word,
+      (@derivesSym g) sym word tr
+      -> (@derivesSym g) sym word tr'
+      -> tr = tr'.
+Proof.
+  intros tbl g Htbl.
+  pose proof Htbl as Htbl'.
+  destruct Htbl as [Hmin Hcom].
+  induction tr using tree_mutual_ind with
+      (P0 := fun f =>
+               forall f' x pre gamma word,
+                 In (x, pre ++ gamma) (productions g)
+                 -> (@derivesGamma g) gamma word f
+                 -> (@derivesGamma g) gamma word f'
+                 ->  f = f').
+  
+  - intros.
+    inv H; inv H0; auto.
+    inv H1.
+
+  - intros.
+    inv H; inv H0.
+    inv H1; inv H2.
+    assert (gamma0 = gamma) by admit. (* get this from LL(1) *)
+    subst.
+    assert (gamma = [] ++ gamma) by auto.
+    rewrite H1 in H.
+    erewrite IHtr; eauto.
+
+  - intros.
+    inv H0; inv H1.
+    auto.
+
+  - intros.
+    inv H0.
+    inv H1.
+    destruct hdSym as [y | x2].
+    + inv H6; inv H4.
+      inv H3.
+      assert (T y :: tlSyms = [T y] ++ tlSyms) by auto.
+      rewrite H0 in H.
+      rewrite app_assoc in H.
+      erewrite IHtr0; eauto.
+    + (* here, we're going to get stuck because we don't know
+         whether prefix = prefix0. It would help if we knew
+         that prefix and prefix0 shared the first lookahead
+         token *)
+Abort.
+
+Lemma derives_det :
+  forall tbl g,
+    isParseTableFor tbl g
+    -> forall tr tr' x
+              pre sym suf
+              word word'
+              wSuf wSuf'
+              f f',
+      In (x, pre ++ sym :: suf) (productions g)
+      -> (@derivesSym g) sym word tr
+      -> (@derivesSym g) sym word' tr'
+      -> (@derivesGamma g) suf wSuf f
+      -> (@derivesGamma g) suf wSuf' f'
+      -> word ++ wSuf = word' ++ wSuf'
+      -> word = word'
+         /\ wSuf = wSuf'
+         /\ tr = tr'.
+Proof.
+  intros tbl g Htbl.
+  pose proof Htbl as Htbl'.
+  destruct Htbl as [Hmin Hcom].
+  induction tr using tree_mutual_ind with
+      (P0 := fun f =>
+               forall f' x pre gamma wPre wPre' wSuf wSuf',
+                 In (x, pre ++ gamma) (productions g)
+                 -> (@derivesGamma g) gamma wSuf f
+                 -> (@derivesGamma g) gamma wSuf' f'
+                 -> wPre ++ wSuf = wPre' ++ wSuf'
+                 ->  wPre = wPre'
+                     /\ wSuf = wSuf'
+                     /\ f = f').
+  - intros.
+    inv H0; inv H1; auto.
+    + inv H4.
+      subst.
+      repeat (split; auto).
+    + inv H5.
+
+  - intros.
+    inv H0; inv H1.
+    inv H5; inv H6.
+    assert (gamma0 = gamma) by admit; subst.
+    eapply IHtr in H1; eauto.
+    + destruct H1.
+      destruct H5.
+      subst.
+      apply suffixes_eq in H4.
+      subst.
+      repeat (split; auto).
+    + admit.
+    + 
+      
+  - intros.
+    inv H0; inv H1.
+    repeat rewrite app_nil_r in *.
+    subst.
+    repeat (split; auto).
+
+  - intros.
+    inv H0; inv H1.
+    pose proof H9 as H9'.
+    eapply IHtr0 with
+        (wPre := wPre ++ prefix)
+        (wPre' := wPre' ++ prefix0) in H9; eauto.
+    + destruct H9.
+      destruct H1.
+      subst.
+      eapply IHtr in H4; eauto.
+      * destruct H4.
+        destruct H3.
+        destruct H4.
+        subst.
+        repeat (split; auto).
+      * 
+
+Lemma derivesSym_det :
+  forall tbl g,
+    isParseTableFor tbl g
+    -> forall tr tr' x
+              gPre
+              sym word word' 
+              gSuf wSuf wSuf' fSuf fSuf',
+      
+      In (x, gPre ++ sym :: gSuf) (productions g)
+                           
+      -> (@derivesSym g) sym word tr
+      -> (@derivesSym g) sym word' tr'
+                         
+      -> (@derivesGamma g) gSuf wSuf fSuf
+      -> (@derivesGamma g) gSuf wSuf' fSuf'
+                           
+      -> word ++ wSuf = word' ++ wSuf'
+                                      
+      ->  word = word'
+          /\ wSuf = wSuf'
+          /\ tr = tr'.
+Proof.
+  intros tbl g Htbl.
+  pose proof Htbl as Htbl'.
+  destruct Htbl as [Hmin Hcom].
+  induction tr using tree_mutual_ind with
+      (P0 := fun fPre =>
+               forall x
+                      gPre wPre wPre' fPre'
+                      gSuf wSuf wSuf' fSuf fSuf',
+                 
+                 In (x, gPre ++ gSuf) (productions g)
+                    
+                 -> (@derivesGamma g) gPre wPre fPre
+                 -> (@derivesGamma g) gPre wPre' fPre'
+                                      
+                 -> (@derivesGamma g) gSuf wSuf fSuf
+                 -> (@derivesGamma g) gSuf wSuf' fSuf'
+
+                 -> wPre ++ wSuf = wPre' ++ wSuf'
+                                      
+                 -> wPre = wPre'
+                    /\ wSuf = wSuf'
+                    /\ fSuf = fSuf').
+  - intros.
+    inv H0; inv H1.
+    + inv H4.
+      repeat (split; auto).
+    + inv H5.
+      
+  - intros.
+    inv H0; inv H1.
+    inv H5; inv H6.
+    assert (gamma0 = gamma) by admit.
+    subst.
+    eapply IHtr with (wSuf := nil)
+                     (wSuf' := nil) in H1; eauto.
+    + destruct H3.
+      destruct H7.
+      subst.
+      split; auto.
+    + econstructor.
+    + econstructor.
+    + simpl.
+    + destruct H1.
+      subst.
+      apply suffixes_eq in H4.
+      subst.
+      repeat (split; auto).
+    + admit.
+    
+  - intros.
+    inv H0; inv H1.
+    repeat (split; auto).
+
+  - intros.
+    inv H0; inv H1.
+    pose proof H8 as H8'.
+    eapply IHtr0 in H8; eauto.
+    + destruct H8.
+      subst.
+    
+    eapply IHtr0 with
+        (wPre := wPre ++ prefix)
+        (wPre' := wPre' ++ prefix0) in H8; eauto.
+    + destruct H8.
+      destruct H0.
+      subst.
+      
+
+(* Input is empty, symbol could be T or NT *)
+Lemma derives_nil_det :
+  forall tbl g,
+    isParseTableFor tbl g
+    -> forall tr tr' sym,
+      (@derivesSym g) sym [] tr
+      -> (@derivesSym g) sym [] tr'
+      -> tr = tr'.
+Proof.
+  intros tbl g Htbl.
+  pose proof Htbl as Htbl'.
+  destruct Htbl as [Hmin Hcom].
+  induction tr using tree_mutual_ind with
+      (P0 := fun f =>
+               forall f' x pre gamma,
+                 In (x, pre ++ gamma) (productions g)
+                 -> (@derivesGamma g) gamma [] f
+                 -> (@derivesGamma g) gamma [] f'
+                 -> f = f').
+  - intros.
+    inv H.
+    inv H1.
+
+  - intros.
+    inv H.
+    inv H1.
+    inv H0.
+    inv H1.
+    assert (gamma0 = gamma) by admit.
+    subst.
+    assert (gamma = [] ++ gamma) by auto.
+    rewrite H1 in H.
+    erewrite IHtr; eauto.
+
+  - intros.
+    inv H0.
+    inv H1.
+    auto.
+
+  - intros.
+    inv H0.
+    inv H1.
+    assert (prefix = []) by admit.
+    assert (prefix0 = []) by admit.
+    assert (suffix = []) by admit.
+    assert (suffix0 = []) by admit.
+    subst.
+    assert (hdSym :: tlSyms = [hdSym] ++ tlSyms) by auto.
+    rewrite H0 in H.
+    rewrite app_assoc in H.
+    erewrite IHtr; eauto.
+    erewrite IHtr0; eauto.
+Admitted.
+
+Lemma derivesGamma_nil_det :
+  forall tbl g,
+    isParseTableFor tbl g
+    -> forall f f' x pre gamma,
       In (x, pre ++ gamma) (productions g)
-      -> (@derivesGamma g) gamma word f
-      -> (@derivesGamma g) gamma word f'
+      -> (@derivesGamma g) gamma [] f
+      -> (@derivesGamma g) gamma [] f'
       -> f = f'.
 Proof.
   intros tbl g Htbl.
@@ -423,60 +3736,2094 @@ Proof.
   destruct Htbl as [Hmin Hcom].
   induction f using forest_mutual_ind with
       (P := fun tr =>
-              forall tr' sym word,
-                (@derivesSym g) sym word tr
-                -> (@derivesSym g) sym word tr'
+              forall tr' sym,
+                (@derivesSym g) sym [] tr
+                -> (@derivesSym g) sym [] tr'
                 -> tr = tr').
-  - intros tr' sym word Hder Hder'.
-    inv Hder.
-    + inv Hder'.
-      auto.
-    + inv H.
 
-  - intros tr' sym word Hder Hder'.
+  - intros.
+    inv H.
+    inv H1.
+
+  - intros.
+    inv H.
+    inv H1.
+    inv H0.
+    inv H1.
+    assert (gamma0 = gamma) by admit.
+    subst.
+    assert (gamma = [] ++ gamma) by auto.
+    rewrite H1 in H.
+    erewrite IHf; eauto.
+
+  - intros.
+    inv H0.
+    inv H1.
+    auto.
+
+  - intros.
+    inv H0.
+    inv H1.
+    assert (prefix = []) by admit.
+    assert (prefix0 = []) by admit.
+    assert (suffix = []) by admit.
+    assert (suffix0 = []) by admit.
+    subst.
+    assert (hdSym :: tlSyms = [hdSym] ++ tlSyms) by auto.
+    rewrite H0 in H.
+    rewrite app_assoc in H.
+    erewrite IHf; eauto.
+    erewrite IHf0; eauto.
+Admitted.
+
+Lemma derives_cons_T_det :
+  forall tbl g,
+    isParseTableFor tbl g
+    -> forall tr tr' y word word',
+      (@derivesSym g) (T y) word tr
+      -> (@derivesSym g) (T y) word' tr'
+      -> tr = tr' /\ word = word'.
+Proof.
+  intros tbl g Htbl.
+  pose proof Htbl as Htbl'.
+  destruct Htbl as [Hmin Hcom].
+  induction tr; intros.
+  - inv H.
+    inv H0.
+    split; auto.
+  - inv H.
+Qed.
+
+
+Lemma prefixes_eq :
+  forall (suf pre pre' : list string),
+    app pre suf = app pre' suf
+    -> pre = pre'.
+Proof.
+  induction suf; intros; simpl in *.
+  - repeat rewrite app_nil_r in H.
+    auto.
+  - assert (a :: suf = app [a] suf) by auto.
+    repeat rewrite H0 in H.
+    repeat rewrite app_assoc in H.
+    apply IHsuf in H.
+    apply app_inj_tail in H.
+    destruct H.
+    auto.
+Qed.
+
+Lemma suffixes_eq :
+  forall (pre suf suf' : list string),
+    app pre suf = app pre suf'
+    -> suf = suf'.
+Proof.
+  induction pre; intros; simpl in *.
+  - auto.
+  - inv H.
+    apply IHpre; auto.
+Qed.
+
+Lemma derives_det :
+  forall tbl g,
+    isParseTableFor tbl g
+    -> forall tr tr' sym word,
+      (@derivesSym g) sym word tr
+      -> (@derivesSym g) sym word tr'
+      -> tr = tr'.
+Proof.
+  intros tbl g Htbl.
+  pose proof Htbl as Htbl'.
+  destruct Htbl as [Hmin Hcom].
+  induction tr using tree_mutual_ind with
+      (P0 := fun f =>
+               forall f' gamma word,
+                 (@derivesGamma g) gamma word f
+                 -> (@derivesGamma g) gamma word f'
+                 ->  f = f').
+  - intros.
+    inv H; inv H0; auto.
+    inv H1.
+  - intros.
+    inv H; inv H0.
+    inv H1; inv H2.
+    assert (gamma0 = gamma) by admit.
+    subst.
+    erewrite IHtr; eauto.
+
+  - intros.
+    inv H; inv H0; auto.
+
+  - intros.
+    inv H; inv H0.
+
+(* Here's what we really want to prove *)
+Lemma derives_det :
+  forall tbl g,
+    isParseTableFor tbl g
+    -> forall tr tr' sym word,
+      (@derivesSym g) sym word tr
+      -> (@derivesSym g) sym word tr'
+      -> tr = tr'.
+Proof.
+  intros tbl g Htbl.
+  pose proof Htbl as Htbl'.
+  destruct Htbl as [Hmin Hcom].
+  induction tr using tree_mutual_ind with
+      (P0 := fun f =>
+               forall f' x pre gamma word,
+                 In (x, pre ++ gamma) (productions g)
+                 -> (@derivesGamma g) gamma word f
+                 -> (@derivesGamma g) gamma word f'
+                 ->  f = f').
+  - intros.
+    inv H; inv H0; auto.
+    inv H1.
+
+  - intros.
+    inv H; inv H0.
+    inv H1; inv H2.
+    assert (gamma0 = gamma) by admit. (* get this from LL(1) *)
+    subst.
+    assert (gamma = [] ++ gamma) by auto.
+    rewrite H1 in H.
+    erewrite IHtr; eauto.
+
+  - intros.
+    inv H0; inv H1.
+    auto.
+
+  - intros.
+    inv H0; inv H1.
+    destruct hdSym as [y | x2].
+    + inv H6; inv H4.
+      inv H3.
+      assert (T y :: tlSyms = [T y] ++ tlSyms) by auto.
+      rewrite H0 in H.
+      rewrite app_assoc in H.
+      erewrite IHtr0; eauto.
+    + (* here, we're going to get stuck because we don't know
+         whether prefix = prefix0. It would help if we knew
+         that prefix and prefix0 shared the first lookahead
+         token *)
+Abort.
+
+(* This gets us almost all the way there, but proving that
+   gamma = gamma0 is the problem. We need to change the
+   derivesSym hypothesis so that it talks about a symbol
+   in the middle of some right-hand side *)
+Lemma derives_det' :
+  forall tbl g,
+    isParseTableFor tbl g
+    -> forall tr tr' sym pre pre' suf suf',
+      (@derivesSym g) sym pre tr
+      -> (@derivesSym g) sym pre' tr'
+      -> pre ++ suf = pre' ++ suf'
+      -> pre = pre' /\ suf = suf' /\ tr = tr'.
+Proof.
+  intros tbl g Htbl.
+  pose proof Htbl as Htbl'.
+  destruct Htbl as [Hmin Hcom].
+  induction tr using tree_mutual_ind with
+      (P0 := fun f =>
+               forall f' x gPre gamma pre pre' suf suf',
+                 In (x, gPre ++ gamma) (productions g)
+                 -> (@derivesGamma g) gamma pre f
+                 -> (@derivesGamma g) gamma pre' f'
+                 -> pre ++ suf = pre' ++ suf'
+                 -> pre = pre' /\ suf = suf' /\ f = f').
+  
+  - intros.
+    inv H; inv H0.
+    + inv H1.
+      repeat (split; auto).
+    + inv H2.
+
+  - intros.
+    inv H; inv H0.
+    inv H2; inv H3.
+    rename s into x.
+    (*
+    assert (gamma0 = gamma).
+    { destruct pre as [| ptok ptoks]; simpl in *.
+      - destruct pre' as [| ptok' ptoks']; simpl in *.
+        + apply derivesGamma_nil_nullable in H0.
+          apply derivesGamma_nil_nullable in H8.
+          assert ((@isLookaheadFor g) EOF (NT x) gamma0).
+          { unfold isLookaheadFor.
+            right.
+            split.
+            - constructor; auto.
+            - constructor; auto.
+              econstructor.
+              econstructor; eauto. }
+          assert ((@isLookaheadFor g) EOF (NT x) gamma).
+          { unfold isLookaheadFor.
+            right.
+            split.
+            - constructor; auto.
+            - constructor; auto.
+              econstructor.
+              econstructor; eauto. }
+          apply Hcom in H2; apply Hcom in H3.
+          destruct H2 as [laMap [Hsf Hlf]].
+          destruct H3 as [laMap' [Hsf' Hlf']].
+          congruence.
+        + admit.
+      *)      
+
+    assert (gamma0 = gamma) by admit.
+    subst.
+    assert (gamma = [] ++ gamma) by auto.
+    rewrite H2 in H.
+    eapply IHtr in H0; eauto.
+    destruct H0.
+    destruct H3.
+    subst; repeat (split; auto).
+          
+  - intros.
+    inv H0; inv H1; auto.
+
+  - intros.
+    destruct gamma as [| sym syms].
+    + inv H0.
+    + destruct f' as [| tr' f'].
+      * inv H1.
+      * inv H0; inv H1.
+        repeat rewrite <- app_assoc in H2.
+        assert (sym :: syms = [sym] ++ syms) by auto.
+        rewrite H0 in H.
+        rewrite app_assoc in H.
+        eapply IHtr with (pre := prefix) in H6; eauto.
+        destruct H6.
+        destruct H3.
+        subst.
+        eapply IHtr0 with (pre := suffix) in H10; eauto.
+        destruct H10.
+        destruct H4.
+        subst.
+        repeat (split; auto).
+Admitted.
+
+  
+    
+(*    
+(* maybe get rid of the rem stuff *)
+Lemma derivesGamma_det' :
+  forall tbl g,
+    isParseTableFor tbl g
+    -> forall f f' x gPre gSuf word word' rem rem',
+      In (x, gPre ++ gSuf) (productions g)
+      -> (@derivesGamma g) gSuf word f
+      -> (@derivesGamma g) gSuf word' f'
+      -> word ++ rem = word' ++ rem'
+      -> word = word' /\ f = f'.
+Proof.
+  intros tbl g Htbl.
+  pose proof Htbl as Htbl'.
+  destruct Htbl as [Hmin Hcom].
+  induction f using forest_mutual_ind with
+      (P := fun tr =>
+              forall tr' x sym
+                     gPre gSuf
+                     wPre wPre'
+                     wSuf wSuf'
+                     f f'
+                     rem rem',
+                In (x, gPre ++ sym :: gSuf) (productions g)
+                -> (@derivesSym g) sym wPre tr
+                -> (@derivesSym g) sym wPre' tr'
+                -> (@derivesGamma g) gSuf wSuf f
+                -> (@derivesGamma g) gSuf wSuf' f'
+                -> wPre ++ rem = wPre' ++ rem'
+                -> wPre = wPre' /\ tr = tr').
+
+  - intros.
+    inv H0; inv H1.
+    + inv H4.
+      repeat (split; auto).
+    + inv H5.
+
+  - intros.
+    inv H0; inv H1.
+    inv H5; inv H6.
+    rename s into x2.
+    assert (gamma0 = gamma).
+    { destruct wPre as [| ptok ptoks]; simpl in *.
+      - destruct wPre' as [| ptok' ptoks']; simpl in *.
+        + apply derivesGamma_nil_nullable in H11.
+          apply derivesGamma_nil_nullable in H1.
+          assert ((@isLookaheadFor g) EOF (NT x2) gamma).
+          { unfold isLookaheadFor.
+            right.
+            split.
+            - constructor; auto.
+            - constructor; auto.
+              eapply FoNu.
+              econstructor; eauto. }
+          assert ((@isLookaheadFor g) EOF (NT x2) gamma0).
+          { unfold isLookaheadFor.
+            right.
+            split.
+            - constructor; auto.
+            - constructor; auto.
+              eapply FoNu.
+              econstructor; eauto. }
+          apply Hcom in H5; apply Hcom in H6.
+          destruct H5 as [laMap [Hsf Hlf]].
+          destruct H6 as [laMap' [Hsf' Hlf']].
+          congruence.
+        + destruct wSuf as [| stok stoks]; simpl in *.
+          * apply derivesGamma_nil_nullable in H11.
+            apply derivesGamma_nil_nullable in H2.
+            assert ((@isLookaheadFor g) EOF (NT x2) gamma).
+            { unfold isLookaheadFor.
+              right.
+              split.
+              - constructor; auto.
+              - constructor; auto.
+                eapply FoLeft.
+                econstructor; eauto. }
+          assert ((@isLookaheadFor g) EOF (NT x2) gamma0).
+          { unfold isLookaheadFor.
+            right.
+            split.
+            - constructor; auto.
+            - constructor; auto.
+              eapply FoNu.
+              econstructor; eauto. }destruct 
+          * inv H4.
+            inv H2.
+      - destruct pre' as [| ptok' ptoks']; simpl in *.
+        + inv H2.
+        + inv H1.
+          apply derivesGamma_cons_firstGamma in H0.
+          apply derivesGamma_cons_firstGamma in H9.
+          assert ((@isLookaheadFor g) (LA ptok') (NT x) gamma).
+          { unfold isLookaheadFor.
+            left.
+            constructor; auto. }
+          assert ((@isLookaheadFor g) (LA ptok') (NT x) gamma0).
+          { unfold isLookaheadFor.
+            left.
+            constructor; auto. }
+          apply Hcom in H1; apply Hcom in H3.
+          destruct H1 as [laMap [Hsf Hlf]].
+          destruct H3 as [laMap' [Hsf' Hlf']].
+          congruence. }
+    assert (gamma0 = gamma) by admit.
+    subst.
+    eapply IHf in H1; eauto.
+    + destruct H1.
+      destruct H5.
+      subst.
+      repeat (split; auto).
+    + assert (gamma = [] ++ gamma) by auto.
+      rewrite H5 in H0.
+      eauto.
+
+  - intros.
+    inv H0; inv H1; auto.
+
+  - intros.
+    inv H0; inv H1.
+    eapply IHf with (wSuf := suffix)
+                    (wSuf' := suffix0)
+                    (rem := rem)
+                    (rem' := rem') in H4; eauto. 
+    + destruct H4.
+      subst.
+      eapply IHf0 with (rem := rem)
+                       (rem' := rem') in H9; eauto.
+      * destruct H9.
+        destruct H1.
+        subst.
+        repeat (split; auto).
+      * assert (hdSym :: tlSyms = [hdSym] ++ tlSyms) by auto.
+        rewrite H0 in H.
+        rewrite app_assoc in H.
+        eauto.
+      * repeat rewrite <- app_assoc in H2.
+        apply suffixes_eq in H2.
+        auto.
+    + repeat rewrite <- app_assoc in H2.
+      auto.
+Admitted.
+*)
+
+Lemma derivesGamma_det' :
+  forall tbl g,
+    isParseTableFor tbl g
+    -> forall gSuf x gPre wPre wPre' wSuf wSuf' f f',
+      In (x, gPre ++ gSuf) (productions g)
+      -> (@derivesGamma g) gSuf wPre f
+      -> (@derivesGamma g) gSuf wPre' f'
+      -> wPre ++ wSuf = wPre' ++ wSuf'
+      -> wPre = wPre' /\ wSuf = wSuf' /\ f = f'.
+Proof.
+  intros tbl g Htbl.
+  pose proof Htbl as Htbl'.
+  destruct Htbl as [Hmin Hcom].
+  induction gSuf as [| sym syms].
+  - intros.
+    inv H0; inv H1; simpl in *.
+    subst.
+    repeat (split; auto).
+  - intros.
+    destruct f as [| tr f].
+    + inv H0.
+    + destruct f' as [| tr' f'].
+      * inv H1.
+      * inv H0; inv H1.
+        destruct sym as [y | x2].
+        -- inv H7; inv H6.
+           inv H2.
+           eapply IHsyms with (wPre := suffix)
+                              (wSuf := wSuf)
+                              (wPre' := suffix0)
+                              (wSuf' := wSuf') in H10; eauto.
+           ++ destruct H10.
+              destruct H2.
+              subst.
+              repeat (split; auto).
+           ++ assert (T y :: syms = [T y] ++ syms) by auto.
+              rewrite H0 in H.
+              rewrite app_assoc in H.
+              eauto.
+        -- inv H7.
+           inv H6.
+           inv H1.
+           inv H3.
+           { destruct prefix as [| ptok ptoks]; simpl in *.
+             - destruct prefix0 as [| ptok' ptoks']; simpl in *.
+               + apply derivesGamma_nil_nullable in H4.
+                 apply derivesGamma_nil_nullable in H5.
+                 assert ((@isLookaheadFor g) EOF (NT x2) gamma).
+                 { unfold isLookaheadFor.
+                   right.
+                   split.
+                   - constructor; auto.
+                   - constructor; auto.
+                     eapply FoNu; eauto.
+                     econstructor; eauto. }
+                 assert ((@isLookaheadFor g) EOF (NT x2) gamma0).
+                 { unfold isLookaheadFor.
+                   right.
+                   split.
+                   - constructor; auto.
+                   - constructor; auto.
+                     eapply FoNu; eauto.
+                     econstructor; eauto. }
+                 apply Hcom in H3; apply Hcom in H6.
+                 destruct H3 as [laMap [Hsf Hlf]].
+                 destruct H6 as [laMap' [Hsf' Hlf']].
+Abort.
+                   
+          
+(* Here we're trying the "sym in the middle of an RHS"
+   strategy *)
+Lemma derives_det'' :
+  forall tbl g,
+    isParseTableFor tbl g
+    -> forall tr tr' x gPre sym gSuf
+              pre pre'
+              suf suf'
+              f f',
+      In (x, gPre ++ sym :: gSuf) (productions g)
+      -> (@derivesSym g) sym pre tr
+      -> (@derivesSym g) sym pre' tr'
+      -> (@derivesGamma g) gSuf suf f
+      -> (@derivesGamma g) gSuf suf' f'
+      -> pre ++ suf = pre' ++ suf'
+      -> pre = pre' /\ suf = suf' /\ tr = tr'.
+(* add the fact that f and f' are equal in the conclusion? *)
+Proof.
+  intros tbl g Htbl.
+  pose proof Htbl as Htbl'.
+  destruct Htbl as [Hmin Hcom].
+  induction tr using tree_mutual_ind with
+      (P0 := fun f =>
+               forall f' x gPre gamma gSuf
+                      pre pre'
+                      suf suf'
+                      fSuf fSuf',
+                 In (x, gPre ++ gamma ++ gSuf) (productions g)
+                 -> (@derivesGamma g) gamma pre f
+                 -> (@derivesGamma g) gamma pre' f'
+                 -> (@derivesGamma g) gSuf suf fSuf
+                 -> (@derivesGamma g) gSuf suf' fSuf'
+                 -> pre ++ suf = pre' ++ suf'
+                 -> pre = pre' /\ suf = suf' /\ f = f'
+                    /\ fSuf = fSuf').
+
+  - intros.
+    inv H0; inv H1.
+    + inv H4.
+      repeat (split; auto).
+    + inv H5.
+
+  - intros.
+    inv H0; inv H1.
+    inv H5; inv H6.
+    rename s into x2.
+    assert (gamma0 = gamma).
+    { 
+      destruct pre as [| ptok ptoks]; simpl in *.
+      - destruct pre' as [| ptok' ptoks']; simpl in *.
+        + apply derivesGamma_nil_nullable in H1.
+          apply derivesGamma_nil_nullable in H11.
+          assert ((@isLookaheadFor g) EOF (NT x2) gamma0).
+          { unfold isLookaheadFor.
+            right.
+            split.
+            - constructor; auto.
+            - constructor; auto.
+              econstructor.
+              econstructor; eauto. }
+          assert ((@isLookaheadFor g) EOF (NT x2) gamma).
+          { unfold isLookaheadFor.
+            right.
+            split.
+            - constructor; auto.
+            - constructor; auto.
+              econstructor.
+              econstructor; eauto. }
+          apply Hcom in H5; apply Hcom in H6.
+          destruct H5 as [laMap [Hsf Hlf]].
+          destruct H6 as [laMap' [Hsf' Hlf']].
+          congruence.
+        + subst.
+          assert ((@isLookaheadFor g) (LA ptok')
+                                      (NT x2)
+                                      gamma).
+          { unfold isLookaheadFor.
+            right.
+            split.
+            - constructor; auto.
+              apply derivesGamma_nil_nullable in H11.
+              auto.
+            - constructor; auto.
+              eapply FoRight with
+                  (x1 := x)
+                  (prefix := gPre)
+                  (suffix := gSuf); eauto.
+              apply derivesGamma_cons_firstGamma in H2.
+              auto. }
+          assert ((@isLookaheadFor g) (LA ptok')
+                                      (NT x2)
+                                      gamma0).
+          { unfold isLookaheadFor.
+            left.
+            constructor; auto.
+            apply derivesGamma_cons_firstGamma in H1.
+            auto. }
+          apply Hcom in H4; apply Hcom in H5.
+          destruct H4 as [laMap [Hsf Hlf]].
+          destruct H5 as [laMap' [Hsf' Hlf']].
+          congruence.
+      - destruct pre' as [| ptok' ptoks']; simpl in *.
+        + subst.
+          assert ((@isLookaheadFor g) (LA ptok)
+                                      (NT x2)
+                                      gamma0).
+          { unfold isLookaheadFor.
+            right.
+            split.
+            - constructor; auto.
+              apply derivesGamma_nil_nullable in H1.
+              auto.
+            - constructor; auto.
+              eapply FoRight with
+                  (x1 := x)
+                  (prefix := gPre)
+                  (suffix := gSuf); eauto.
+              apply derivesGamma_cons_firstGamma in H3.
+              auto. }
+          assert ((@isLookaheadFor g) (LA ptok)
+                                      (NT x2)
+                                      gamma).
+          { unfold isLookaheadFor.
+            left.
+            constructor; auto.
+            apply derivesGamma_cons_firstGamma in H11.
+            auto. }
+          apply Hcom in H4; apply Hcom in H5.
+          destruct H4 as [laMap [Hsf Hlf]].
+          destruct H5 as [laMap' [Hsf' Hlf']].
+          congruence.
+        + inv H4.
+          assert ((@isLookaheadFor g) (LA ptok')
+                                      (NT x2)
+                                      gamma).
+          { unfold isLookaheadFor.
+            left.
+            constructor; auto.
+            apply derivesGamma_cons_firstGamma in H11.
+            auto. }
+          assert ((@isLookaheadFor g) (LA ptok')
+                                      (NT x2)
+                                      gamma0).
+          { unfold isLookaheadFor.
+            left.
+            constructor; auto.
+            apply derivesGamma_cons_firstGamma in H1.
+            auto. }
+          apply Hcom in H4; apply Hcom in H5.
+          destruct H4 as [laMap [Hsf Hlf]].
+          destruct H5 as [laMap' [Hsf' Hlf']].
+          congruence. }
+    subst.
+    
+           
+    eapply IHtr with (gamma := [NT x2])
+                     (pre := pre)
+                     (pre' := pre')
+                     (suf := suf)
+                     (suf' := suf')
+                     (f' := f1) in H; eauto.
+    + destruct H.
+      destruct H5.
+      destruct H6.
+      subst.
+      repeat (split; auto).
+    + admit.
+    + admit.
+    
+  - intros.
+    inv H0; inv H1; auto.
+    simpl in *.
+    subst.
+    admit.
+    
+  - intros.
+    destruct gamma as [| sym syms].
+    + inv H0.
+    + destruct f' as [| tr' f'].
+      * inv H1.
+      * inv H0; inv H1.
+        repeat rewrite <- app_assoc in H2.
+        eapply (IHtr tr' x gPre sym syms prefix prefix0
+                     (suffix ++ suf) (suffix0 ++ suf')
+                     _ _) in H8; eauto.
+        -- destruct H8.
+           destruct H1.
+           subst.
+           repeat rewrite <- app_assoc in H4.
+           assert (suffix ++ suf = suffix0 ++ suf') by admit.
+           (* this is an easy prefix/suffix fact *)
+           eapply IHtr0 with (pre := suffix)
+                             (pre' := suffix0)
+                             (suf := suf)
+                             (suf' := suf') in H12; eauto.
+           ++ destruct H12.
+              destruct H5.
+              destruct H6.
+              subst.
+Abort.
+
+Lemma two_gammas :
+  forall tbl g,
+    isParseTableFor tbl g
+    -> forall x gamma gamma' word word' f f',
+      In (x, gamma) (productions g)
+      -> In (x, gamma') (productions g)
+      -> (@derivesGamma g) gamma word f
+      -> (@derivesGamma g) gamma' word' f'
+      -> (peek word = peek word' -> gamma = gamma')
+         /\ (peek word <> peek word' -> gamma <> gamma').
+Proof.
+Admitted.
+
+Lemma derives_det''' :
+  forall tbl g,
+    isParseTableFor tbl g
+    -> forall tr tr' sym pre pre' suf suf',
+      (@derivesSym g) sym pre tr
+      -> (@derivesSym g) sym pre' tr'
+      -> pre ++ suf = pre' ++ suf'
+      -> peek (pre ++ suf) = peek (pre' ++ suf')
+      -> pre = pre' /\ suf = suf' /\ tr = tr'.
+Proof.
+  intros tbl g Htbl.
+  pose proof Htbl as Htbl'.
+  destruct Htbl as [Hmin Hcom].
+  induction tr using tree_mutual_ind with
+      (P0 := fun f =>
+               forall f' x gPre gamma pre pre' suf suf',
+                 In (x, gPre ++ gamma) (productions g)
+                 -> (@derivesGamma g) gamma pre f
+                 -> (@derivesGamma g) gamma pre' f'
+                 -> pre ++ suf = pre' ++ suf'
+                 -> peek (pre ++ suf) = peek (pre' ++ suf')
+                 -> pre = pre' /\ suf = suf' /\ f = f').
+
+  - intros.
+    inv H; inv H0.
+    + inv H1.
+      repeat (split; auto).
+    + inv H3.
+
+  - intros.
+    inv H; inv H0.
+    inv H3; inv H4.
+    rename s into x.
+    assert (gamma0 = gamma).
+    { destruct pre as [| ptok ptoks]; simpl in *.
+      - destruct pre' as [| ptok' ptoks']; simpl in *.
+        + subst.
+          apply derivesGamma_nil_nullable in H9.
+          apply derivesGamma_nil_nullable in H0.
+          assert ((@isLookaheadFor g) EOF (NT x) gamma).
+          { unfold isLookaheadFor.
+            right.
+            split.
+            - constructor; auto.
+            - constructor; auto.
+              eapply FoNu.
+              econstructor; eauto. }
+          assert ((@isLookaheadFor g) EOF (NT x) gamma0).
+          { unfold isLookaheadFor.
+            right.
+            split.
+            - constructor; auto.
+            - constructor; auto.
+              eapply FoNu.
+              econstructor; eauto. }
+          apply Hcom in H1; apply Hcom in H3.
+          destruct H1 as [laMap [Hsf Hlf]].
+          destruct H3 as [laMap' [Hsf' Hlf']].
+          congruence.
+        + destruct suf as [| stok stoks]; simpl in *.
+          * inv H2.
+          * inv H2.
+            
+      - destruct pre' as [| ptok' ptoks']; simpl in *.
+        + inv H2.
+        + inv H1.
+          apply derivesGamma_cons_firstGamma in H0.
+          apply derivesGamma_cons_firstGamma in H9.
+          assert ((@isLookaheadFor g) (LA ptok') (NT x) gamma).
+          { unfold isLookaheadFor.
+            left.
+            constructor; auto. }
+          assert ((@isLookaheadFor g) (LA ptok') (NT x) gamma0).
+          { unfold isLookaheadFor.
+            left.
+            constructor; auto. }
+          apply Hcom in H1; apply Hcom in H3.
+          destruct H1 as [laMap [Hsf Hlf]].
+          destruct H3 as [laMap' [Hsf' Hlf']].
+          congruence. }
+    subst.
+    assert (gamma = [] ++ gamma) by auto.
+    rewrite H3 in H.
+    eapply IHtr in H0; eauto.
+    destruct H0.
+    destruct H4.
+    subst.
+    repeat (split; auto).
+
+  - intros.
+    inv H0; inv H1; auto.
+
+  - intros.
+    destruct gamma as [| sym syms].
+    + inv H0.
+    + destruct f' as [| tr' f'].
+      * inv H1.
+      * inv H0; inv H1.
+        destruct (prefix ++ suffix) eqn:Hpre; simpl in *.
+        -- destruct (prefix0 ++ suffix0) eqn:Hpre0; simpl in *.
+           ++ subst.
+              assert (prefix = nil) by admit.
+              assert (prefix0 = nil) by admit.
+              assert (suffix = nil) by admit.
+              assert (suffix0 = nil) by admit.
+              subst.
+              eapply IHtr in H7; eauto.
+              destruct H7.
+              destruct H1.
+              subst.
+              eapply IHtr0 with (suf := nil)
+                                (suf' := nil) in H11; eauto.
+              ** destruct H11.
+                 destruct H4.
+                 subst.
+                 repeat (split; auto).
+              ** admit.
+           ++ inv H3.
+        -- destruct (prefix0 ++ suffix0) eqn:Hpre0; simpl in *.
+           ++ inv H3.
+           ++ inv H3.
+              destruct prefix; destruct suffix; simpl in *.
+              ** inv Hpre.
+              ** inv Hpre.
+Abort.                
+
+
+(* This gets us almost all the way there, but proving that
+   gamma = gamma0 is the problem. We need to change the
+   derivesSym hypothesis so that it talks about a symbol
+   in the middle of some right-hand side *)
+Lemma derives_det' :
+  forall tbl g,
+    isParseTableFor tbl g
+    -> forall tr tr' sym pre pre' suf suf',
+      (@derivesSym g) sym pre tr
+      -> (@derivesSym g) sym pre' tr'
+      -> pre ++ suf = pre' ++ suf'
+      -> pre = pre' /\ suf = suf' /\ tr = tr'.
+Proof.
+  intros tbl g Htbl.
+  pose proof Htbl as Htbl'.
+  destruct Htbl as [Hmin Hcom].
+  induction tr using tree_mutual_ind with
+      (P0 := fun f =>
+               forall f' x gPre gamma pre pre' suf suf',
+                 In (x, gPre ++ gamma) (productions g)
+                 -> (@derivesGamma g) gamma pre f
+                 -> (@derivesGamma g) gamma pre' f'
+                 -> pre ++ suf = pre' ++ suf'
+                 -> pre = pre' /\ suf = suf' /\ f = f').
+  
+  - intros.
+    inv H; inv H0.
+    + inv H1.
+      repeat (split; auto).
+    + inv H2.
+
+  - intros.
+    inv H; inv H0.
+    inv H2; inv H3.
+    rename s into x.
+    (*
+    assert (gamma0 = gamma).
+    { destruct pre as [| ptok ptoks]; simpl in *.
+      - destruct pre' as [| ptok' ptoks']; simpl in *.
+        + apply derivesGamma_nil_nullable in H0.
+          apply derivesGamma_nil_nullable in H8.
+          assert ((@isLookaheadFor g) EOF (NT x) gamma0).
+          { unfold isLookaheadFor.
+            right.
+            split.
+            - constructor; auto.
+            - constructor; auto.
+              econstructor.
+              econstructor; eauto. }
+          assert ((@isLookaheadFor g) EOF (NT x) gamma).
+          { unfold isLookaheadFor.
+            right.
+            split.
+            - constructor; auto.
+            - constructor; auto.
+              econstructor.
+              econstructor; eauto. }
+          apply Hcom in H2; apply Hcom in H3.
+          destruct H2 as [laMap [Hsf Hlf]].
+          destruct H3 as [laMap' [Hsf' Hlf']].
+          congruence.
+        + admit.
+      *)      
+
+    assert (gamma0 = gamma) by admit.
+    subst.
+    assert (gamma = [] ++ gamma) by auto.
+    rewrite H2 in H.
+    eapply IHtr in H0; eauto.
+    destruct H0.
+    destruct H3.
+    subst; repeat (split; auto).
+          
+  - intros.
+    inv H0; inv H1; auto.
+
+  - intros.
+    destruct gamma as [| sym syms].
+    + inv H0.
+    + destruct f' as [| tr' f'].
+      * inv H1.
+      * inv H0; inv H1.
+        repeat rewrite <- app_assoc in H2.
+        assert (sym :: syms = [sym] ++ syms) by auto.
+        rewrite H0 in H.
+        rewrite app_assoc in H.
+        eapply IHtr with (pre := prefix) in H6; eauto.
+        destruct H6.
+        destruct H3.
+        subst.
+        eapply IHtr0 with (pre := suffix) in H10; eauto.
+        destruct H10.
+        destruct H4.
+        subst.
+        repeat (split; auto).
+Admitted.
+           
+        
+        
+    
+  
+
+Lemma if_trees_eq_then_syms_and_words_eq :
+  forall tbl g,
+    isParseTableFor tbl g
+    -> forall tr tr' sym sym' word word',
+      (@derivesSym g) sym word tr
+      -> (@derivesSym g) sym' word' tr'
+      -> (tr = tr' -> sym = sym' /\ word = word')
+         /\ (tr <> tr' -> sym <> sym' \/ word <> word').
+Proof.
+  intros tbl g Htbl.
+  pose proof Htbl as Htbl'.
+  destruct Htbl as [Hmin Hcom].
+  induction tr using tree_mutual_ind with
+      (P0 := fun f =>
+               forall f' x pre gamma gamma' word word',
+                 In (x, pre ++ gamma) (productions g)
+                 -> In (x, pre ++ gamma') (productions g)
+                 -> (@derivesGamma g) gamma word f
+                 -> (@derivesGamma g) gamma' word' f'
+                 -> (f = f' ->  gamma = gamma' /\ word = word')
+                    /\ (f <> f' -> gamma <> gamma'
+                                   \/ word <> word')).
+
+  - intros.
+    inv H.
+    + inv H0.
+      * split.
+        -- intros; split; congruence.
+        -- intros.
+           left.
+           unfold not; intros.
+           inv H0.
+           congruence.
+      * inv H.
+        split; intros.
+        -- congruence.
+        -- left.
+           congruence.
+    + inv H1.
+
+  - intros.
+    inv H; inv H0.
+    inv H1.
+    split; intros.
+    + congruence.
+    + left.
+      congruence.
+    + inv H1; inv H.
+      split; intros.
+      * inv H.
+        eapply IHtr with (pre := nil) (gamma := gamma) in H0;
+          eauto.
+        destruct H0.
+        destruct H; auto.
+      * destruct (forest_eq_dec f f0).
+        -- subst.
+           
+        
+          
+        
+
+    
+Qed.      
+        
+
+(* This time, we relax the restriction that the two words be
+   equal, and just require them to share a lookahead token *)
+Lemma derives_det :
+  forall tbl g,
+    isParseTableFor tbl g
+    -> forall tr tr' sym word word',
+      (@derivesSym g) sym word tr
+      -> (@derivesSym g) sym word' tr'
+      -> peek word = peek word'
+      -> tr = tr' /\ word = word'.
+Proof.
+  intros tbl g Htbl.
+  pose proof Htbl as Htbl'.
+  destruct Htbl as [Hmin Hcom].
+  induction tr using tree_mutual_ind with
+      (P0 := fun f =>
+               forall f' x pre gamma word,
+                 In (x, pre ++ gamma) (productions g)
+                 -> (@derivesGamma g) gamma word f
+                 -> (@derivesGamma g) gamma word f'
+                 ->  f = f').
+  - intros.
+    inv H; inv H0; auto.
+    inv H2.
+
+  - intros.
+    inv H; inv H0.
+    inv H2; inv H3.
+    assert (gamma0 = gamma) by admit. (* get this from LL(1) *)
+    subst.
+    assert (gamma = [] ++ gamma) by auto.
+    rewrite H2 in H.
+    split.
+    + erewrite IHtr; auto.
+      * eauto.
+      * eauto.
+      * (* we're stuck, because the IH still requires the two
+           words to be the same. Let's try relaxing that
+           restriction. *)
+Abort.
+
+
+
+
+    
+
+Lemma if_trees_eq_then_syms_and_words_eq :
+  forall tbl g,
+    isParseTableFor tbl g
+    -> forall tr sym sym' word word',
+      (@derivesSym g) sym word tr
+      -> (@derivesSym g) sym' word' tr
+      -> sym = sym' /\ word = word'.
+Proof.
+  intros tbl g Htbl.
+  pose proof Htbl as Htbl'.
+  destruct Htbl as [Hmin Hcom].
+  induction tr using tree_mutual_ind with
+      (P0 := fun f =>
+               forall x pre gamma gamma' word word',
+                 In (x, pre ++ gamma) (productions g)
+                 -> In (x, pre ++ gamma') (productions g)
+                 -> (@derivesGamma g) gamma word f
+                 -> (@derivesGamma g) gamma' word' f
+                 ->  gamma = gamma' /\ word = word').
+
+  - intros.
+    inv H.
+    + inv H0.
+      * split; auto.
+      * inv H.
+    + inv H1.
+
+  - intros.
+    inv H; inv H0.
+    inv H; inv H1.
+    eapply IHtr with (gamma := gamma)
+                     (word := word) in H7; auto.
+    + destruct H7.
+      split; auto.
+    + assert (gamma = [] ++ gamma) by auto.
+      rewrite H in H5.
+      eauto.
+    + auto.
+  - intros.
+    inv H1; inv H2.
+    split; auto.
+    
+  - intros.
+    inv H1; inv H2.
+    eapply IHtr with
+        (sym := hdSym) (word := prefix) in H6; auto.
+    destruct H6; subst.
+    eapply IHtr0 with
+        (gamma := tlSyms) (word := suffix) in H9; auto.
+    + destruct H9.
+      subst; split; auto.
+    + assert (hdSym0 :: tlSyms = [hdSym0] ++ tlSyms) by auto.
+      rewrite H1 in H.
+      rewrite app_assoc in H.
+      eauto.
+    + assert (hdSym0 :: tlSyms0 = [hdSym0] ++ tlSyms0) by auto.
+      rewrite H1 in H0.
+      rewrite app_assoc in H0.
+      auto.
+Qed.      
+
+
+
+
+
+Lemma derives_cons_NT_det :
+  forall tbl g,
+    isParseTableFor tbl g
+    -> forall tr tr' x tok toks toks',
+      (@derivesSym g) (NT x) (tok :: toks) tr
+      -> (@derivesSym g) (NT x) (tok :: toks') tr'
+      -> tr = tr' /\ toks = toks'.
+Proof.
+  intros tbl g Htbl.
+  pose proof Htbl as Htbl'.
+  destruct Htbl as [Hmin Hcom].
+  induction tr using tree_mutual_ind with
+      (P0 := fun f =>
+               forall f' x pre gamma tok toks toks',
+                 In (x, pre ++ gamma) (productions g)
+                 -> (@derivesGamma g) gamma (tok :: toks) f
+                 -> (@derivesGamma g) gamma (tok :: toks') f'
+                 -> f = f' /\ toks = toks').
+  - intros.
+    inv H.
+    inv H2.
+    
+  - intros.
+    inv H.
+    inv H2.
+    inv H0.
+    inv H1.
+    assert (gamma0 = gamma) by admit.
+    subst.
+    assert (gamma = [] ++ gamma) by auto.
+    rewrite H1 in H.
+    eapply IHtr in H0; eauto.
+    destruct H0.
+    subst.
+    split; auto.
+
+  - intros.
+    inv H0.
+    
+  - intros.
+    inv H0.
+    inv H1.
+    destruct hdSym as [y | x2].
+    + destruct prefix as [| ptok ptoks]; simpl in *.
+      * inv H6.
+      * destruct prefix0 as [| ptok' ptoks']; simpl in *.
+        -- inv H5.
+        -- inv H4.
+           inv H2.
+           inv H5.
+           inv H6.
+           simpl in *.
+           
+           
+           split; auto.
+    + destruct prefix as [| ptok ptoks]; simpl in *.
+      * destruct prefix0 as [| ptok' ptoks']; simpl in *.
+        -- eapply derives_nil_det with (tr := tr) in H3; eauto.
+           subst.
+           split; auto.
+        -- destruct suffix0 as [| stok stoks]; simpl in *.
+           ++ 
+      
+           
+           
+
+    
+  induction tr using tree_mutual_ind with
+      (P0 := fun f =>
+               forall f' x pre gamma tok toks toks',
+                 In (x, pre ++ gamma) (productions g)
+                 -> (@derivesGamma g) gamma (tok :: toks) f
+                 -> (@derivesGamma g) gamma (tok :: toks') f'
+                 -> f = f' /\ toks = toks').
+
+  - intros.
+    inv H.
+    + inv H0.
+      split; auto.
+    + inv H1.
+
+  - intros.
+    inv H.
+    inv H1.
+    inv H0.
+    inv H1.
+    assert (gamma0 = gamma) by admit.
+    subst.
+    assert (gamma = [] ++ gamma) by auto.
+    rewrite H1 in H.
+    eapply IHtr in H0; eauto.
+    destruct H0.
+    subst.
+    split; auto.
+
+  - intros.
+    inv H0.
+
+  - intros.
+    inv H0.
+    inv H1.
+    destruct hdSym as [y | x2].
+    + destruct prefix.
+      * inv H6.
+      * destruct prefix0.
+        -- inv H5.
+        -- inv H4.
+           eapply IHtr with (toks := []) in H5.
+           ++ destruct H5.
+              subst.
+      * inv H5.
+      * simpl in *.
+        inv H4.
+      
+    
+Lemma if_trees_eq_then_syms_and_words_eq :
+  forall tbl g,
+    isParseTableFor tbl g
+    -> forall tr tr' sym word word',
+      (@derivesSym g) sym word tr
+      -> (@derivesSym g) sym word' tr'
+      -> peek word = peek word'
+      -> tr = tr' /\ word = word'.
+Proof.
+  intros tbl g Htbl.
+  pose proof Htbl as Htbl'.
+  destruct Htbl as [Hmin Hcom].
+  induction tr using tree_mutual_ind with
+      (P0 := fun f =>
+               forall f' x pre gamma word word',
+                 In (x, pre ++ gamma) (productions g)
+                 -> (@derivesGamma g) gamma word f
+                 -> (@derivesGamma g) gamma word' f'
+                 -> peek word = peek word'
+                 -> f = f' /\ word = word').
+  - intros.
+    inv H; inv H0; auto.
+    inv H2.
+
+  - intros.
+    inv H; inv H0.
+    inv H2; inv H3.
+    assert (gamma0 = gamma) by admit.
+    subst.
+    eapply IHtr with (word := word) in H0; eauto.
+    + destruct H0; subst; split; auto.
+    + assert (gamma = [] ++ gamma) by auto.
+      rewrite H2 in H.
+      eauto.
+
+  - intros.
+    inv H0; inv H1; auto.
+
+  - intros.
+
+    
+        
+
+
+
+
+
+
+
+
+
+
+    
+    
+Lemma if_trees_eq_then_syms_and_words_eq :
+  forall tbl g,
+    isParseTableFor tbl g
+    -> forall tr tr' sym sym' word word',
+      (@derivesSym g) sym word tr
+      -> (@derivesSym g) sym' word' tr'
+      -> peek word = peek word'
+      -> (tr = tr' -> sym = sym' /\ word = word')
+         /\ (tr <> tr' -> sym <> sym').
+Proof.
+  intros tbl g Htbl.
+  pose proof Htbl as Htbl'.
+  destruct Htbl as [Hmin Hcom].
+  induction tr using tree_mutual_ind with
+      (P0 := fun f =>
+               forall f' gamma gamma' word word',
+                 (@derivesGamma g) gamma word f
+                 -> (@derivesGamma g) gamma' word' f'
+                 -> peek word = peek word'
+                 -> (f = f' -> gamma = gamma' /\ word = word')
+                    /\ (f <> f' -> gamma <> gamma')).
+  
+  - intros.
+    inv H.
+    + inv H0.
+      * split; intros.
+        -- inv H.
+           split; auto.
+        -- congruence.
+      * inv H.
+        split; intros; congruence.
+    + inv H2.
+
+  - intros.
+    inv H.
+    inv H2.
+    inv H0.
+    + split; intros; congruence.
+    + inv H.
+      pose proof H2 as H2'.
+      eapply IHtr with (gamma := gamma) (word := word)
+        in H2; eauto.
+      destruct H2.
+      split; intros.
+      * inv H3.
+        destruct H; auto.
+      * unfold not; intros.
+        inv H4.
+        assert (gamma0 = gamma) by admit.
+        subst.
+        destruct (forest_eq_dec f f0).
+        -- subst.
+           congruence.
+        -- apply H2 in n.
+           congruence.
+
+  - intros.
+    inv H; inv H0.
+    + split; intros; auto.
+    + split; intros; congruence.
+
+  - intros.
+    inv H; inv H0.
+    + split; intros; congruence.
+    + split; intros.
+      * inv H0.
+        destruct prefix as [| ptok ptoks]; simpl in *.
+        -- destruct prefix0 as [| ptok' ptoks']; simpl in *.
+           ++ destruct suffix as [| stok stoks]; simpl in *.
+              ** simpl in *.
+                 destruct suffix0 as [| stok' stoks'];
+                   simpl in *.
+                 --- eapply IHtr0 with
+                         (gamma := tlSyms) in H2; eauto.
+                     destruct H2.
+                     destruct H0; auto.
+                     subst.
+                     eapply IHtr with (sym := hdSym)
+                       in H; eauto.
+                     destruct H.
+                     destruct H; auto.
+                     subst.
+                     split; auto.
+                 --- inv H1.
+              ** destruct suffix0 as [| stok' stoks'];
+                   simpl in *.
+                 --- inv H1.
+                 --- inv H1.
+                     eapply IHtr0 with
+                         (gamma := tlSyms) in H2; eauto.
+                     destruct H2.
+                     destruct H0; auto.
+                     inv H2.
+                     subst.
+                     eapply IHtr with
+                         (sym := hdSym) in H; eauto.
+                     destruct H.
+                     destruct H; auto.
+                     subst.
+                     split; auto.
+           ++ destruct suffix as [| stok stoks]; simpl in *.
+              ** inv H1.
+              ** inv H1.
+                 destruct suffix0 as [| stok' stoks'];
+                   simpl in *.
+                 --- eapply IHtr0 with (gamma := tlSyms)
+                     in H2; eauto.
+                     +++ destruct H2.
+                         destruct H0; auto.
+                         inv H2.
+                     +++ eapply IHtr
+
+             
+  - intros.
+    inv H1; inv H2.
+    + split; intros; congruence.
+    + split; intros.
+      * inv H2.
+        eapply IHtr with (sym := hdSym) in H3; eauto.
+        -- destruct H3.
+           destruct H2; auto.
+           eapply IHtr0 with (gamma := tlSyms) in H5; eauto.
+           ++ destruct H5.
+              destruct H2; auto.
+           ++ assert (hdSym :: tlSyms = [hdSym] ++ tlSyms)
+               by auto.
+              rewrite H2 in H.
+              rewrite app_assoc in H.
+              eauto.
+           ++ assert (hdSym :: tlSyms0 = [hdSym] ++ tlSyms0)
+               by auto.
+              rewrite H2 in H0.
+              rewrite app_assoc in H0.
+              auto.
+           ++ 
+
+Lemma derivesSym_det :
+  forall tbl g,
+    isParseTableFor tbl g
+    -> forall tr tr' sym word word',
+      (@derivesSym g) sym word tr
+      -> (@derivesSym g) sym word' tr'
+      -> peek word = peek word'
+      -> tr = tr'.
+Proof.
+  intros tbl g Htbl.
+  pose proof Htbl as Htbl'.
+  destruct Htbl as [Hmin Hcom].
+  induction tr using tree_mutual_ind with
+      (P0 := fun f =>
+               forall f' x pre gamma word word',
+                 In (x, pre ++ gamma) (productions g)
+                 -> (@derivesGamma g) gamma word f
+                 -> (@derivesGamma g) gamma word' f'
+                 -> f = f').
+  - intros.
+    inv H; inv H0; auto.
+    inv H2.
+
+  - intros.
+    inv H; inv H0.
+    inv H2; inv H3.
+    assert (gamma0 = gamma) by admit.
+    subst.
+    assert (gamma = [] ++ gamma) by auto.
+    rewrite H2 in H.
+    erewrite IHtr; eauto.
+
+  - intros.
+    inv H0; inv H1; auto.
+
+  - intros.
+    inv H0; inv H1.
+    destruct hdSym as [y | x2].
+    + inv H3; inv H6.
+      assert (T y :: tlSyms = [T y] ++ tlSyms) by auto.
+      rewrite H0 in H.
+      rewrite app_assoc in H.
+      erewrite IHtr0; eauto.
+    + 
+    destruct prefix as [| ptok ptoks].
+    + destruct prefix0 as [| ptok' ptoks']; simpl in *.
+      * eapply IHtr in H3; eauto.
+        subst.
+        eapply IHtr0 in H8; eauto.
+        subst.
+        auto.
+      * (* first/follow *)
+        inv H6; inv H3.
+        inv H; inv H2.
+        destruct suffix as [| stok stoks].
+        -- inv H1.
+        -- simpl in *.
+           inv H1.
+           
+
+
+
+        
+           
+
+    
+
+Lemma if_trees_eq_then_syms_and_words_eq :
+  forall tbl g,
+    isParseTableFor tbl g
+    -> forall tr sym sym' word word',
+      (@derivesSym g) sym word tr
+      -> (@derivesSym g) sym' word' tr
+      -> sym = sym' /\ word = word'.
+Proof.
+  intros tbl g Htbl.
+  pose proof Htbl as Htbl'.
+  destruct Htbl as [Hmin Hcom].
+  induction tr using tree_mutual_ind with
+      (P0 := fun f =>
+               forall x pre gamma gamma' word word',
+                 In (x, pre ++ gamma) (productions g)
+                 -> In (x, pre ++ gamma') (productions g)
+                 -> (@derivesGamma g) gamma word f
+                 -> (@derivesGamma g) gamma' word' f
+                 ->  gamma = gamma' /\ word = word').
+
+  - intros.
+    inv H.
+    + inv H0.
+      * split; auto.
+      * inv H.
+    + inv H1.
+
+  - intros.
+    inv H; inv H0.
+    inv H; inv H1.
+    eapply IHtr with (gamma := gamma)
+                     (word := word) in H7; auto.
+    + destruct H7.
+      split; auto.
+    + assert (gamma = [] ++ gamma) by auto.
+      rewrite H in H5.
+      eauto.
+    + auto.
+  - intros.
+    inv H1; inv H2.
+    split; auto.
+    
+  - intros.
+    inv H1; inv H2.
+    eapply IHtr with
+        (sym := hdSym) (word := prefix) in H6; auto.
+    destruct H6; subst.
+    eapply IHtr0 with
+        (gamma := tlSyms) (word := suffix) in H9; auto.
+    + destruct H9.
+      subst; split; auto.
+    + assert (hdSym0 :: tlSyms = [hdSym0] ++ tlSyms) by auto.
+      rewrite H1 in H.
+      rewrite app_assoc in H.
+      eauto.
+    + assert (hdSym0 :: tlSyms0 = [hdSym0] ++ tlSyms0) by auto.
+      rewrite H1 in H0.
+      rewrite app_assoc in H0.
+      auto.
+Qed.      
+    
+    
+Lemma derivesSym_det :
+  forall tbl g,
+    isParseTableFor tbl g
+    -> forall tr sym sym' word word',
+      (@derivesSym g) sym word tr
+      -> (@derivesSym g) sym' word' tr'
+      -> (tr = tr' -> sym = sym' /\ word = word').
+         (* /\ (tr <> tr' -> sym <> sym'). *)
+Proof.
+  intros tbl g Htbl.
+  pose proof Htbl as Htbl'.
+  destruct Htbl as [Hmin Hcom].
+  induction tr using tree_mutual_ind with
+      (P0 := fun f =>
+               forall f' x pre gamma gamma' word word',
+                 In (x, pre ++ gamma) (productions g)
+                 -> In (x, pre ++ gamma') (productions g)
+                 -> (@derivesGamma g) gamma word f
+                 -> (@derivesGamma g) gamma' word' f'
+                 -> (f = f' -> gamma = gamma' /\ word = word')
+                    /\ (f <> f' -> gamma <> gamma')).
+
+  - intros.
+    inv H.
+    + inv H0.
+      * split; intros.
+        -- inv H; split; auto.
+        -- congruence.
+      * inv H; split; intros; congruence.
+    + inv H1.
+        
+  - intros.
+    inv H.
+    inv H1.
+    inv H0.
+    + split; intros; congruence.
+    + inv H.
+      destruct (forest_eq_dec f f0).
+      * subst.
+        assert (gamma = [] ++ gamma) by auto.
+        rewrite H in H6.
+        eapply IHtr with (gamma := gamma) in H1; auto.
+        -- split; intros.
+           ++ inv H2.
+              destruct H1.
+              destruct H1; auto.
+              split; eauto.
+           ++ unv
+           subst.
+           split; intros.
+           ++ inv H1; split; auto.
+           ++ unfold not; intros.
+              inv H3.
+              apply H1.
+              auto.
+        -- assert (gamma0 = [] ++ gamma0) by auto.
+           rewrite H2 in H0.
+           auto.
+      split; intros.
+      * inv H.
+        split; auto.
+      * unfold not; intros.
+        inv H2.
+        apply H; clear H.
+        assert (gamma0 = gamma) by admit.
+        subst.
+        assert (gamma = [] ++ gamma) by auto.
+        rewrite H in H0.
+        eapply IHtr with (gamma := gamma) in H1; eauto.
+        destruct H1.
+        destruct (forest_eq_dec f f0).
+        -- subst; auto.
+        -- simpl in *.
+           apply H2 in n.
+           congruence.
+
+  - intros.
+    inv H1; inv H2; split; intros; auto; try congruence.
+
+  - intros.
+    inv H1; inv H2; split; intros; try congruence.
+    + inv H2.
+      
+        
+        
+        
+      
+
+
+Lemma derivesSym_det :
+  forall tbl g,
+    isParseTableFor tbl g
+    -> forall tr tr' sym word,
+      (@derivesSym g) sym word tr
+      -> (@derivesSym g) sym word tr'
+      -> tr = tr'.
+  intros tbl g Htbl.
+  pose proof Htbl as Htbl'.
+  destruct Htbl as [Hmin Hcom].
+  induction tr using tree_mutual_ind with
+      (P0 := fun f =>
+               forall x pre gamma word f',
+                 In (x, pre ++ gamma) (productions g)
+                 -> (@derivesGamma g) gamma word f
+                 -> (@derivesGamma g) gamma word f'
+                 -> f = f').
+  - intros.
+    inv H; inv H0; auto.
+    inv H1.
+
+  - intros.
+    inv H; inv H0.
+    inv H1; inv H2.
+    assert (gamma0 = gamma) by admit.
+    subst.
+    assert (gamma = [] ++ gamma) by auto.
+    rewrite H1 in H.
+    erewrite IHtr; eauto.
+
+  - intros.
+    inv H0; inv H1; auto.
+
+  - intros.
+    inv H0.
+    
+
+
+Lemma derivesProd_det :
+  forall tbl g,
+    isParseTableFor tbl g
+    -> forall tr x gamma word,
+      (@derivesProd g) x gamma word tr
+      -> forall tr',
+          (@derivesProd g) x gamma word tr'
+          -> tr = tr'.
+Proof.
+  intros tbl g Htbl tr x gamma word Hderp.
+  pose proof Htbl as Htbl'.
+  destruct Htbl as [Hmin Hcom].
+  induction Hderp using derivesProd_mut_ind with
+      (P := fun x gamma word tr
+                (pf : (@derivesProd g) x gamma word tr) =>
+              forall tr',
+                (@derivesProd g) x gamma word tr'
+                -> tr = tr')
+      (P0 := fun gSuf wSuf fSuf
+                 (pf : (@derivesGamma g) gSuf wSuf fSuf) =>
+               forall x gPre fSuf',
+                 In (x, gPre ++ gSuf) (productions g)
+                 -> (forall wPre fPre fPre',
+                        (@derivesGamma g) gPre wPre fPre
+                        -> (@derivesGamma g) gPre wPre fPre'
+                        -> fPre = fPre')
+                 -> (@derivesGamma g) gSuf wSuf fSuf'
+                 -> fSuf = fSuf')
+      (P1 := fun sym word tr
+                 (pf : (@derivesSym g) sym word tr) =>
+                  forall tr',
+                    (@derivesSym g) sym word tr'
+                    -> tr = tr').
+
+  - intros.
+    inv H.
+    assert (gamma = [] ++ gamma) by auto.
+    rewrite H in H0.
+    erewrite IHHderp; eauto.
+    intros.
+    inv H2.
+    inv H3.
+    auto.
+
+  - intros.
+    rewrite app_nil_r in *.
+    inv H1.
+    auto.
+
+  - intros.
+    inv H1.
+Abort.              
+
+Lemma derivesSym_det :
+  forall tbl g,
+    isParseTableFor tbl g
+    -> forall tr tr' x pre preWord preF sym word suf,
+      In (x, pre ++ sym :: suf) (productions g)
+      -> (@derivesGamma g) pre preWord preF
+      -> (@derivesSym g) sym word tr
+      -> (@derivesSym g) sym word tr'
+      -> tr = tr'.
+Proof.
+  intros tbl g Htbl.
+  pose proof Htbl as Htbl'.
+  destruct Htbl as [Hmin Hcom].
+  induction tr using tree_mutual_ind with
+      (P0 := fun f =>
+               forall x pre gamma word f',
+                 In (x, pre ++ gamma) (productions g)
+                 -> (@derivesGamma g) gamma word f
+                 -> (@derivesGamma g) gamma word f'
+                 -> f = f').
+  - intros.
+    inv H1; inv H2; auto.
+    inv H3.
+
+  - intros.
+    inv H1; inv H2.
+    inv H3; inv H4.
+    assert (gamma0 = gamma) by admit.
+    subst.
+    assert (gamma = [] ++ gamma) by auto.
+    rewrite H3 in H1.
+    erewrite IHtr; eauto.
+
+  - intros.
+    inv H0; inv H1; auto.
+
+  - intros.
+    destruct gamma as [| sym syms].
+    + inv H0.
+    + destruct sym as [y | x2].
+      * inv H0; inv H1.
+        inv H4; inv H6.
+        inv H3.
+        assert (T y :: syms = [T y] ++ syms) by auto.
+        rewrite H0 in H.
+        rewrite app_assoc in H.
+        erewrite IHtr0; eauto.
+      * destruct word as [| tok toks].
+        -- 
+        
+    
+    
+      
+
+    
+Lemma derivesSym_det :
+  forall tbl g,
+    isParseTableFor tbl g
+    -> forall tr tr' sym word,
+      (@derivesSym g) sym word tr
+      -> (@derivesSym g) sym word tr'
+      -> tr = tr'.
+  intros tbl g Htbl.
+  pose proof Htbl as Htbl'.
+  destruct Htbl as [Hmin Hcom].
+  induction tr using tree_mutual_ind with
+      (P0 := fun f =>
+               forall x pre preWord preF gamma word f',
+                 In (x, pre ++ gamma) (productions g)
+                 -> (@derivesGamma g) pre preWord preF
+                 -> (@derivesGamma g) gamma word f
+                 -> (@derivesGamma g) gamma word f'
+                 -> f = f').
+
+  - intros.
+    inv H; inv H0; auto.
+    inv H1.
+
+  - intros.
+    inv H; inv H0.
+    inv H1; inv H2.
+    assert (gamma0 = gamma) by admit.
+    subst.
+    assert (gamma = [] ++ gamma) by auto.
+    erewrite IHtr with (pre := nil); eauto.
+    constructor.
+
+  - intros.
+    inv H1; inv H2; auto.
+
+  - intros.
+    destruct gamma as [| sym suf].
+    + inv H1.
+    + destruct sym as [y | x2].
+      * inv H1; inv H2.
+        inv H5; inv H7.
+        inv H4.
+        erewrite IHtr0 with (f' := tlTrees); auto.
+        -- assert (T y :: suf = [T y] ++ suf) by auto.
+           rewrite H1 in H.
+           rewrite app_assoc in H.
+           eauto.
+        -- eapply derives_app; eauto.
+           repeat constructor.
+        -- eauto.
+        -- auto.
+      * destruct word as [| tok toks].
+        -- inv H1; inv H2.
+           
+Proof.
+
+Lemma derivesSym_det :
+  forall tbl g,
+    isParseTableFor tbl g
+    -> forall gamma x pre preWord preF word f f',
+      In (x, pre ++ gamma) (productions g)
+      -> (@derivesGamma g) gamma word f
+      -> (@derivesGamma g) gamma word f'
+      -> (@derivesGamma g) pre preWord preF
+      -> f = f'.
+Proof.
+  intros tbl g Htbl.
+  pose proof Htbl as Htbl'.
+  destruct Htbl as [Hmin Hcom].
+  induction gamma as [| sym syms].
+  - intros.
+    inv H0; inv H1; auto.
+  - intros.
+    destruct sym as [y | x2].
+    + destruct word as [| tok toks].
+      * inv H0.
+        assert (prefix = nil) by admit.
+        subst.
+        inv H6.
+      * inv H0; inv H1.
+        inv H6; inv H7.
+        inv H5; inv H4.
+        erewrite IHsyms with (f := tlTrees)
+                             (f' := tlTrees0); auto.
+        -- assert (T tok :: syms = [T tok] ++ syms) by auto.
+           rewrite H0 in H.
+           rewrite app_assoc in H.
+           eauto.
+        -- eauto.
+        -- auto.
+        -- eapply derives_app; eauto.
+           repeat constructor.
+    + destruct word as [| tok toks].
+      * inv H0; inv H1.
+        assert (suffix = nil) by admit.
+        assert (suffix0 = nil) by admit.
+        subst.
+        rewrite app_nil_r in *.
+        subst.
+
+        
+        
+      
+
+    
+
+    
+  - intros.
+    inv H0; inv H1; auto.
+    assert (prefix = nil) by admit.
+    assert (prefix0 = nil) by admit.
+    assert (suffix = nil) by admit.
+    assert (suffix0 = nil) by admit.
+    subst.
+    destruct hdSym as [y | x2].
+    + inv H3.
+    + admit.
+  - intros.
+    
+      
+
+
+    
+Lemma derivesSym_det :
+  forall tbl g,
+    isParseTableFor tbl g
+    -> forall tr tr' x pre sym suf word,
+      In (x, pre ++ sym :: suf) (productions g)
+      -> (@derivesSym g) sym word tr
+      -> (@derivesSym g) sym word tr'
+      -> tr = tr'.
+Proof.
+  intros tbl g Htbl.
+  pose proof Htbl as Htbl'.
+  destruct Htbl as [Hmin Hcom].
+  induction tr using tree_mutual_ind with
+      (P0 := fun f =>
+               forall f' x pre gamma suf word,
+                 In (x, pre ++ gamma ++ suf) (productions g)
+                 -> (@derivesGamma g) gamma word f
+                 -> (@derivesGamma g) gamma word f'
+                 -> f = f').
+                                       
+  - intros.
+    inv H0; inv H1; auto.
+    inv H2.
+
+  - intros.
+    inv H0; inv H1.
+    inv H2; inv H3.
+    assert (gamma0 = gamma) by admit.
+    subst.
+    assert (gamma = nil ++ gamma ++ nil).
+    { rewrite app_nil_r; auto. }
+    rewrite H2 in H0.
+    eapply IHtr in H0; eauto.
+    subst; auto.
+
+  - intros.
+    inv H0; inv H1; auto.
+
+  - intros.
+    destruct gamma as [| sym syms].
+    + inv H0.
+    + inv H0; inv H1.
+      
+    
+
+    
+    + inv H1.
+    + pose proof H1 as H1'.
+      pose proof H2 as H2'.
+      inv H1.
+      inv H2.
+      assert (sym :: syms = [sym] ++ syms) by auto.
+      rewrite H1 in H.
+      rewrite app_assoc in H.
+      pose proof H as H'.
+      eapply (IHtr0 tlTrees x (pre ++ [sym]) syms
+                    (preWord ++ prefix) suffix preF) in H.
+      * destruct H.
+        pose proof H5.
+        admit.
+      * 
+        apply IHtr in H5; auto.
+        -- rewrite H.
+           rewrite H5.
+           auto.
+        -- 
+
+          
+                with (preWord := preWord ++ prefix) in H.
+      pose proof H as H''.
+      destruct H.
+      assert (appF preF (Fcons tr f) =
+              appF (appF preF (Fcons tr Fnil)) f) by admit.
+      rewrite H3; clear H3.
+      assert (appF preF (Fcons hdTree tlTrees) =
+              appF (appF preF (Fcons hdTree Fnil)) tlTrees) by admit.
+      rewrite H3; clear H3.
+      split.
+      * rewrite H.
+        rewrite H in H2.
+        
+
+
+      eapply IHtr0 with (preF := appF preF (Fcons hdTree Fnil))
+                        (f' := tlTrees) in H.
+      * destruct H.
+        subst.
+        assert (suffix = suffix0) by admit. (* need lemma *)
+        subst.
+        assert (prefix0 = prefix) by admit.
+        subst.
+        apply IHtr in H5; auto.
+        subst.
+        split; auto.
+      * apply derives_app with (wPre := preWord)
+                               (wSuf := prefix0); auto.
+        assert (prefix0 = prefix0 ++ nil).
+        { rewrite app_nil_r; auto. }
+        rewrite H2.
+        constructor.
+        auto.
+        constructor.
+      * eauto.
+      * eauto.
+
+        
+        assert (suffix = suffix0) by admit.
+        subst.
+        assert (prefix = prefix0) by admit.
+        subst.
+        erewrite IHtr; eauto.
+      * eapply derives_app.
+        -- eauto.
+        -- assert (prefix = prefix ++ nil) by
+              (rewrite app_nil_r; auto).
+           rewrite H2.
+           eapply derivesFcons; eauto.
+           constructor.
+      * auto.
+        -- 
+        
+      
+
+    rewrite H2.
+    clear H1; clear H2.
+    assert (appF preF (Fcons hdTree tlTrees) =
+            appF preF (appF (Fcons hdTree Fnil) tlTrees)) by admit.
+    rewrite H1.
+    assert (appF preF (appF (Fcons hdTree Fnil) tlTrees) =
+            appF (appF preF (Fcons hdTree Fnil)) tlTrees) by admit.
+    rewrite H2.
+    clear H1; clear H2.
+    
+
+    
+Lemma derivesGamma_det : 
+  forall tbl g,
+    isParseTableFor tbl g
+    -> forall suf x pre sym word f f',
+      In (x, pre ++ sym :: suf) (productions g)
+      -> (@derivesGamma g) (sym :: suf) word f
+      -> (@derivesGamma g) (sym :: suf) word f'
+      -> f = f'.
+Proof.
+  intros tbl g Htbl.
+  pose proof Htbl as Htbl'.
+  destruct Htbl as [Hmin Hcom].
+  induction suf as [| sym' suf].
+    apply IHsuf in 
+    
+      
+Lemma derivesGamma_det : 
+  forall tbl g,
+    isParseTableFor tbl g
+    -> forall sufForest sufForest'
+              preGamma sufGamma
+              preWord sufWord
+              preForest x,
+      In (x, preGamma ++ sufGamma) (productions g)
+      -> (@derivesGamma g) preGamma preWord preForest
+      -> (@derivesGamma g) sufGamma sufWord sufForest
+      -> (@derivesGamma g) sufGamma sufWord sufForest'
+      -> sufForest = sufForest'.
+Proof.
+  intros tbl g Htbl.
+  pose proof Htbl as Htbl'.
+  destruct Htbl as [Hmin Hcom].
+  induction sufForest using forest_mutual_ind with
+      (P := fun tr =>
+              forall tr' x pre sym symWord suf sufWord sufForest sufForest',
+                In (x, pre ++ sym :: suf) (productions g)
+                -> (@derivesSym g) sym symWord tr
+                -> (@derivesSym g) sym symWord tr'
+                -> (@derivesGamma g) suf sufWord sufForest
+                -> (@derivesGamma g) suf sufWord sufForest'
+                -> Fcons tr sufForest = Fcons tr' sufForest').
+  - intros.
+    inv H0; inv H1; auto.
+    + 
+
+  - intros tr' x pre sym suf word Hin Hder Hder'.
     inv Hder; inv Hder'.
     inv H; inv H1.
     assert (gamma = gamma0) by admit.
     subst.
-    erewrite IHf; eauto.
-    assert (gamma0 = [] ++ gamma0) by auto.
-    rewrite H1 in H.
-    eauto.
+    admit.
 
-  - intros f' x pre gamma word Hin Hder Hder'.
-    inv Hder.
-    inv Hder'.
-    auto.
+  - intros sufForest' preGamma sufGamma preWord sufWord
+           preForest x Hin Hderp Hders Hders'.
+    inv Hders; inv Hders'; auto.
 
-  - intros f' x pre gamma word Hin Hder Hder'.
-    inv Hder; inv Hder'.
-    destruct tlSyms.
-    + inv H6; inv H4.
-      repeat rewrite app_nil_r in *.
-      subst.
-      erewrite IHf; eauto.
-    + 
-      
-    
-    destruct hdSym as [y | x2].
-    + inv H2; inv H3.
-      inv H1.
-      erewrite IHf0; auto.
-      * assert (T y :: tlSyms = [T y] ++ tlSyms) by auto.
-        rewrite H in Hin.
-        rewrite app_assoc in Hin.
-        eauto.
-      * eauto.
-      * auto.
-    + revert Hin.
-      revert pre.
-      revert 
-      * inv H6.
-        inv H4.
-        repeat rewrite app_nil_r in *.
-        subst.
-        erewrite IHf; eauto.
-      * 
+  - intros sufForest' preGamma sufGamma preWord sufWord
+           preForest x Hin Hderp Hders Hders'.
+    inv Hders; inv Hders'.
       
 
           
