LL1/DeterminismWalkthrough.v
@@ -1,0 +1,844 @@
+Require Import List Omega String.
+Require Import Derivation Grammar Lemmas ParseTable Lib.Utils
+        ParseTree LL1.Parser Lib.Tactics
+        LL1.CorrectnessProof LL1.MonotonicityLemmas.
+Import ListNotations.
+Open Scope list_scope.
+
+(* THIS SECTION CONTAINS COMPLETED LEMMAS *)
+
+Lemma derivesForest_nil_nullable :
+  forall f g gamma,
+    (@derivesForest g) gamma [] f
+    -> (@nullableGamma g) gamma.
+Proof.
+  induction f using forest_mutual_ind with
+      (P := fun tr =>
+              forall g x,
+                (@derivesTree g) (NT x) nil tr
+                -> (@nullableSym g) (NT x))
+      (P0 := fun f =>
+               forall g gamma,
+                 (@derivesForest g) gamma nil f
+                 -> (@nullableGamma g) gamma); intros.
+
+  - inv H.
+  - inv H.
+    apply IHf in H5.
+    econstructor.
+    econstructor; eauto.
+  - inv H.
+    constructor.
+  - destruct gamma.
+    + constructor.
+    + inv H.
+      assert (prefix = nil) by
+          (destruct prefix; try inv H2; auto).
+      assert (suffix = nil) by
+          (destruct prefix; try inv H2; auto).
+      subst.
+      inv H4.
+      constructor.
+      * apply IHf.
+        econstructor; eauto.
+      * apply IHf0.
+        auto.
+Qed.
+
+Lemma derivesTree_nil_nullable :
+  forall t g x,
+    (@derivesTree g) (NT x) [] t
+    -> (@nullableSym g) (NT x).
+Proof.
+  induction t using tree_mutual_ind with
+      (P := fun tr =>
+              forall g x,
+                (@derivesTree g) (NT x) nil tr
+                -> (@nullableSym g) (NT x))
+      (P0 := fun f =>
+               forall g gamma,
+                 (@derivesForest g) gamma nil f
+                 -> (@nullableGamma g) gamma); intros.
+
+    - inv H.
+  - inv H.
+    apply IHt in H5.
+    econstructor.
+    econstructor; eauto.
+  - inv H.
+    constructor.
+  - destruct gamma.
+    + constructor.
+    + inv H.
+      assert (prefix = nil) by
+          (destruct prefix; try inv H2; auto).
+      assert (suffix = nil) by
+          (destruct prefix; try inv H2; auto).
+      subst.
+      inv H4.
+      constructor.
+      * apply IHt.
+        econstructor; eauto.
+      * apply IHt0.
+        auto.
+Qed.
+
+Lemma derivesForest_cons_firstGamma :
+  forall f g tok toks gamma,
+    (@derivesForest g) gamma (tok :: toks) f
+    -> (@firstGamma g) (LA tok) gamma.
+Proof.
+  intro f.
+  induction f using forest_mutual_ind with
+      (P0 := fun f =>
+              forall g tok toks gamma,
+                (@derivesForest g) gamma (tok :: toks) f
+                -> (@firstGamma g) (LA tok) gamma)
+      (P := fun tr =>
+               forall g tok toks x,
+                 (@derivesTree g) x (tok :: toks) tr
+                 -> (@firstSym g) (LA tok) x); intros.
+
+  - inv H.
+    constructor.
+
+  - inv H.
+    apply IHf with (tok := tok) (toks := toks) in H5.
+    eapply FiNT.
+    constructor; eauto.
+
+  - inv H.
+
+  - inv H.
+    destruct prefix.
+    + simpl in *.
+      subst.
+      apply IHf0 in H5.
+      destruct hdRoot.
+      * inv H4.
+      * apply FiGammaTl.
+        -- apply derivesTree_nil_nullable in H4.
+           auto.
+        -- auto.
+    + simpl in *.
+      inv H0.
+      apply IHf in H4.
+      apply FiGammaHd.
+      auto.
+Qed.
+
+Lemma nullable_middle_sym :
+  forall g xs ys sym,
+    (@nullableGamma g) (xs ++ sym :: ys)
+    -> (@nullableSym g) sym.
+Proof.
+  induction xs; intros.
+  - simpl in H.
+    inv H.
+    auto.
+  - eapply IHxs.
+    inv H.
+    eauto.
+Qed.
+
+Lemma gamma_with_terminal_not_nullable :
+  forall g xs y zs,
+    (@nullableGamma g) (xs ++ T y :: zs)
+    -> False.
+Proof.
+  induction xs; intros.
+  - simpl in H.
+    inv H.
+  - destruct a.
+    + inv H.
+    + inv H.
+      eapply IHxs; eauto.
+Qed.
+
+Lemma nullable_split :
+  forall g xs ys,
+    (@nullableGamma g) (xs ++ ys)
+    -> (@nullableGamma g) ys.
+Proof.
+  induction xs; intros.
+  - auto.
+  - inv H.
+    eapply IHxs; eauto.
+Qed.
+  
+Lemma no_first_follow_conflicts :
+  forall tbl g,
+    isParseTableFor tbl g
+    -> forall la sym gamma,
+      (@firstProd g) la sym gamma
+      -> (@nullableProd g) sym gamma
+      -> (@followProd g) la sym gamma
+      -> False.
+Proof.
+  intros tbl g Htbl la sym gamma Hfi.
+  destruct Htbl as [Hmin Hcom].
+  induction Hfi using firstProd_mutual_ind with
+      (P := fun la sym gamma
+                (pf : (@firstProd g) la sym gamma) =>
+              (@nullableProd g) sym gamma
+              -> (@followProd g) la sym gamma
+              -> False)
+      (P0 := fun la gammaSuf
+                 (pf : (@firstGamma g) la gammaSuf) =>
+               forall sym gammaPre,
+                 (@firstProd g) la sym (gammaPre ++ gammaSuf)
+                 -> (@nullableProd g) sym (gammaPre ++ gammaSuf)
+                 -> (@followProd g) la sym (gammaPre ++ gammaSuf)
+                 -> False)
+      (P1 := fun la sym (pf : (@firstSym g) la sym) =>
+              (@nullableSym g) sym
+              -> (@followSym g) la sym
+              -> False).
+
+  - intros Hnu Hfo.
+    eapply IHHfi; auto.
+    + assert (gamma = [] ++ gamma) by auto.
+      rewrite H in i.
+      econstructor; eauto.
+    + auto.
+    + auto.
+
+  - intros sym gammaSuf Hfi Hnu Hfo.
+    eapply IHHfi.
+    + inv Hnu.
+      apply nullable_middle_sym in H0.
+      auto.
+    + destruct hd.
+      * inv Hnu.
+        apply gamma_with_terminal_not_nullable in H0.
+        inv H0.
+      * inv Hfo.
+        inv Hnu.
+        eapply FoLeft; eauto.
+        assert (NT n :: tl = [NT n] ++ tl) by auto.
+        rewrite H1 in H3.
+        rewrite app_assoc in H3.
+        eapply nullable_split in H3.
+        auto.        
+
+  - intros sym gammaPre Hfi Hnu Hfo.
+    eapply IHHfi.
+    + assert (NT x :: tl = [NT x] ++ tl) by auto.
+      rewrite H in Hfi.
+      rewrite app_assoc in Hfi.
+      eauto.
+    + rewrite <- app_assoc.
+      simpl.
+      auto.
+    + rewrite <- app_assoc.
+      simpl.
+      auto.
+
+  - intros Hnu Hfo.
+    inv Hnu.
+    inv H.
+
+  - intros Hnu Hfo.
+    inv Hnu.
+    inv H.
+    assert (Hlk : (@isLookaheadFor g) la (NT x) gamma).
+    { unfold isLookaheadFor.
+      left.
+      auto. }
+    assert (Hlk' : (@isLookaheadFor g) la (NT x) ys).
+    { unfold isLookaheadFor.
+      right.
+      split.
+      { constructor; auto. }
+      { constructor; auto. }}
+    unfold ptComplete in Hcom.
+    apply Hcom in Hlk; apply Hcom in Hlk'.
+    destruct Hlk as [laMap [Hsf Hlf]].
+    destruct Hlk' as [laMap' [Hsf' Hlf']].
+    assert (gamma = ys) by congruence.
+    subst.
+    apply IHHfi.
+    + constructor; auto.
+    + constructor; auto.
+Qed.
+
+Lemma firstGamma_split :
+  forall g la xs ys,
+    (@firstGamma g) la xs
+    -> (@firstGamma g) la (xs ++ ys).
+Proof.
+  induction xs; intros.
+  - inv H.
+  - inv H.
+    + constructor; auto.
+    + eapply FiGammaTl; eauto.
+Qed.
+
+ Fixpoint appF f f2 :=
+   match f with
+   | Fnil => f2
+   | Fcons tr f' => Fcons tr (appF f' f2)
+   end.
+
+Lemma appF_nil_r : forall f,
+    appF f Fnil = f.
+Proof.
+  induction f; simpl.
+  - auto.
+  - rewrite IHf. auto.
+Qed.
+
+Lemma appF_nil_l : forall f,
+    appF Fnil f = f.
+Proof.
+  intros. simpl. auto.
+Qed.
+
+Lemma derives_app :
+  forall g gPre gSuf wPre wSuf fPre fSuf,
+    (@derivesForest g) gPre wPre fPre
+    -> (@derivesForest g) gSuf wSuf fSuf
+    -> (@derivesForest g) (gPre ++ gSuf)
+                          (wPre ++ wSuf)
+                          (appF fPre fSuf).
+Proof.
+  induction gPre; intros; simpl in *.
+  - inv H.
+    auto.
+  - inv H.
+    simpl.
+    rewrite <- app_assoc.
+    constructor.
+    + auto.
+    + apply IHgPre; auto.
+Qed.
+
+Lemma prefixes_eq :
+  forall (suf pre pre' : list string),
+    app pre suf = app pre' suf
+    -> pre = pre'.
+Proof.
+  induction suf; intros; simpl in *.
+  - repeat rewrite app_nil_r in H.
+    auto.
+  - assert (a :: suf = app [a] suf) by auto.
+    repeat rewrite H0 in H.
+    repeat rewrite app_assoc in H.
+    apply IHsuf in H.
+    apply app_inj_tail in H.
+    destruct H.
+    auto.
+Qed.
+
+Lemma suffixes_eq :
+  forall (pre suf suf' : list string),
+    app pre suf = app pre suf'
+    -> suf = suf'.
+Proof.
+  induction pre; intros; simpl in *.
+  - auto.
+  - inv H.
+    apply IHpre; auto.
+Qed.
+
+(* This is a version of the determinism proof from the
+   Rosenkrantz paper, which describes only the determinism
+   of the derivation, not the structure of the generated
+   parse tree *)
+Lemma rosenkrantz_lemma_4 :
+  forall tbl g,
+    isParseTableFor tbl g
+    -> forall lx gpre rx gamma gsuf
+              wpre wmid wsuf
+              fpre fmid fsuf,
+      In (lx, gpre ++ NT rx :: gsuf) (productions g)
+      -> In (rx, gamma) (productions g)
+      -> (@derivesForest g) gpre wpre fpre
+      -> (@derivesForest g) gamma wmid fmid
+      -> (@derivesForest g) gsuf wsuf fsuf
+      -> forall gamma' fmid',
+          In (rx, gamma') (productions g)
+          -> (@derivesForest g) gamma' wmid fmid'
+          -> gamma = gamma'.
+Proof.
+  intros.
+  destruct H as [Hmin Hcom].
+  destruct wmid as [| tok toks].
+  - apply derivesForest_nil_nullable in H3.
+    apply derivesForest_nil_nullable in H6.
+    assert (Hlk : (@isLookaheadFor g) EOF (NT rx) gamma).
+      { unfold isLookaheadFor.
+        right.
+        split.
+        - constructor; auto.
+        - constructor; auto.
+          repeat (econstructor; eauto). }
+      assert (Hlk' : (@isLookaheadFor g) EOF (NT rx) gamma').
+      { unfold isLookaheadFor.
+        right.
+        split.
+        - constructor; auto.
+        - constructor; auto.
+          repeat (econstructor; eauto). }
+      unfold ptComplete in Hcom.
+      apply Hcom in Hlk.
+      apply Hcom in Hlk'.
+      destruct Hlk as [laMap [Hsf Hlf]].
+      destruct Hlk' as [laMap' [Hsf' Hlf']].
+      assert (gamma = gamma') by congruence.
+      auto.
+  - apply derivesForest_cons_firstGamma in H3.
+    apply derivesForest_cons_firstGamma in H6.
+    assert (Hlk : (@isLookaheadFor g) (LA tok) (NT rx) gamma).
+    { unfold isLookaheadFor.
+      left.
+      constructor; auto. }
+    assert (Hlk' : (@isLookaheadFor g) (LA tok) (NT rx) gamma').
+    { unfold isLookaheadFor.
+      left.
+        constructor; auto. }
+      unfold ptComplete in Hcom.
+      apply Hcom in Hlk.
+      apply Hcom in Hlk'.
+      destruct Hlk as [laMap [Hsf Hlf]].
+      destruct Hlk' as [laMap' [Hsf' Hlf']].
+      assert (gamma = gamma') by congruence.
+      auto.
+Qed.
+
+(* This is a modified version of the previous lemma that 
+   doesn't require wmid to be the same in the statements 
+   about gamma and gamma'. It says that whenever wmid and
+   wmid' are two possibly different prefixes of the same 
+   word, gamma and gamma' must be equal.
+
+   Maybe I can also prove that wmid = wmid' and 
+   wsuf = wsuf' ? *)
+Lemma rosenkrantz_lemma_4' :
+  forall tbl g,
+    isParseTableFor tbl g
+    -> forall lx gpre rx gamma gsuf
+              wpre wmid wsuf
+              fpre fmid fsuf,
+      In (lx, gpre ++ NT rx :: gsuf) (productions g)
+      -> In (rx, gamma) (productions g)
+      -> (@derivesForest g) gpre wpre fpre
+      -> (@derivesForest g) gamma wmid fmid
+      -> (@derivesForest g) gsuf wsuf fsuf
+      -> forall wmid' wsuf' gamma' fmid' fsuf',
+          In (rx, gamma') (productions g)
+          -> (@derivesForest g) gamma' wmid' fmid'
+          -> (@derivesForest g) gsuf wsuf' fsuf'
+          -> wmid ++ wsuf = wmid' ++ wsuf'
+          -> gamma = gamma'.
+Proof.
+  intros.
+  pose proof H as H'.
+  destruct H as [Hmin Hcom].
+  destruct wmid as [| mtok mtoks].
+  - destruct wmid' as [| mtok' mtoks'].
+    + apply derivesForest_nil_nullable in H3.
+      apply derivesForest_nil_nullable in H6.
+      assert (Hlk : (@isLookaheadFor g) EOF (NT rx) gamma).
+      { unfold isLookaheadFor.
+        right.
+        split.
+        - constructor; auto.
+        - constructor; auto.
+          repeat (econstructor; eauto). }
+      assert (Hlk' : (@isLookaheadFor g) EOF (NT rx) gamma').
+      { unfold isLookaheadFor.
+        right.
+        split.
+        - constructor; auto.
+        - constructor; auto.
+          repeat (econstructor; eauto). }
+      unfold ptComplete in Hcom.
+      apply Hcom in Hlk.
+      apply Hcom in Hlk'.
+      destruct Hlk as [laMap [Hsf Hlf]].
+      destruct Hlk' as [laMap' [Hsf' Hlf']].
+      assert (gamma = gamma') by congruence.
+      auto.
+    + destruct wsuf as [| stok stoks].
+      * inv H8.
+      * (* first/follow conflict *)
+        exfalso.
+        inv H8.
+        assert (Hlk : (@isLookaheadFor g)
+                        (LA mtok')
+                        (NT rx)
+                        gamma).
+          { unfold isLookaheadFor.
+            right.
+            split.
+            { constructor; auto.
+              apply derivesForest_nil_nullable in H3.
+              auto. }
+            { constructor; auto.
+              eapply FoRight; eauto.
+              apply derivesForest_cons_firstGamma in H4.
+              auto. }}
+          assert (Hlk' : (@isLookaheadFor g)
+                           (LA mtok')
+                           (NT rx)
+                           gamma').
+          { unfold isLookaheadFor.
+            left.
+            constructor; auto.
+            apply derivesForest_cons_firstGamma in H6.
+            auto. }
+          unfold ptComplete in Hcom.
+          apply Hcom in Hlk; apply Hcom in Hlk'.
+          destruct Hlk as [laMap [Hsf Hlf]].
+          destruct Hlk' as [laMap' [Hsf' Hlf']].
+          assert (gamma = gamma') by congruence.
+          subst.
+          assert ((@firstProd g)
+                    (LA mtok')
+                    (NT rx) gamma').
+          { constructor; auto.
+            apply derivesForest_cons_firstGamma in H6.
+            auto. }
+          assert ((@nullableProd g) (NT rx) gamma').
+          { constructor; auto.
+            apply derivesForest_nil_nullable in H3.
+            auto. }
+          assert ((@followProd g)
+                    (LA mtok')
+                    (NT rx) gamma').
+          { constructor; auto.
+            econstructor; eauto.
+            apply derivesForest_cons_firstGamma in H4.
+            auto. }
+          eapply no_first_follow_conflicts; eauto.
+  - destruct wmid' as [| mtok' mtoks']; simpl in *; subst.
+    + (* another first/follow conflict *)
+      exfalso.
+      assert (Hlk : (@isLookaheadFor g)
+                      (LA mtok)
+                      (NT rx)
+                      gamma').
+      { unfold isLookaheadFor.
+        right.
+        split.
+        { constructor; auto.
+          apply derivesForest_nil_nullable in H6.
+          auto. }
+        { constructor; auto.
+          eapply FoRight; eauto.
+          apply derivesForest_cons_firstGamma in H7.
+          auto. }}
+      assert (Hlk' : (@isLookaheadFor g)
+                       (LA mtok)
+                       (NT rx)
+                       gamma).
+      { unfold isLookaheadFor.
+        left.
+        constructor; auto.
+        apply derivesForest_cons_firstGamma in H3.
+        auto. }
+      unfold ptComplete in Hcom.
+      apply Hcom in Hlk; apply Hcom in Hlk'.
+      destruct Hlk as [laMap [Hsf Hlf]].
+      destruct Hlk' as [laMap' [Hsf' Hlf']].
+      assert (gamma = gamma') by congruence.
+      subst.
+      assert ((@firstProd g)
+                (LA mtok)
+                (NT rx) gamma').
+      { constructor; auto.
+        apply derivesForest_cons_firstGamma in H3.
+        auto. }
+      assert ((@nullableProd g) (NT rx) gamma').
+      { constructor; auto.
+        apply derivesForest_nil_nullable in H6.
+        auto. }
+      assert ((@followProd g)
+                (LA mtok)
+                (NT rx) gamma').
+      { constructor; auto.
+        econstructor; eauto.
+        apply derivesForest_cons_firstGamma in H7.
+        auto. }
+      eapply no_first_follow_conflicts; eauto.
+    + inv H8.
+      apply derivesForest_cons_firstGamma in H3.
+      apply derivesForest_cons_firstGamma in H6.
+      assert (Hlk : (@isLookaheadFor g)
+                      (LA mtok')
+                      (NT rx)
+                      gamma).
+      { unfold isLookaheadFor.
+        left.
+        constructor; auto. }
+      assert (Hlk' : (@isLookaheadFor g)
+                       (LA mtok')
+                       (NT rx)
+                       gamma').
+      { unfold isLookaheadFor.
+        left.
+        constructor; auto. }
+      unfold ptComplete in Hcom.
+      apply Hcom in Hlk.
+      apply Hcom in Hlk'.
+      destruct Hlk as [laMap [Hsf Hlf]].
+      destruct Hlk' as [laMap' [Hsf' Hlf']].
+      assert (gamma = gamma') by congruence.
+      auto.
+Qed.
+
+(* THE NEXT SECTION CONTAINS DIFFERENT ATTEMPTS AT PROVING
+   DETERMINISM OF LL(1) DERIVATIONS *)
+
+(* Here's a natural-seeming way of stating the
+   determinism property, although it turns out to be
+   incomplete *)
+Lemma derives_det :
+  forall tbl g,
+    isParseTableFor tbl g
+    -> forall tr tr' sym word,
+      (@derivesTree g) sym word tr
+      -> (@derivesTree g) sym word tr'
+      -> tr = tr'.
+Proof.
+  intros tbl g Htbl.
+  pose proof Htbl as Htbl'.
+  destruct Htbl as [Hmin Hcom].
+  induction tr using tree_mutual_ind with
+      (P0 := fun f =>
+               forall f' gamma word,
+                 (@derivesForest g) gamma word f
+                 -> (@derivesForest g) gamma word f'
+                 -> f = f'); intros.
+  - inv H; inv H0; auto.
+
+  - inv H; inv H0.
+    (* We can derive the fact that gamma = gamma0 from the
+       fact that the grammar is LL(1). I'll demonstrate how
+       to do this in the next example. *)
+    assert (gamma0 = gamma) by admit. 
+    subst.
+    erewrite IHtr; eauto.
+
+  - inv H; inv H0; auto.
+
+  - inv H.
+    inv H0.
+    (* Here, we're going to get stuck because we don't know
+       whether prefix = prefix0, so we can't use either IH.
+       In general, though, our P0 property isn't necessarily
+       true of any gamma -- only a gamma that appears as part
+       of a right-hand side of some grammar production. *)
+Abort.
+
+(* In this attempt, I show how to prove that when two 
+   productions with the same left-hand nonterminal
+   derive a word, their right-hand sides must be the same.
+
+   I also modify the P0 to specify that gamma must be part
+   of the right-hand side of some production. *)
+Lemma derives_det :
+  forall tbl g,
+    isParseTableFor tbl g
+    -> forall tr tr' sym word,
+      (@derivesTree g) sym word tr
+      -> (@derivesTree g) sym word tr'
+      -> tr = tr'.
+Proof.
+  intros tbl g Htbl.
+  pose proof Htbl as Htbl'.
+  destruct Htbl as [Hmin Hcom].
+  induction tr using tree_mutual_ind with
+      (P0 := fun fsuf =>
+               forall fsuf' x gpre gsuf wsuf,
+                 In (x, gpre ++ gsuf) (productions g)
+                 -> derivesForest gsuf wsuf fsuf
+                 -> derivesForest gsuf wsuf fsuf'
+                 -> fsuf = fsuf'); intros.
+  
+  - inv H; inv H0; auto.
+
+  - inv H; inv H0.
+    (* Here, we can prove that gamma = gamma0 using an approach
+       similar to the one in the Rosenkrantz lemma above. *)
+    assert (gamma0 = gamma).
+    { destruct word as [| tok toks].
+      apply derivesForest_nil_nullable in H2.
+      apply derivesForest_nil_nullable in H6.
+      assert (Hlk : (@isLookaheadFor g) EOF (NT s) gamma).
+      { unfold isLookaheadFor.
+        right.
+        split.
+        - constructor; auto.
+        - constructor; auto.
+          repeat (econstructor; eauto). }
+      assert (Hlk' : (@isLookaheadFor g) EOF (NT s) gamma0).
+      { unfold isLookaheadFor.
+        right.
+        split.
+        - constructor; auto.
+        - constructor; auto.
+          repeat (econstructor; eauto). }
+      unfold ptComplete in Hcom.
+      apply Hcom in Hlk.
+      apply Hcom in Hlk'.
+      destruct Hlk as [laMap [Hsf Hlf]].
+      destruct Hlk' as [laMap' [Hsf' Hlf']].
+      assert (gamma = gamma0) by congruence.
+      auto.
+  - apply derivesForest_cons_firstGamma in H2.
+    apply derivesForest_cons_firstGamma in H6.
+    assert (Hlk : (@isLookaheadFor g) (LA tok) (NT s) gamma).
+    { unfold isLookaheadFor.
+      left.
+      constructor; auto. }
+    assert (Hlk' : (@isLookaheadFor g) (LA tok) (NT s) gamma0).
+    { unfold isLookaheadFor.
+      left.
+        constructor; auto. }
+      unfold ptComplete in Hcom.
+      apply Hcom in Hlk.
+      apply Hcom in Hlk'.
+      destruct Hlk as [laMap [Hsf Hlf]].
+      destruct Hlk' as [laMap' [Hsf' Hlf']].
+      assert (gamma = gamma0) by congruence.
+      auto. }
+    subst.
+    erewrite IHtr with (gpre := nil); eauto.
+
+  - inv H0; inv H1; auto.
+
+  - inv H0.
+    inv H1.
+    (* Here, we're still stuck because we don't know whether
+       the prefixes are equal (or whether the suffixes are
+       equal). This makes the IH's useless, because they only
+       apply when we already know that the strings are equal,
+       so they need to be generalized. *)
+Abort.
+
+(* In this attempt, I try to prove that each symbol on the
+   right-hand side of a production and the symbols to its
+   right can only split the input in one way. *)
+Lemma derives_det :
+  forall tbl g,
+    isParseTableFor tbl g
+    -> forall tr tr' x gpre sym gsuf
+              wpre wpre' wsuf wsuf'
+              fsuf fsuf',
+      In (x, gpre ++ sym :: gsuf) (productions g)
+      -> (@derivesTree g) sym wpre tr
+      -> (@derivesTree g) sym wpre' tr'
+      -> (@derivesForest g) gsuf wsuf fsuf
+      -> (@derivesForest g) gsuf wsuf' fsuf'
+      -> wpre ++ wsuf = wpre' ++ wsuf'
+      -> wpre = wpre'
+         /\ wsuf = wsuf'
+         /\ tr = tr'.
+Proof.
+  intros tbl g Htbl.
+  pose proof Htbl as Htbl'.
+  destruct Htbl as [Hmin Hcom].
+  induction tr using tree_mutual_ind with
+      (P0 := fun fsuf =>
+               forall fsuf' x gpre gsuf
+                      wpre wpre' wsuf wsuf'
+                      fpre fpre',
+                 In (x, gpre ++ gsuf) (productions g)
+                 -> derivesForest gpre wpre fpre
+                 -> derivesForest gpre wpre' fpre'
+                 -> derivesForest gsuf wsuf fsuf
+                 -> derivesForest gsuf wsuf' fsuf'
+                 -> wpre ++ wsuf = wpre' ++ wsuf'
+                 -> wpre = wpre'
+                    /\ wsuf = wsuf'
+                    /\ fsuf = fsuf'); intros.
+  
+  - inv H0; inv H1.
+    inv H4.
+    repeat (split; auto).
+
+  - inv H0; inv H1.
+    assert (gamma0 = gamma) by admit; subst.
+    (* This is looking good, but if we try to apply IHtr
+       to one of our other hypotheses, we run into trouble
+       because it expects gpre and gsuf to appear in the
+       same production, whereas the gamma in our hypotheses
+       appears a level below gsuf. *)
+    eapply IHtr with
+        (gpre := nil)
+        (wpre := nil)
+        (wpre' := nil) in H6; eauto.
+    + destruct H6.
+      destruct H1.
+      subst.
+      apply suffixes_eq in H4.
+      repeat (split; auto).
+    + constructor.
+    + constructor.
+    + (* We can't prove this append fact, so we're stuck *)
+Abort.
+
+(* In this attempt, I try to prove that each symbol on the
+   right-hand side of a production and the symbols to its
+   right can only split the input in one way. *)
+Lemma derives_det :
+  forall tbl g,
+    isParseTableFor tbl g
+    -> forall tr tr' x gpre sym gsuf
+              wpre wpre' wsuf wsuf'
+              fsuf fsuf',
+      In (x, gpre ++ sym :: gsuf) (productions g)
+      -> (@derivesTree g) sym wpre tr
+      -> (@derivesTree g) sym wpre' tr'
+      -> (@derivesForest g) gsuf wsuf fsuf
+      -> (@derivesForest g) gsuf wsuf' fsuf'
+      -> wpre ++ wsuf = wpre' ++ wsuf'
+      -> wpre = wpre'
+         /\ wsuf = wsuf'
+         /\ tr = tr'.
+Proof.
+  intros tbl g Htbl.
+  pose proof Htbl as Htbl'.
+  destruct Htbl as [Hmin Hcom].
+  induction tr using tree_mutual_ind with
+      (P0 := fun fsuf =>
+               forall fsuf' x gpre gsuf
+                      wpre wpre' wsuf wsuf'
+                      fpre fpre',
+                 In (x, gpre ++ gsuf) (productions g)
+                 -> derivesForest gpre wpre fpre
+                 -> derivesForest gpre wpre' fpre'
+                 -> derivesForest gsuf wsuf fsuf
+                 -> derivesForest gsuf wsuf' fsuf'
+                 -> wpre ++ wsuf = wpre' ++ wsuf'
+                 -> wpre = wpre'
+                    /\ wsuf = wsuf'
+                    /\ fsuf = fsuf'); intros.
+  
+  - inv H0; inv H1.
+    inv H4.
+    repeat (split; auto).
+
+  - inv H0; inv H1.
+    assert (gamma0 = gamma) by admit; subst.
+    (* This is looking good, but if we try to apply IHtr
+       to one of our other hypotheses, we run into trouble
+       because it expects gpre and gsuf to appear in the
+       same production, whereas the gamma in our hypotheses
+       appears a level below gsuf. *)
+    eapply IHtr with
+        (gpre := nil)
+        (wpre := nil)
+        (wpre' := nil) in H6; eauto.
+    + destruct H6.
+      destruct H1.
+      subst.
+      apply suffixes_eq in H4.
+      repeat (split; auto).
+    + constructor.
+    + constructor.
+    + (* We can't prove this append fact, so we're stuck *)
+Abort.
+
